format-version: 1.2
auto-generated-by: java
default-namespace: yam_trait_ontology
ontology: TEMP
owl-axioms: Prefix(owl:=<http://www.w3.org/2002/07/owl#>)\nPrefix(rdf:=<http://www.w3.org/1999/02/22-rdf-syntax-ns#>)\nPrefix(xml:=<http://www.w3.org/XML/1998/namespace>)\nPrefix(xsd:=<http://www.w3.org/2001/XMLSchema#>)\nPrefix(rdfs:=<http://www.w3.org/2000/01/rdf-schema#>)\n\n\nOntology(\nDeclaration(AnnotationProperty(<http://www.geneontology.org/formats/oboInOwl#auto-generated-by>))\nDeclaration(AnnotationProperty(<http://www.geneontology.org/formats/oboInOwl#id>))\n\n\nAnnotationAssertion(<http://www.geneontology.org/formats/oboInOwl#auto-generated-by> <http://purl.obolibrary.org/obo/CO_343_0003024> \"\"^^xsd:dateTime)\nAnnotationAssertion(<http://www.geneontology.org/formats/oboInOwl#id> <http://purl.obolibrary.org/obo/TEMP.owl#CO_343:0003028> \"CO_343:0000432\"^^xsd:string)\nAnnotationAssertion(<http://www.geneontology.org/formats/oboInOwl#id> <http://purl.obolibrary.org/obo/TEMP.owl#CO_343:0003029> \"CO_343:0010149\"^^xsd:string)\n)

[Term]
id: CO_343:0000000
name: pollinated florets number
namespace: YamTrait
def: "Quantity of Female Flowers which has been pollinated using male flower from a monoecious or dioecious parent" []
synonym: "NpollF" EXACT []
is_a: CO_343:1000008 ! Agronomical_trait
created_by: A. Lopez-Montes

[Term]
id: CO_343:0000003
name: pollinated spikes number
namespace: YamTrait
def: "Quantity of Female spikes where flowers has been pollinated using male flower from a monoecious or dioecious parent" []
synonym: "NPollSpk" EXACT []
synonym: "NPOLS" EXACT []
is_a: CO_343:1000008 ! Agronomical_trait
created_by: A. Lopez-Montes

[Term]
id: CO_343:0000006
name: fruit developed number
namespace: YamTrait
def: "Quantity of developed fruits per crosses" []
synonym: "FrtN" EXACT []
synonym: "Nfrts" EXACT []
is_a: CO_343:1000010 ! Morphological_trait
created_by: A. Lopez-Montes

[Term]
id: CO_343:0000009
name: fruits harvested number
namespace: YamTrait
def: "Number of harvested fruits per cross after physiological maturity" []
synonym: "FrtHvstN" EXACT []
synonym: "Matfrt" EXACT []
synonym: "Matured fruit" EXACT []
is_a: CO_343:1000010 ! Morphological_trait
created_by: A. Lopez-Montes

[Term]
id: CO_343:0000012
name: seed germination rate
namespace: YamTrait
def: "A proportion of sown true (botanical) seed which germinate and produce seedling" []
synonym: "germRate" EXACT []
synonym: "GR" EXACT []
is_a: CO_343:1000008 ! Agronomical_trait
created_by: A. Lopez-Montes

[Term]
id: CO_343:0000015
name: seedling establishment rate
namespace: YamTrait
def: "Establishment rate of seedlings" []
synonym: "sder" EXACT []
synonym: "sderat" EXACT []
is_a: CO_343:1000008 ! Agronomical_trait
created_by: A. Lopez-Montes

[Term]
id: CO_343:0000021
name: yam anthracnose disease severity
namespace: YamTrait
def: "Anthracnose severity caused by the pathogen Colletotricum gloeosporioides. The reaction of plants in a plot to anthracnose infestation (blight or leaf spot) under screenhouse or in the field under natural infestation or artificial inoculation" []
synonym: "AnthracSev" EXACT []
synonym: "YADS" EXACT []
is_a: CO_343:1000005 ! Biotic_stress_trait
created_by: A. Lopez-Montes

[Term]
id: CO_343:0000024
name: tuber shape
namespace: YamTrait
def: "Tuber predominant shape" []
synonym: "TbrSh" EXACT []
synonym: "TUBSHA" EXACT []
is_a: CO_343:1000010 ! Morphological_trait
created_by: A. Lopez-Montes

[Term]
id: CO_343:0000027
name: tuber size
namespace: YamTrait
def: "Tuber size" []
synonym: "TbrSz" EXACT []
synonym: "TUBSIZE" EXACT []
is_a: CO_343:1000010 ! Morphological_trait
created_by: A. Lopez-Montes

[Term]
id: CO_343:0000030
name: canopy architecture
namespace: YamTrait
def: "Organisation or structural arrangements of branchs and leaves distribution giving a specific shape to the above ground part of the plant" []
synonym: "Canarc" EXACT []
synonym: "canopy" EXACT []
is_a: CO_343:1000010 ! Morphological_trait
created_by: A. Lopez-Montes

[Term]
id: CO_343:0000036
name: tuber dormancy period
namespace: YamTrait
def: "Tuber dormancy period" []
synonym: "Dorm" EXACT []
synonym: "TubDorm" EXACT []
is_a: CO_343:1000006 ! Phenological_trait
created_by: A. Lopez-Montes

[Term]
id: CO_343:0000042
name: yam tuber dry rot incidence
namespace: YamTrait
def: "Dry rot caused by nematodes (Scutellonema bradys and Practylenchus spp.) in tubers at harvest" []
synonym: "Dryrot" EXACT []
synonym: "S_Bri" EXACT []
is_a: CO_343:1000005 ! Biotic_stress_trait
created_by: A. Lopez-Montes

[Term]
id: CO_343:0000045
name: yam tuber dry rot severity
namespace: YamTrait
def: "Dry rot caused by nematodes (Scutellonema bradys and Practylenchus spp.) in tubers at harvest" []
synonym: "Dryrot" EXACT []
synonym: "S_Brs" EXACT []
is_a: CO_343:1000005 ! Biotic_stress_trait
created_by: A. Lopez-Montes

[Term]
id: CO_343:0000048
name: root knot nematode incidence
namespace: YamTrait
def: "Root knot incidence caused by Meloidogyne spp." []
synonym: "R_Kni" EXACT []
synonym: "RKNInc" EXACT []
is_a: CO_343:1000005 ! Biotic_stress_trait
created_by: A. Lopez-Montes

[Term]
id: CO_343:0000051
name: root knot nematode severity
namespace: YamTrait
def: "Root knot severity caused by Meloidogyne spp." []
synonym: "R_kns" EXACT []
synonym: "RKNSev" EXACT []
is_a: CO_343:1000005 ! Biotic_stress_trait
created_by: A. Lopez-Montes

[Term]
id: CO_343:0000054
name: tubers planted
namespace: YamTrait
def: "Number of seed tubers planted in a plot or unit area" []
synonym: "NTP" EXACT []
synonym: "seed yam" EXACT []
synonym: "sett-N" EXACT []
is_a: CO_343:1000008 ! Agronomical_trait
created_by: A.Amele

[Term]
id: CO_343:0000057
name: weight of planted tubers
namespace: YamTrait
def: "Weight of seed tubers (whole seed yams or setts ) planted in a plot  or per unit area. Planting  material from a tuber is called sett. Seed tuber could be either small, healthy whole tuber or large tubers cut into pieces (sett)" []
synonym: "Setts planted weight" EXACT []
synonym: "SETW" EXACT []
synonym: "WTP" EXACT []
is_a: CO_343:1000008 ! Agronomical_trait
created_by: A. Lopez-Montes

[Term]
id: CO_343:0000060
name: plant vigor
namespace: YamTrait
def: "The vigour of the vine and leaves of the new plant." []
synonym: "PLNV" EXACT []
synonym: "PVigor" EXACT []
is_a: CO_343:1000008 ! Agronomical_trait
created_by: A. Lopez-Montes

[Term]
id: CO_343:0000063
name: sprout color
namespace: YamTrait
def: "Color of the sprout (vine and leaves)." []
synonym: "SPCOLO" EXACT []
synonym: "SprtCol" EXACT []
is_a: CO_343:1000010 ! Morphological_trait
created_by: A. Lopez-Montes

[Term]
id: CO_343:0000066
name: proportion of emerged plants
namespace: YamTrait
def: "Proportion of plants /sprouts emerged in a plot" []
synonym: "PPE" EXACT []
synonym: "ratio of emerged plants or sprouts" EXACT []
synonym: "SPROUT" EXACT []
is_a: CO_343:1000008 ! Agronomical_trait
created_by: A.Amele, A. Lopez-Mentes

[Term]
id: CO_343:0000069
name: proportion of established plants
namespace: YamTrait
def: "Proportion of plants in a plot well established (plantsgrowing with good vigour and without severe constraints)" []
synonym: "Estbp-ratio" EXACT []
synonym: "Plant establishement ratio" EXACT []
synonym: "STRATE" EXACT []
is_a: CO_343:1000008 ! Agronomical_trait
created_by: A.Amele

[Term]
id: CO_343:0000072
name: stems per plant
namespace: YamTrait
def: "Number of stems (vines) with leaves and branches per plant" []
synonym: "Nstem" EXACT []
synonym: "stnp" EXACT []
is_a: CO_343:1000008 ! Agronomical_trait
created_by: A. Lopez-Montes

[Term]
id: CO_343:0000075
name: yam anthracnose disease incidence
namespace: YamTrait
def: "Anthracnose incidence caused by the pathogen Colletotricum gloeosporioides. % of anthracnose ‘blight’ or ''leaf spot''affected plants in a plot" []
synonym: "AnthracInc" EXACT []
synonym: "YADI" EXACT []
is_a: CO_343:1000005 ! Biotic_stress_trait
created_by: A. Lopez-Montes

[Term]
id: CO_343:0000081
name: virus incidence
namespace: YamTrait
def: "Reaction of the total plants per plot to the virus infection, producing yellow mottle, mosaic and leaves deformation" []
synonym: "VirusInc" EXACT []
synonym: "VRSI" EXACT []
is_a: CO_343:1000005 ! Biotic_stress_trait
created_by: A. Lopez-Montes

[Term]
id: CO_343:0000084
name: virus severity
namespace: YamTrait
def: "Grade of reaction of the plant to the viruses infection, varying from mottle, mosaics until total leaves deformation" []
synonym: "VirusSev" EXACT []
synonym: "VRSS" EXACT []
is_a: CO_343:1000005 ! Biotic_stress_trait
created_by: A. Lopez-Montes

[Term]
id: CO_343:0000087
name: secondary sprouting
namespace: YamTrait
def: "Emergence of secondary sprouts on a plant" []
synonym: "SECSP" EXACT []
synonym: "SecSP" EXACT []
is_a: CO_343:1000008 ! Agronomical_trait
created_by: A.Amele

[Term]
id: CO_343:0000090
name: time to flower initiation
namespace: YamTrait
def: "Time of the first flower initiation on a plant/s in a plot or any of the plants in a plot shows the first flower" []
synonym: "TIMFlrin" EXACT []
is_a: CO_343:1000006 ! Phenological_trait
created_by: A. Lopez-Montes

[Term]
id: CO_343:0000093
name: plant sex
namespace: YamTrait
def: "Predominat plant or flower sex" []
synonym: "flower sex" EXACT []
synonym: "flrsex" EXACT []
synonym: "plntsex" EXACT []
synonym: "Sex" EXACT []
is_a: CO_343:1000008 ! Agronomical_trait
created_by: A.Amele

[Term]
id: CO_343:0000096
name: flowering intensity
namespace: YamTrait
def: "Abundance or degree of flowering" []
synonym: "FLRI" EXACT []
synonym: "Flrint" EXACT []
is_a: CO_343:1000010 ! Morphological_trait
created_by: A. Lopez-Montes

[Term]
id: CO_343:0000099
name: fruit set number
namespace: YamTrait
def: "Intensity or proportion of fruit set or development under open or controlled pollination." []
synonym: "FRTINT" EXACT []
synonym: "NFrtSet" EXACT []
is_a: CO_343:1000010 ! Morphological_trait
created_by: A. Lopez-Montes

[Term]
id: CO_343:0000105
name: presence of bulbil
namespace: YamTrait
def: "Presence of bulbils or aerial tubers in the nodes of the vines" []
synonym: "Aerial tuber formation" EXACT []
synonym: "AeTuber" EXACT []
synonym: "Bulbil" EXACT []
is_a: CO_343:1000008 ! Agronomical_trait
created_by: A. Lopez-Montes

[Term]
id: CO_343:0000108
name: time to bulbil initiation
namespace: YamTrait
def: "Bulbil initiation time" []
synonym: "Aerial tuber initiation time" EXACT []
synonym: "Aetbrin" EXACT []
synonym: "TIMbub" EXACT []
is_a: CO_343:1000006 ! Phenological_trait
created_by: A. Lopez-Montes

[Term]
id: CO_343:0000111
name: foliage senescence time
namespace: YamTrait
def: "Time to all plants in a plot or unit area show full or complete foliage senescence" []
synonym: "DAYHS" EXACT []
synonym: "Times to complete senescence" EXACT []
synonym: "TIMfsen" EXACT []
is_a: CO_343:1000006 ! Phenological_trait
created_by: A. Lopez-Montes

[Term]
id: CO_343:0000117
name: number of bulbil
namespace: YamTrait
def: "Number of bulbils or aerial tubers produced" []
synonym: "Aetbrp" EXACT []
synonym: "Bulbp" EXACT []
synonym: "Number of aerial tuber" EXACT []
is_a: CO_343:1000008 ! Agronomical_trait
created_by: A. Lopez-Montes

[Term]
id: CO_343:0000120
name: bulbil yield
namespace: YamTrait
def: "Yield of vine bulbils or aerial tubers harvest" []
synonym: "Aerial tuber yield" EXACT []
synonym: "AetbrwtPl" EXACT []
synonym: "Bulbwtpl" EXACT []
is_a: CO_343:1000008 ! Agronomical_trait
created_by: A.Amele

[Term]
id: CO_343:0000123
name: stand harvested number
namespace: YamTrait
def: "Number of plants harvested" []
synonym: "No_std" EXACT []
synonym: "NPH" EXACT []
is_a: CO_343:1000008 ! Agronomical_trait
created_by: A. Lopez-Montes

[Term]
id: CO_343:0000126
name: total tubers per plot
namespace: YamTrait
def: "Number of total (all size) tubers in a net plot or unit area" []
synonym: "TNTP" EXACT []
is_a: CO_343:1000008 ! Agronomical_trait
created_by: A.Amele

[Term]
id: CO_343:0000132
name: total tuber yield
namespace: YamTrait
def: "Total tuber yield nonadjusted tons per hectare" []
synonym: "TTYNA" EXACT []
synonym: "TubYld" EXACT []
is_a: CO_343:1000008 ! Agronomical_trait
created_by: A.Amele

[Term]
id: CO_343:0000135
name: big size yam yield
namespace: YamTrait
def: "Big size tubers yield nonadjusted tons per hectare" []
synonym: "BTYld" EXACT []
is_a: CO_343:1000008 ! Agronomical_trait
created_by: A. Lopez-Montes

[Term]
id: CO_343:0000138
name: rotten or diseased tubers per plot
namespace: YamTrait
def: "Number of rotten and/or rotten yam tubers in a net plot or unit area" []
synonym: "NRDT" EXACT []
is_a: CO_343:1000008 ! Agronomical_trait
created_by: A.Amele

[Term]
id: CO_343:0000141
name: tuber surface texture
namespace: YamTrait
def: "Tuber surface smoothness" []
synonym: "TBRST" EXACT []
synonym: "Tbrtxtur" EXACT []
is_a: CO_343:1000008 ! Agronomical_trait
created_by: A. Lopez-Montes

[Term]
id: CO_343:0000144
name: tuber thorniness
namespace: YamTrait
def: "Exsistence of thorns on the tuber surface" []
synonym: "Tbrspns" EXACT []
synonym: "Thorn" EXACT []
synonym: "Tuber spineness" EXACT []
is_a: CO_343:1000008 ! Agronomical_trait
created_by: A. Lopez-Montes

[Term]
id: CO_343:0000147
name: tuber flesh color
namespace: YamTrait
def: "The surface color of the yam tuber flesh" []
synonym: "Tbrfclr" EXACT []
is_a: CO_343:1000007 ! Quality_trait
created_by: A. Lopez-Montes

[Term]
id: CO_343:0000150
name: tuber flesh oxidation
namespace: YamTrait
def: "Tuber flesh enzymatic oxidation rate" []
synonym: "Oxid" EXACT []
synonym: "Tfoxd" EXACT []
is_a: CO_343:1000007 ! Quality_trait
created_by: A.Amele

[Term]
id: CO_343:0000153
name: leaf beetle damage incidence
namespace: YamTrait
def: "Incidence of leaf beetle damage." []
synonym: "Btl_I" EXACT []
synonym: "Lfbtinc" EXACT []
is_a: CO_343:1000005 ! Biotic_stress_trait
created_by: A. Lopez-Montes

[Term]
id: CO_343:0000156
name: leaf beetle damage severity
namespace: YamTrait
def: "Severity of leaf beetle damage." []
synonym: "Btl_S" EXACT []
synonym: "Lfbtsev" EXACT []
is_a: CO_343:1000005 ! Biotic_stress_trait
created_by: A. Lopez-Montes

[Term]
id: CO_343:0000159
name: mealybug tuber infestation incidence
namespace: YamTrait
def: "Incidence of mealybug tuber infestation." []
synonym: "M_Bi" EXACT []
synonym: "MbugInc" EXACT []
is_a: CO_343:1000005 ! Biotic_stress_trait
created_by: A. Lopez-Montes

[Term]
id: CO_343:0000162
name: mealybug tuber infestation severity
namespace: YamTrait
def: "Severity of mealybug tuber infestation." []
synonym: "M_Bs" EXACT []
synonym: "MbugSev" EXACT []
is_a: CO_343:1000005 ! Biotic_stress_trait
created_by: A. Lopez-Montes

[Term]
id: CO_343:0000165
name: tuber beetle incidence
namespace: YamTrait
def: "Incidence of tuber beetle damage." []
synonym: "Tbeti" EXACT []
synonym: "Tubtlinc" EXACT []
is_a: CO_343:1000005 ! Biotic_stress_trait
created_by: A. Lopez-Montes

[Term]
id: CO_343:0000168
name: tuber beetle severity
namespace: YamTrait
def: "Severity of tuber beetle damage." []
synonym: "Tbets" EXACT []
synonym: "Tubtlsev" EXACT []
is_a: CO_343:1000005 ! Biotic_stress_trait
created_by: A. Lopez-Montes

[Term]
id: CO_343:0000174
name: tuber dry matter content
namespace: YamTrait
def: "Proportion of dry matter in the tuber." []
synonym: "TDMC" EXACT []
synonym: "TubDMC" EXACT []
is_a: CO_343:1000008 ! Agronomical_trait
created_by: A. Lopez-Montes

[Term]
id: CO_343:0000180
name: seeds set per fruit
namespace: YamTrait
def: "Number of seeds developed per fruit after hand flowers pollination" []
synonym: "SdSet" EXACT []
is_a: CO_343:1000008 ! Agronomical_trait
created_by: A. Lopez-Montes

[Term]
id: CO_343:0000183
name: tuber hairiness
namespace: YamTrait
def: "Presence of secondary roots on the tuber bark" []
synonym: "RTBS" EXACT []
synonym: "TBR_Hairy" EXACT []
is_a: CO_343:1000010 ! Morphological_trait
created_by: A. Lopez-Montes

[Term]
id: CO_343:0000188
name: tuber appearance
namespace: YamTrait
def: "Tuber surface look in relation to presence or absence of roots, thorns and sprouted buds on the tuber surface" []
synonym: "Tbrappr" EXACT []
is_a: CO_343:1000010 ! Morphological_trait
created_by: A. Lopez-Montes

[Term]
id: CO_343:0000191
name: stickiness of pounded yam
namespace: YamTrait
def: "The degree to which the pounded yam is adhesive or stick to the fingure, mouth surface and teeth" []
synonym: "Con_Stick_PY" EXACT []
synonym: "StickPndedYam" EXACT []
is_a: CO_343:1000007 ! Quality_trait
created_by: A. Lopez-Montes

[Term]
id: CO_343:0000194
name: taste of pounded yam
namespace: YamTrait
def: "Taste of pounded yam when eaten without any additional complementary food" []
synonym: "Con_Taste_PY" EXACT []
synonym: "TastePndedYam" EXACT []
is_a: CO_343:1000007 ! Quality_trait
created_by: A. Lopez-Montes

[Term]
id: CO_343:0000196
name: Tubers planted counting/plot
namespace: YamTrait
def: "The count of the number of tuber planted per plot or unit area" []
synonym: "NTP_cou_tbrplot" EXACT []
synonym: "Sett-N" EXACT []
is_a: CO_343:1000003 ! Variable
relationship: variable_of CO_343:0000054 ! tubers planted
relationship: variable_of CO_343:0010000 ! tubers (seed yams or setts) planted - counting
relationship: variable_of CO_343:0100000 ! number of tubers

[Term]
id: CO_343:0000197
name: Weight of planted tubers computation/ gm
namespace: YamTrait
def: "Measurement of the weight of N planted tubers (whole seed yams or setts)in gm/sett and record the average (in gm/sett) planted in a plot or per unit area, where the planting material from a tuber is called sett and the seed tuber could be either small, healthy whole tuber or large tubers cut into pieces (sett)" []
synonym: "SETW" EXACT []
synonym: "WTP_Comp_gm" EXACT []
is_a: CO_343:1000003 ! Variable
relationship: variable_of CO_343:0000057 ! weight of planted tubers
relationship: variable_of CO_343:0010001 ! setts or seed yams planted weight - computation
relationship: variable_of CO_343:0100001 ! gm/sett

[Term]
id: CO_343:0000198
name: first sprout emergence time
namespace: YamTrait
def: "Time to the  first sprout (plant) emerge in a plot" []
synonym: "DtFSE" EXACT []
synonym: "TIMFSE" EXACT []
is_a: CO_343:1000006 ! Phenological_trait
created_by: A.Amele

[Term]
id: CO_343:0000199
name: First sprout emergence time estimation in yy/mm/dd
namespace: YamTrait
def: "The time of first spout (plant) emergence in a plot is recorded as Date(yyyymmdd)." []
synonym: "DATFSE_date_ymd" EXACT []
synonym: "Emerdt" EXACT []
is_a: CO_343:1000003 ! Variable
relationship: variable_of CO_343:0000198 ! first sprout emergence time
relationship: variable_of CO_343:0010002 ! time first sprout emergence-estimation
relationship: variable_of CO_343:0100002 ! date (yyyymmdd)

[Term]
id: CO_343:0000200
name: 50% sprout emergence time
namespace: YamTrait
def: "Time to 50% sprouts (plants) emerge in a plot" []
synonym: "DtSE" EXACT []
synonym: "TIMSE" EXACT []
is_a: CO_343:1000006 ! Phenological_trait
created_by: A.Amele

[Term]
id: CO_343:0000201
name: 50% sprout emergence time estimation in yy/mm/dd
namespace: YamTrait
def: "The time to 50% of sprouts emergence is recorded as the Date(yyyymmdd) in which it emerged in a plot." []
synonym: "DATSE_date_ymd" EXACT []
synonym: "DtFemer" EXACT []
is_a: CO_343:1000003 ! Variable
relationship: variable_of CO_343:0000200 ! 50% sprout emergence time
relationship: variable_of CO_343:0010003 ! time 50% of sprout emergence-estimation
relationship: variable_of CO_343:0100002 ! date (yyyymmdd)

[Term]
id: CO_343:0000202
name: First sprout emergence time computation in days
namespace: YamTrait
def: "The number of days is computed as the time to the first sprout (plant) emergence, which is required from the date of planting to the date in which the first sprout (plant) emerged in a plot" []
synonym: "Emerday" EXACT []
synonym: "TIMFSE_dt_days" EXACT []
is_a: CO_343:1000003 ! Variable
relationship: variable_of CO_343:0000198 ! first sprout emergence time
relationship: variable_of CO_343:0010004 ! times to first sprout emergence-computation
relationship: variable_of CO_343:0100003 ! days

[Term]
id: CO_343:0000203
name: 50% sprout emergence time computation in days
namespace: YamTrait
def: "The number of days is computed as the time to 50% sprouts (plants) emergence, which is required from date of planting to the date 50% of sprouts (plants) emerged in a plot" []
synonym: "DyFemer" EXACT []
synonym: "TIMSE_dt_days" EXACT []
is_a: CO_343:1000003 ! Variable
relationship: variable_of CO_343:0000200 ! 50% sprout emergence time
relationship: variable_of CO_343:0010005 ! times to 50% spout emergence-computation
relationship: variable_of CO_343:0100003 ! days

[Term]
id: CO_343:0000204
name: number of emerged plants
namespace: YamTrait
def: "Number of an emerged plants (sprouts) in a plot" []
synonym: "NEP" EXACT []
is_a: CO_343:1000008 ! Agronomical_trait
created_by: A.Amele

[Term]
id: CO_343:0000205
name: Emerged plants counting/plot
namespace: YamTrait
def: "The number of emerged plants (sprouts) per plot is counted every week starting from first plant/sprout emergence date till the last plant or spourt emerges in a plot" []
synonym: "NEP_Cou_sprouts" EXACT []
is_a: CO_343:1000003 ! Variable
relationship: variable_of CO_343:0000204 ! number of emerged plants
relationship: variable_of CO_343:0010006 ! emerged sprouts -counting
relationship: variable_of CO_343:0100004 ! plants per plot

[Term]
id: CO_343:0000206
name: Proportion of emerged plants (sprouts) computation/%
namespace: YamTrait
def: "The proportion or ratio of plants/sprouts emerged in percentage is computed as the number of emerged plants/sprouts divided by the total number of tubers (seed yam or setts) planted in a plot multiplied by 100" []
synonym: "PPE_Comp_pct" EXACT []
synonym: "Ratiosp" EXACT []
is_a: CO_343:1000003 ! Variable
relationship: variable_of CO_343:0000066 ! proportion of emerged plants
relationship: variable_of CO_343:0010007 ! emerged sprouts or plants proportion-computation
relationship: variable_of CO_343:0100005 ! percentage

[Term]
id: CO_343:0000207
name: established plants
namespace: YamTrait
def: "Number of well established plants ( plants growing with good vigour and without severe constraints) in a plot" []
synonym: "estbp-N" EXACT []
synonym: "NESP" EXACT []
is_a: CO_343:1000008 ! Agronomical_trait
created_by: A.Amele

[Term]
id: CO_343:0000208
name: Established plants counting/plot
namespace: YamTrait
def: "The number of well established plants per plot is usually counted at two months after planting" []
synonym: "Estbp-N" EXACT []
synonym: "NESP_cou_plts" EXACT []
is_a: CO_343:1000003 ! Variable
relationship: variable_of CO_343:0000207 ! established plants
relationship: variable_of CO_343:0010008 ! number of well established plants -counting
relationship: variable_of CO_343:0100004 ! plants per plot

[Term]
id: CO_343:0000209
name: Field establishment rate compuation in %
namespace: YamTrait
def: "The proportion or ratio of well-established plants (growing with good vigour and without severe constraints) in a plot are computed from the total number of tubers (seed yam or setts) planted expressed in percentage" []
synonym: "Estbp-ratio" EXACT []
synonym: "STRATE_Comp_pct" EXACT []
is_a: CO_343:1000003 ! Variable
relationship: variable_of CO_343:0000069 ! proportion of established plants
relationship: variable_of CO_343:0010009 ! field establishment-computation
relationship: variable_of CO_343:0100006 ! %

[Term]
id: CO_343:0000210
name: Secondary sprouting estimation nominal 0&1
namespace: YamTrait
def: "Visual assessment of the emergence of new secondary sprouts on a plant from the planted seed tuber/sett in a plot at three months after planting using a 0 - 1 scale, where 0=Absent and 1=Present" []
synonym: "SECSP" EXACT []
synonym: "SecSP_E_0to1" EXACT []
is_a: CO_343:1000003 ! Variable
relationship: variable_of CO_343:0000087 ! secondary sprouting
relationship: variable_of CO_343:0010010 ! secondary sprouting - estimation
relationship: variable_of CO_343:0100007 ! 0-1 scale

[Term]
id: CO_343:0000211
name: Sprout color estimation 1-5
namespace: YamTrait
def: "Visual assessment of the predominant color of the sprouts (vine and leaves) per plot at 20 days after emergence using a 1-5 scale, where 1=Green, 2=Purplish green, 3=Brownish green, 4=Dark brown and 5=Purple" []
synonym: "SPCOLO" EXACT []
synonym: "SprtCol_E_1to5" EXACT []
is_a: CO_343:1000003 ! Variable
relationship: variable_of CO_343:0000063 ! sprout color
relationship: variable_of CO_343:0010011 ! sprout color - estimation
relationship: variable_of CO_343:0100008 ! 1-5 scale

[Term]
id: CO_343:0000212
name: sprout length
namespace: YamTrait
def: "Length of sprouted shoots (vines)" []
synonym: "Spleng" EXACT []
synonym: "SPRTL" EXACT []
is_a: CO_343:1000010 ! Morphological_trait
created_by: A.Amele

[Term]
id: CO_343:0000213
name: Sprout length measurement in cm
namespace: YamTrait
def: "The average length of sprouted shoots (vines) in cm of five representative plants measurement taken in a plot is computed" []
synonym: "SPleng_M_cm" EXACT []
synonym: "SPRTL" EXACT []
is_a: CO_343:1000003 ! Variable
relationship: variable_of CO_343:0000212 ! sprout length
relationship: variable_of CO_343:0010012 ! sprout length-computation
relationship: variable_of CO_343:0100009 ! cm

[Term]
id: CO_343:0000214
name: presence of spot on spine base
namespace: YamTrait
def: "Presence of colored spots at the spine base of sprouted shoots (vine) with spines" []
synonym: "SPBCOL" EXACT []
is_a: CO_343:1000010 ! Morphological_trait
created_by: A.Amele

[Term]
id: CO_343:0000215
name: Spine base color estimation nominal 0&1
namespace: YamTrait
def: "Visual assessment of the presence (existence) of colored spot at base of spines on a sprout (vine) using a 0-1 scale, where 0=Absent and 1=Present" []
synonym: "SPBCOL_E_0to1" EXACT []
is_a: CO_343:1000003 ! Variable
relationship: variable_of CO_343:0000214 ! presence of spot on spine base
relationship: variable_of CO_343:0010013 ! colored spots on spine base-estimation
relationship: variable_of CO_343:0100007 ! 0-1 scale

[Term]
id: CO_343:0000216
name: spines on sprout presence
namespace: YamTrait
def: "Presence of spines on sprout (vines)" []
synonym: "SPNSP" EXACT []
is_a: CO_343:1000010 ! Morphological_trait
created_by: A.Amele

[Term]
id: CO_343:0000217
name: Spines on sprout presence estimation nominal 0&1
namespace: YamTrait
def: "Visual assessment of the absence or presence of spines on a sprout (vine) using a 0-1 scale, where 0=Absent and 1=Present" []
synonym: "SPNSP_E_0to1" EXACT []
is_a: CO_343:1000003 ! Variable
relationship: variable_of CO_343:0000216 ! spines on sprout presence
relationship: variable_of CO_343:0010014 ! spines on sprout base-estimation
relationship: variable_of CO_343:0100007 ! 0-1 scale

[Term]
id: CO_343:0000218
name: sprout hairiness
namespace: YamTrait
def: "Hairs on sprout (vines)" []
synonym: "HAIRSP" EXACT []
is_a: CO_343:1000010 ! Morphological_trait
created_by: A.Amele

[Term]
id: CO_343:0000219
name: Sprout hairiness estimation nominal 0&2
namespace: YamTrait
def: "Visual assessment of the existence of hairs on a sprout (vine) using a 0-2 scale, where 0=Absent, 1=Sparse and 2=Dense" []
synonym: "HAIRSP_E_0to2" EXACT []
is_a: CO_343:1000003 ! Variable
relationship: variable_of CO_343:0000218 ! sprout hairiness
relationship: variable_of CO_343:0010015 ! hairiness of sprout - estimation
relationship: variable_of CO_343:0100010 ! 0-2 scale

[Term]
id: CO_343:0000220
name: time to first leaf emergence
namespace: YamTrait
def: "Time to the first leaf emergence on a plant or sprouted shoot (vine) in a plot" []
synonym: "TIMLE" EXACT []
is_a: CO_343:1000006 ! Phenological_trait
created_by: A.Amele

[Term]
id: CO_343:0000221
name: First leaf emergence time estimation in yy/mm/dd
namespace: YamTrait
def: "Visual observation of the time of first leaf emergence on sprouted shoot (vine) using the date(yyyymmdd) it emerges" []
synonym: "DateLE_date_ymd" EXACT []
is_a: CO_343:1000003 ! Variable
relationship: variable_of CO_343:0000220 ! time to first leaf emergence
relationship: variable_of CO_343:0010016 ! time of  first leaf emergence on sprouted shoot (vines)-estimation
relationship: variable_of CO_343:0100002 ! date (yyyymmdd)

[Term]
id: CO_343:0000222
name: Time to first leaf emergence computation
namespace: YamTrait
def: "Computation of the time to the first leaf emergence using the number of days from first sprout emergence to the first leaf that emerges on a sprouted shoot (vine) in a plot" []
synonym: "TIMLE_dt_day" EXACT []
is_a: CO_343:1000003 ! Variable
relationship: variable_of CO_343:0000220 ! time to first leaf emergence
relationship: variable_of CO_343:0010017 ! times to the first leaf emergence on sprouted shoot (vines)-computation
relationship: variable_of CO_343:0100003 ! days

[Term]
id: CO_343:0000223
name: leaf apex shape
namespace: YamTrait
def: "Leaf apex shape" []
synonym: "Lfapx" EXACT []
is_a: CO_343:1000010 ! Morphological_trait
created_by: A.Amele

[Term]
id: CO_343:0000224
name: Leaf apex shape estimation 1-3
namespace: YamTrait
def: "Visual assessment of the leaf apex shape of mature plants in a plot using a 1-3 general scale, where 1=obtuse, 2= acute and 3=emarginate" []
synonym: "Lfapx_E_1to3" EXACT []
is_a: CO_343:1000003 ! Variable
relationship: variable_of CO_343:0000223 ! leaf apex shape
relationship: variable_of CO_343:0010018 ! leaf apex shape-estimation
relationship: variable_of CO_343:0100011 ! 1-3 general scale

[Term]
id: CO_343:0000225
name: leaf shape
namespace: YamTrait
def: "Leaf shape of plants" []
synonym: "Lfshp" EXACT []
is_a: CO_343:1000010 ! Morphological_trait
created_by: A.Amele

[Term]
id: CO_343:0000226
name: Leaf shape estimation 1-7
namespace: YamTrait
def: "Visual assessment of leaf shape of mature plants in a plot using a 1-7 genearal scale, where 1= Ovate, 3= Cordate, 5= Sagittate and 7 = Hastate" []
synonym: "Lfshp_E_1to7" EXACT []
is_a: CO_343:1000003 ! Variable
relationship: variable_of CO_343:0000225 ! leaf shape
relationship: variable_of CO_343:0010019 ! leaf shape-estimation
relationship: variable_of CO_343:0100012 ! 1-7 general scale

[Term]
id: CO_343:0000227
name: Stems per plant computation per plant
namespace: YamTrait
def: "Computation of average of the number of stems (vines) with leaves and branches per established plants in a plot" []
synonym: "Nstem_cou_stmplnt" EXACT []
synonym: "stnp" EXACT []
is_a: CO_343:1000003 ! Variable
relationship: variable_of CO_343:0000072 ! stems per plant
relationship: variable_of CO_343:0010020 ! number of stems per plant-computation
relationship: variable_of CO_343:0100013 ! number of stem

[Term]
id: CO_343:0000228
name: stem diameter
namespace: YamTrait
def: "Stem diameter of a mature plant (5 to 6 month old plant)" []
synonym: "stemdim" EXACT []
synonym: "STMDM" EXACT []
is_a: CO_343:1000008 ! Agronomical_trait
created_by: A.Amele

[Term]
id: CO_343:0000229
name: Stem diameter computation in mm
namespace: YamTrait
def: "Measurement of the stem diameter in mm of a mature plant (5 to 6 month old plant) at 15 cm above the base of five plants before senescence in a plot and the computation of the average" []
synonym: "stemdim" EXACT []
synonym: "STMDM_M_mm" EXACT []
is_a: CO_343:1000003 ! Variable
relationship: variable_of CO_343:0000228 ! stem diameter
relationship: variable_of CO_343:0010021 ! stem diameter-computation
relationship: variable_of CO_343:0100014 ! mm

[Term]
id: CO_343:0000230
name: internode length
namespace: YamTrait
def: "Stem internode length of a mature plant (5 to 6 month old plant)" []
synonym: "INODL" EXACT []
synonym: "Inodlgth" EXACT []
is_a: CO_343:1000010 ! Morphological_trait
created_by: A.Amele

[Term]
id: CO_343:0000231
name: Internode length computation in cm
namespace: YamTrait
def: "Measurement of the stem internode length of five matured plants (5 to 6 month old plant) before senescence at 1 meter height and computation of the average" []
synonym: "INODL" EXACT []
synonym: "InodLgth_M_cm" EXACT []
is_a: CO_343:1000003 ! Variable
relationship: variable_of CO_343:0000230 ! internode length
relationship: variable_of CO_343:0010022 ! internode length -computation
relationship: variable_of CO_343:0100009 ! cm

[Term]
id: CO_343:0000232
name: number of internodes to first branching
namespace: YamTrait
def: "Number of internodes to first branchs on a plant" []
synonym: "NINFB" EXACT []
is_a: CO_343:1000010 ! Morphological_trait
created_by: A.Amele

[Term]
id: CO_343:0000233
name: Number of internodes to first branching computation/plot
namespace: YamTrait
def: "Computation of average number of internodes to first branching of a plant on at least five plants internode counts taken in a plot" []
synonym: "NINFB_E_intrnod" EXACT []
is_a: CO_343:1000003 ! Variable
relationship: variable_of CO_343:0000232 ! number of internodes to first branching
relationship: variable_of CO_343:0010023 ! number of internode-computation
relationship: variable_of CO_343:0100015 ! number of internode

[Term]
id: CO_343:0000234
name: spines on stem density
namespace: YamTrait
def: "Intensity of spines on stem (vine) above base of mature plant (5 to 6 month old plant)" []
synonym: "SPNAB" EXACT []
is_a: CO_343:1000010 ! Morphological_trait
created_by: A.Amele

[Term]
id: CO_343:0000235
name: Spines on stem estimation 0-2
namespace: YamTrait
def: "Visual assessment of the intensity of spines on a stem (vine) above the base of mature plants (5 to 6 month old plant) in a plot using 0-2 scale, where 0 = Absent, 1 = Few and 2 = Many" []
synonym: "SPNAB_E_0to2" EXACT []
is_a: CO_343:1000003 ! Variable
relationship: variable_of CO_343:0000234 ! spines on stem density
relationship: variable_of CO_343:0010024 ! density of spines on stem base of a plant-etimation
relationship: variable_of CO_343:0100010 ! 0-2 scale

[Term]
id: CO_343:0000236
name: plant type
namespace: YamTrait
def: "A tendency of a plant to grow in a certain shape and to attain a certain mature height and spread" []
synonym: "GH" EXACT []
synonym: "Growth habit" EXACT []
synonym: "Plntype" EXACT []
is_a: CO_343:1000008 ! Agronomical_trait
created_by: A.Amele

[Term]
id: CO_343:0000237
name: Plant type estimation 1-3
namespace: YamTrait
def: "Visual assessment of the tendency of a plant to grow in a certain shape and to attain certain matured height and spread using a 1-3 general scale, where 1=dwaft, 2=shrub-like and 3=climbing" []
synonym: "GH" EXACT []
synonym: "Plntype_E_1to3" EXACT []
is_a: CO_343:1000003 ! Variable
relationship: variable_of CO_343:0000236 ! plant type
relationship: variable_of CO_343:0010025 ! plant type-estimation
relationship: variable_of CO_343:0100011 ! 1-3 general scale

[Term]
id: CO_343:0000238
name: Canopy architecture estimation 1-4
namespace: YamTrait
def: "Determination of predominant canopy architecture of the structural arrangements (organisation) of branchs and leaves distribution giving a specific shape to the above ground part of the plant using a 1-4 general scale, where 1= One vine, palmiform, many branches and erect, 2= One vine palmiform erect, large and few branches, 3= Several vines, shorts, many branches, palmiform and erects, and 4= One large vine, few branches, palmiform and postrated." []
synonym: "Canarc_E_1to4" EXACT []
synonym: "Canopy" EXACT []
is_a: CO_343:1000003 ! Variable
relationship: variable_of CO_343:0000030 ! canopy architecture
relationship: variable_of CO_343:0010026 ! canopy architecture - estimation
relationship: variable_of CO_343:0100016 ! 1-4 general scale

[Term]
id: CO_343:0000239
name: Plant vigor estimation 1-3
namespace: YamTrait
def: "Visual assessment of the vigour of the vine and leaves of the new plant in a plot at two month after planting using a 1-3 general scale, where 1=weak, 2= moderate or medium and 3= vigorous" []
synonym: "PLNV" EXACT []
synonym: "PVigor_E_1to3" EXACT []
is_a: CO_343:1000003 ! Variable
relationship: variable_of CO_343:0000060 ! plant vigor
relationship: variable_of CO_343:0010027 ! plant vigor - estimation
relationship: variable_of CO_343:0100011 ! 1-3 general scale

[Term]
id: CO_343:0000240
name: twining habit
namespace: YamTrait
def: "Tendency of climbing or trailling" []
synonym: "climbhab" EXACT []
synonym: "climbing habit" EXACT []
synonym: "trailling" EXACT []
synonym: "TWNH" EXACT []
is_a: CO_343:1000008 ! Agronomical_trait
created_by: A.Amele

[Term]
id: CO_343:0000241
name: Twining habit estimation 0-1
namespace: YamTrait
def: "Visual assessment of the tendency of vine to twine or climb using a 0-1 nominal scale, where 0= No and 1= Yes" []
synonym: "TWNH" EXACT []
synonym: "TWNH_E_0to1" EXACT []
is_a: CO_343:1000003 ! Variable
relationship: variable_of CO_343:0000240 ! twining habit
relationship: variable_of CO_343:0010028 ! twining habit-estimation
relationship: variable_of CO_343:0100017 ! 0-1 nominal scale

[Term]
id: CO_343:0000242
name: twining direction
namespace: YamTrait
def: "Twining direction" []
synonym: "climbdir" EXACT []
synonym: "twndir" EXACT []
synonym: "vine climbing direction" EXACT []
is_a: CO_343:1000010 ! Morphological_trait
created_by: A. Amele

[Term]
id: CO_343:0000243
name: Twining direction estimation 1-2
namespace: YamTrait
def: "Visual assessment of the twining (climbing) direction of the vine using a 1-2 nominal scale, where 1= Clockwise (climbing to the left) and 2= Anticlockwise (climbing to the right)" []
synonym: "Twndir_E_1to2" EXACT []
is_a: CO_343:1000003 ! Variable
relationship: variable_of CO_343:0000242 ! twining direction
relationship: variable_of CO_343:0010029 ! twining direction-estimation
relationship: variable_of CO_343:0100018 ! 1-2 nominal scale

[Term]
id: CO_343:0000244
name: Flower initiation time estimation in yy/mm/dd
namespace: YamTrait
def: "Visual assessment of time (date) of first flower initiation on a plant (or any of the plants in a plot shows the first flower)" []
synonym: "Datflrin_date_ymd" EXACT []
synonym: "DtFlrin" EXACT []
is_a: CO_343:1000003 ! Variable
relationship: variable_of CO_343:0000090 ! time to flower initiation
relationship: variable_of CO_343:0010030 ! flower initaition time - estimation
relationship: variable_of CO_343:0100002 ! date (yyyymmdd)

[Term]
id: CO_343:0000245
name: time to 50% flowering
namespace: YamTrait
def: "Time when 50% of the plants flower in a plot" []
synonym: "DF" EXACT []
synonym: "TIMFL" EXACT []
is_a: CO_343:1000006 ! Phenological_trait
created_by: A.Amele

[Term]
id: CO_343:0000246
name: Flowering time estimation in yy/mm/dd
namespace: YamTrait
def: "Visual assessment of time (date) when 50% plants in a plot are having at least one flower/inflorescence as Date(yyyymmdd)" []
synonym: "Datflr_date_ymd" EXACT []
synonym: "DtFFlr" EXACT []
is_a: CO_343:1000003 ! Variable
relationship: variable_of CO_343:0000245 ! time to 50% flowering
relationship: variable_of CO_343:0010031 ! 50% flowering time - estimation
relationship: variable_of CO_343:0100002 ! date (yyyymmdd)

[Term]
id: CO_343:0000247
name: time to end of flowering
namespace: YamTrait
def: "End of flowering time or when a plant does not produce new flower in a plot" []
synonym: "TIMEF" EXACT []
is_a: CO_343:1000006 ! Phenological_trait
created_by: A. Lopez-Montes

[Term]
id: CO_343:0000248
name: End of flowering time estimation in yy/mm/dd
namespace: YamTrait
def: "Visual assessment of time or date (yyyymmdd) when the plant does not produce more new flowers in a plot" []
synonym: "Datendflr_date_ymd" EXACT []
synonym: "DtendFlr" EXACT []
is_a: CO_343:1000003 ! Variable
relationship: variable_of CO_343:0000247 ! time to end of flowering
relationship: variable_of CO_343:0010032 ! end of flowering time - estimation
relationship: variable_of CO_343:0100002 ! date (yyyymmdd)

[Term]
id: CO_343:0000249
name: Flower initiation time computation in days
namespace: YamTrait
def: "Computation of the number of days required from first sprout emergence to first flower initiation as the time of the first flower initiation on a plant/s in a plot or any of the plants in a plot shows the first flower" []
synonym: "Dayflrin" EXACT []
synonym: "TIMflrin_dt_days" EXACT []
is_a: CO_343:1000003 ! Variable
relationship: variable_of CO_343:0000090 ! time to flower initiation
relationship: variable_of CO_343:0010033 ! flower initaition time - computation
relationship: variable_of CO_343:0100003 ! days

[Term]
id: CO_343:0000250
name: Flowering time computation in days
namespace: YamTrait
def: "Computation the number of days (time) required from 50% of sprouts in plot emerged to when 50% of plants in a plot are having at least one flower/inflorescence" []
synonym: "DF" EXACT []
synonym: "TIMFlr_dt_days" EXACT []
is_a: CO_343:1000003 ! Variable
relationship: variable_of CO_343:0000245 ! time to 50% flowering
relationship: variable_of CO_343:0010034 ! 50% flowering time - computation
relationship: variable_of CO_343:0100003 ! days

[Term]
id: CO_343:0000251
name: End of flowering time computation in days
namespace: YamTrait
def: "Computation the number of days required from 50% of sprout emergence to when plant does not produce more new flowers as the end of its flowering time" []
synonym: "Dayendflr" EXACT []
synonym: "TIMendflr_dt_days" EXACT []
is_a: CO_343:1000003 ! Variable
relationship: variable_of CO_343:0000247 ! time to end of flowering
relationship: variable_of CO_343:0010035 ! end of flowering time - computation
relationship: variable_of CO_343:0100003 ! days

[Term]
id: CO_343:0000252
name: crossing date
namespace: YamTrait
def: "Date crossing or pollination attempted" []
synonym: "datcross" EXACT []
synonym: "Polldate" EXACT []
is_a: CO_343:1000006 ! Phenological_trait
created_by: A.Amele

[Term]
id: CO_343:0000253
name: Crossing date esimation in yy/mm/dd
namespace: YamTrait
def: "Visual assessment of the date (yyymmdd) crossing made in particular flower of a plant or pollination was attempted" []
synonym: "datcross_date_ymd" EXACT []
synonym: "Polldate" EXACT []
is_a: CO_343:1000003 ! Variable
relationship: variable_of CO_343:0000252 ! crossing date
relationship: variable_of CO_343:0010036 ! date crossing-estimation
relationship: variable_of CO_343:0100002 ! date (yyyymmdd)

[Term]
id: CO_343:0000254
name: Pollinated florets counting
namespace: YamTrait
def: "The number of pollinated florets per female parent per cross is counted as the quantity of Female Flowers which has been pollinated using male flower from a monoecious or dioecious parent" []
synonym: "NPollF_Cou_flrplnt" EXACT []
is_a: CO_343:1000003 ! Variable
relationship: variable_of CO_343:0000000 ! pollinated florets number
relationship: variable_of CO_343:0010037 ! floret pollinated number - counting
relationship: variable_of CO_343:0100019 ! number of florets

[Term]
id: CO_343:0000255
name: Pollinated spikes counting
namespace: YamTrait
def: "The number of pollinated spikes per female parent per cross is counted as the quantity of Female spikes where flowers has been pollinated using male flower from a monoecious or dioecious parent" []
synonym: "NPollSpk_Cou_Pollspk" EXACT []
synonym: "NPOLS" EXACT []
is_a: CO_343:1000003 ! Variable
relationship: variable_of CO_343:0000003 ! pollinated spikes number
relationship: variable_of CO_343:0010038 ! pollinated spike number - estimation
relationship: variable_of CO_343:0100020 ! number of spikes

[Term]
id: CO_343:0000256
name: Flowering intensity estimation 0-9
namespace: YamTrait
def: "Visual assessment of the abundance or intensity (degree) of flowering when more than 50% of the plants are flowered in a plot using a 0-9 scale , where 0= No flower or bud (No inflorescence and not flowering at all), 1= aborted flower (Presence of small or rudimentary inflorescences/flowers that can show an abortion or abscission point at joint of the pedicel), 3= Low (flowering is scare with the presence of few flowers mostly less than 10 inflorescences per plant), 5= Moderate (producing some flowers mostly 10-29 inflorescences per plant), 7 = Profuse (plant producing many more flowers mostly 30 to 50 inflorescences per plant) and 9 = Extremely pofuse (plant producing with abundant flowring mostly more than 50 inflorescences per plant)." []
synonym: "FLRI" EXACT []
synonym: "Flrint_E_0to9" EXACT []
is_a: CO_343:1000003 ! Variable
relationship: variable_of CO_343:0000096 ! flowering intensity
relationship: variable_of CO_343:0010039 ! flowering intensity - estimation
relationship: variable_of CO_343:0100021 ! 0-9 scale

[Term]
id: CO_343:0000257
name: inflorescence initiation time
namespace: YamTrait
def: "Time of first inflorescence initiation" []
synonym: "Datinflor" EXACT []
is_a: CO_343:1000006 ! Phenological_trait
created_by: A.Amele

[Term]
id: CO_343:0000258
name: First inflorescence initiation time estimation in yy/mm/dd
namespace: YamTrait
def: "Visual observation of time or date(yyyymmdd) when plant is having the first inflorescence initiation in a plot." []
synonym: "Datinflor_E_ymd" EXACT []
is_a: CO_343:1000003 ! Variable
relationship: variable_of CO_343:0000257 ! inflorescence initiation time
relationship: variable_of CO_343:0010040 ! first inflorescence time - estimation
relationship: variable_of CO_343:0100002 ! date (yyyymmdd)

[Term]
id: CO_343:0000259
name: First inflorescence initiation time computation
namespace: YamTrait
def: "Computation of the number of days as the time required to first inflorescence emergence in a plot." []
synonym: "TIMinflor_E_days" EXACT []
is_a: CO_343:1000003 ! Variable
relationship: variable_of CO_343:0000257 ! inflorescence initiation time
relationship: variable_of CO_343:0010041 ! first inflorescence time - compuation
relationship: variable_of CO_343:0100003 ! days

[Term]
id: CO_343:0000260
name: inflorescence type
namespace: YamTrait
def: "The arrangement of flowers on stem or twig of a plant" []
synonym: "Inft" EXACT []
is_a: CO_343:1000010 ! Morphological_trait
created_by: A.Amele

[Term]
id: CO_343:0000261
name: Inflorescence type estimation
namespace: YamTrait
def: "Visual observation of the type of inflorescence and score it as the arrangement of flowers on stem or twig of a plant using a 1-3 scale, where 1= spike, 2= raceme and 3= panicle." []
synonym: "Inflortyp_E_1to3" EXACT []
is_a: CO_343:1000003 ! Variable
relationship: variable_of CO_343:0000260 ! inflorescence type
relationship: variable_of CO_343:0010042 ! inflorescence type-estimation
relationship: variable_of CO_343:0100022 ! 1-3 scale

[Term]
id: CO_343:0000262
name: female flowering intensity
namespace: YamTrait
def: "Intensity or abudance of female flowers on spikes/infloresences" []
synonym: "femal flower abudance per inflorence" EXACT []
synonym: "fflrab" EXACT []
synonym: "fflrint" EXACT []
is_a: CO_343:1000010 ! Morphological_trait
created_by: A.Amele

[Term]
id: CO_343:0000263
name: Female flowering intensity per spike estimation 1-4
namespace: YamTrait
def: "Visual observation of the female flowering intensity or abudance per inflorences (spikes) and rating using a 1-4 general scale, where 1= ≤10 flowers, 2=11-25 flowers, 3=26-100 flowers and 4 = ≥ 101 flowers." []
synonym: "fflrab" EXACT []
synonym: "Fflrint_E_1to4" EXACT []
is_a: CO_343:1000003 ! Variable
relationship: variable_of CO_343:0000262 ! female flowering intensity
relationship: variable_of CO_343:0010043 ! femal flowers abundance or intensity per inflorescence-estimation
relationship: variable_of CO_343:0100016 ! 1-4 general scale

[Term]
id: CO_343:0000264
name: pollination type
namespace: YamTrait
def: "Mode of plant to plant pollen transfer" []
synonym: "Mechanism of pollination" EXACT []
synonym: "Pollmech" EXACT []
synonym: "Polltyp" EXACT []
is_a: CO_343:1000008 ! Agronomical_trait
created_by: A.Amele

[Term]
id: CO_343:0000265
name: Pollination type estimation 1-4
namespace: YamTrait
def: "Visual assessment of the method or mode used to transfer the pollen grains from the anther of a flower to the stigma of a flower of the same or different plant of the same species using a 1-4 scale, where 1= Controlled cross pollination (transfer of pollen grains from the anther of a flower to the stigma of a flower of a different plant of the same species), 2= Self pollination (the transfer of pollen grains from the anther to the stigma of the same flower), 3= Bulk pollination (Pollen from the selected plant can be bulked to pollinate these some plants) and 4= Open pollination (Pollenation happen naturally from any plant )." []
synonym: "Pollmech" EXACT []
synonym: "Polltyp_E_1to4" EXACT []
is_a: CO_343:1000003 ! Variable
relationship: variable_of CO_343:0000264 ! pollination type
relationship: variable_of CO_343:0010044 ! pollination type-estimation
relationship: variable_of CO_343:0100023 ! 1-4 scale

[Term]
id: CO_343:0000266
name: Plant sex estimation 0-4
namespace: YamTrait
def: "Visual assesment of the most frequent (predominant) plant or flower sex type when more than 50% of the plants are flowered using a 0-4 scale, where 0= Non flowering, 1= Male flower, 2=female flower, 3= Monoecious male (m>f) and 4= Monoecious female(f>m)." []
synonym: "flrsex" EXACT []
synonym: "plntsex" EXACT []
synonym: "Sex_E_0to4" EXACT []
is_a: CO_343:1000003 ! Variable
relationship: variable_of CO_343:0000093 ! plant sex
relationship: variable_of CO_343:0010045 ! plant or flower sex-estimation
relationship: variable_of CO_343:0100024 ! 0-4 scale

[Term]
id: CO_343:0000267
name: Fruits developed per cross counting
namespace: YamTrait
def: "Computation of the number of developed fruits or fruit set in pollinated flowers/inflorescence as the quantity of developed fruits per crosses" []
synonym: "FrtN" EXACT []
synonym: "NFrts_Ct_frt per plot" EXACT []
is_a: CO_343:1000003 ! Variable
relationship: variable_of CO_343:0000006 ! fruit developed number
relationship: variable_of CO_343:0010046 ! fruits developed number - counting
relationship: variable_of CO_343:0100025 ! fruits/cross

[Term]
id: CO_343:0000268
name: time to fruit setting
namespace: YamTrait
def: "Times fruit formation or set on a monoeciuse or femal flowers of dioeciouse yam plants" []
synonym: "Datfrtset" EXACT []
is_a: CO_343:1000006 ! Phenological_trait
created_by: A.Amele

[Term]
id: CO_343:0000269
name: Fruit setting time estimation in yy/mm/dd
namespace: YamTrait
def: "Visual observation of the date(yyyymmdd) fruit set in 50% of plants in a plot as the time fruit formation or set on a monoeciuse or female flowers of dioeciouse yam plants" []
synonym: "DatFrtset_date_ymd" EXACT []
is_a: CO_343:1000003 ! Variable
relationship: variable_of CO_343:0000268 ! time to fruit setting
relationship: variable_of CO_343:0010047 ! 50% fruit set time-estimation
relationship: variable_of CO_343:0100002 ! date (yyyymmdd)

[Term]
id: CO_343:0000270
name: Fruit setting estimation 0&1
namespace: YamTrait
def: "Visual assessment of fruit setting or formation of female flowers of monoeciouse and dieciouse yam plants and rating the ability set for form fruits using a 0-1 scale, where 0= no fruit set, and 1= yes fruit set." []
synonym: "frtform" EXACT []
synonym: "Frtset_E_0to1" EXACT []
is_a: CO_343:1000003 ! Variable
relationship: variable_of CO_343:0000268 ! time to fruit setting
relationship: variable_of CO_343:0010048 ! ability to set or form fruts-estimation
relationship: variable_of CO_343:0100007 ! 0-1 scale

[Term]
id: CO_343:0000271
name: Fruits harvested per cross counting
namespace: YamTrait
def: "Computation of the number of harvested fruits per cross after physiological maturity." []
synonym: "Matfrt" EXACT []
synonym: "NfrtH_E" EXACT []
is_a: CO_343:1000003 ! Variable
relationship: variable_of CO_343:0000009 ! fruits harvested number
relationship: variable_of CO_343:0010049 ! fruits harvested number - counting
relationship: variable_of CO_343:0100026 ! number of fruits

[Term]
id: CO_343:0000272
name: time to fruit harvesting
namespace: YamTrait
def: "Time of fruit harvesting" []
synonym: "DateFH" EXACT []
is_a: CO_343:1000006 ! Phenological_trait
created_by: A.Amele

[Term]
id: CO_343:0000273
name: Fruit harvest time estimation in yy/mm/dd
namespace: YamTrait
def: "Visual observation and recording of the time or date(yyyymmdd) of fruits harvest in a crossing block or from plant." []
synonym: "DateFH_date_ymd" EXACT []
is_a: CO_343:1000003 ! Variable
relationship: variable_of CO_343:0000272 ! time to fruit harvesting
relationship: variable_of CO_343:0010050 ! fruit harvesting time- estimation
relationship: variable_of CO_343:0100002 ! date (yyyymmdd)

[Term]
id: CO_343:0000274
name: time to fruit maturity
namespace: YamTrait
def: "Times 90% of fruits attain physiological maturity" []
synonym: "TIMFrtM" EXACT []
is_a: CO_343:1000006 ! Phenological_trait
created_by: A.Amele

[Term]
id: CO_343:0000275
name: Fruit maturity time estimation in yy/mm/dd
namespace: YamTrait
def: "Visual observation and recording of the time or date (yyyymmdd) 90% of the developed fruits shows sign of physiological maturity (turning brown)" []
synonym: "DatFM_date_ymd" EXACT []
is_a: CO_343:1000003 ! Variable
relationship: variable_of CO_343:0000274 ! time to fruit maturity
relationship: variable_of CO_343:0010051 ! fruit maturity time - estimation
relationship: variable_of CO_343:0100002 ! date (yyyymmdd)

[Term]
id: CO_343:0000276
name: Times to fruit maturity computation in days
namespace: YamTrait
def: "Computation of the number of days required from fruit set to fruit phyisological maturity as the time 90% of fruits attain physiological maturity." []
synonym: "DFM" EXACT []
synonym: "TIMfrtm_dt_days" EXACT []
is_a: CO_343:1000003 ! Variable
relationship: variable_of CO_343:0000274 ! time to fruit maturity
relationship: variable_of CO_343:0010052 ! fruit maturity time - computation
relationship: variable_of CO_343:0100003 ! days

[Term]
id: CO_343:0000277
name: Fruit set number estimation 1-3
namespace: YamTrait
def: "Visual assessment of the intensity (proportion of fruit set or development under open or controlled pollination) in categorical scale when more than 50% of the plants set fruits using a 1-3 scale, where 1 = low, 2=medium and 3=high." []
synonym: "FRTINT" EXACT []
synonym: "Frtint_E_1to3" EXACT []
is_a: CO_343:1000003 ! Variable
relationship: variable_of CO_343:0000099 ! fruit set number
relationship: variable_of CO_343:0010053 ! fruit set number - estimation
relationship: variable_of CO_343:0100022 ! 1-3 scale

[Term]
id: CO_343:0000278
name: fruit set number percentage
namespace: YamTrait
def: "Computation of the intensity or proportion of pollinated flowers developing or setting a fruit under open or controlled pollination and expressed in %" []
synonym: "Pfrtset_Comp_pct" EXACT []
is_a: CO_343:1000003 ! Variable
relationship: variable_of CO_343:0000099 ! fruit set number
relationship: variable_of CO_343:0010054 ! fruit set number - computation
relationship: variable_of CO_343:0100006 ! %

[Term]
id: CO_343:0000279
name: status of fruit development
namespace: YamTrait
def: "Fruit development status on monoecious and female flower of dioeciouse yam plant" []
synonym: "FrtDev" EXACT []
is_a: CO_343:1000010 ! Morphological_trait
created_by: A.Amele

[Term]
id: CO_343:0000280
name: Fruit development status estimation 1-2
namespace: YamTrait
def: "Visual assessment and scoring of the degree of fruit development status on monoecious and female flower of dioeciouse yam plant using av1-2 scale, where 1= mostly well developed fruits, and 2= Poorly developed fruits." []
synonym: "FrtDev_E_1to2" EXACT []
is_a: CO_343:1000003 ! Variable
relationship: variable_of CO_343:0000279 ! status of fruit development
relationship: variable_of CO_343:0010055 ! fruit development intensity-estimation
relationship: variable_of CO_343:0100027 ! 1-2 scale

[Term]
id: CO_343:0000281
name: Seeds set/fruit computation
namespace: YamTrait
def: "The number of seeds set on each fruits after hand flowers pollination is counted and the average seeds per fruit computed." []
synonym: "SdSet_Comp_sdfrt" EXACT []
is_a: CO_343:1000003 ! Variable
relationship: variable_of CO_343:0000180 ! seeds set per fruit
relationship: variable_of CO_343:0010056 ! seeds set - comp
relationship: variable_of CO_343:0100028 ! number of seed

[Term]
id: CO_343:0000282
name: true seeds harvested
namespace: YamTrait
def: "Number of true seed harvested or obained per cross or family" []
synonym: "bontanical seed" EXACT []
synonym: "Botseed" EXACT []
synonym: "Tsdh" EXACT []
is_a: CO_343:1000008 ! Agronomical_trait
created_by: A.Amele

[Term]
id: CO_343:0000283
name: True seeds harvested/cross counting
namespace: YamTrait
def: "The total number of true (botanical) seed harvested or obtained per cross/family is recorded by counting." []
synonym: "Botseed" EXACT []
synonym: "Tsdh_Cou_TS" EXACT []
is_a: CO_343:1000003 ! Variable
relationship: variable_of CO_343:0000282 ! true seeds harvested
relationship: variable_of CO_343:0010057 ! quantity of true seed harvested -counting
relationship: variable_of CO_343:0100028 ! number of seed

[Term]
id: CO_343:0000284
name: fruit index
namespace: YamTrait
def: "Fruit index is an estimation of pollinated flowers developing physiologically mature fruits" []
is_a: CO_343:1000008 ! Agronomical_trait
created_by: A.Amele

[Term]
id: CO_343:0000285
name: Fruit index computation 0 to 1
namespace: YamTrait
def: "The ratio of number of fruit of pollinated florets developing physiologically mature fruits is computed as the fruit index." []
synonym: "Frtindx_Comp_idx" EXACT []
is_a: CO_343:1000003 ! Variable
relationship: variable_of CO_343:0000284 ! fruit index
relationship: variable_of CO_343:0010058 ! fruit index
relationship: variable_of CO_343:0100029 ! number of fruit

[Term]
id: CO_343:0000286
name: seed index
namespace: YamTrait
def: "Seed index is an estimation of pollinated flowers producing seeds" []
is_a: CO_343:1000008 ! Agronomical_trait
created_by: A.Amele

[Term]
id: CO_343:0000287
name: Seed index computation 0 to 1
namespace: YamTrait
def: "Computation of thee Seed index (which is an estimation of pollinated flowers producing seeds) as the ratio of pollinated florets developing seeds." []
synonym: "Seedindx_Comp_idx" EXACT []
is_a: CO_343:1000003 ! Variable
relationship: variable_of CO_343:0000286 ! seed index
relationship: variable_of CO_343:0010059 ! seed index
relationship: variable_of CO_343:0100028 ! number of seed

[Term]
id: CO_343:0000288
name: seeds sown
namespace: YamTrait
def: "Quantity of botanical or true seeds sown per family or cross" []
synonym: "Sdsown" EXACT []
is_a: CO_343:1000008 ! Agronomical_trait
created_by: A.Amele

[Term]
id: CO_343:0000289
name: Seeds sown/family counting
namespace: YamTrait
def: "The number of botanical or true seeds sown per cross or family is counted and recorded as its quantity." []
synonym: "Sdsown_Cou_Sd" EXACT []
is_a: CO_343:1000003 ! Variable
relationship: variable_of CO_343:0000288 ! seeds sown
relationship: variable_of CO_343:0010060 ! number of true seeds sown-counting
relationship: variable_of CO_343:0100028 ! number of seed

[Term]
id: CO_343:0000290
name: seeds germination start time
namespace: YamTrait
def: "Time the first seed germination occurred" []
synonym: "DAFGR" EXACT []
synonym: "Date sart of seed germination" EXACT []
synonym: "germstart" EXACT []
is_a: CO_343:1000006 ! Phenological_trait
created_by: A.Amele

[Term]
id: CO_343:0000291
name: Seeds germination start time estimation in yy/mm/dd
namespace: YamTrait
def: "Visual observation of time or date(yyyymmdd) the first seed germination per cross or family." []
synonym: "DAFGR" EXACT []
synonym: "germstart_date_ymd" EXACT []
is_a: CO_343:1000003 ! Variable
relationship: variable_of CO_343:0000290 ! seeds germination start time
relationship: variable_of CO_343:0010061 ! time of first seed germination-estimation
relationship: variable_of CO_343:0100002 ! date (yyyymmdd)

[Term]
id: CO_343:0000292
name: seeds germination end time
namespace: YamTrait
def: "Time last seed germination occurred" []
synonym: "DAEGR" EXACT []
synonym: "Date end of seed germination" EXACT []
synonym: "germend" EXACT []
is_a: CO_343:1000006 ! Phenological_trait
created_by: A.Amele

[Term]
id: CO_343:0000293
name: End of seeds germination time estiamtion in yy/mm/dd
namespace: YamTrait
def: "Visual observation of the time or date(yyyymmdd) the last seed germination per cross or family" []
synonym: "DAEGR" EXACT []
synonym: "germend_date_ymd" EXACT []
is_a: CO_343:1000003 ! Variable
relationship: variable_of CO_343:0000292 ! seeds germination end time
relationship: variable_of CO_343:0010062 ! date end of seed germination-estimation
relationship: variable_of CO_343:0100002 ! date (yyyymmdd)

[Term]
id: CO_343:0000294
name: Seed germination rate percentage
namespace: YamTrait
def: "Computation of the proportion in % of sown true or botanical seed which germinate and produce seedling ready for transplant , usually visual observation is carried out three weeks after sowing." []
synonym: "germrat_Comp_pct" EXACT []
synonym: "GR" EXACT []
is_a: CO_343:1000003 ! Variable
relationship: variable_of CO_343:0000012 ! seed germination rate
relationship: variable_of CO_343:0010063 ! germination rate - computation
relationship: variable_of CO_343:0100006 ! %

[Term]
id: CO_343:0000295
name: seeds germinated
namespace: YamTrait
def: "Quanity of sown true (botanical) seeds germinated per cross or family" []
synonym: "sdgerm" EXACT []
is_a: CO_343:1000008 ! Agronomical_trait
created_by: A.Amele

[Term]
id: CO_343:0000296
name: Seeds germinated counting
namespace: YamTrait
def: "The number (quantity) of sown true (botanical) seeds germinated per cross or family is recorded." []
synonym: "sdgerm_Cou_Sd" EXACT []
is_a: CO_343:1000003 ! Variable
relationship: variable_of CO_343:0000295 ! seeds germinated
relationship: variable_of CO_343:0010064 ! number of germinated seedling-counting
relationship: variable_of CO_343:0100028 ! number of seed

[Term]
id: CO_343:0000297
name: Seedling establishment rate percentage
namespace: YamTrait
def: "Computation of the proportion (establishment rate) of seedlings per family (cross) establish well and ready for transplanting, usually visual assessment is carried out five weeks after sowing." []
synonym: "sder" EXACT []
synonym: "sderat_Comp_pct" EXACT []
is_a: CO_343:1000003 ! Variable
relationship: variable_of CO_343:0000015 ! seedling establishment rate
relationship: variable_of CO_343:0010065 ! seedling establishment rate-computation
relationship: variable_of CO_343:0100006 ! %

[Term]
id: CO_343:0000298
name: seedling transplant survival rate
namespace: YamTrait
def: "Establishment rate of seedlings four weeks after transplanting operation" []
synonym: "Tsurvrat" EXACT []
is_a: CO_343:1000008 ! Agronomical_trait
created_by: A.Amele

[Term]
id: CO_343:0000299
name: Seedling survival rate percentage
namespace: YamTrait
def: "Computation of the proportion of seedlings survived or established rate of seedlings four weeks after transplant operation." []
synonym: "Sdsuvrat_Comp_pct" EXACT []
is_a: CO_343:1000003 ! Variable
relationship: variable_of CO_343:0000298 ! seedling transplant survival rate
relationship: variable_of CO_343:0010066 ! seedling tranplant survival rate-computation
relationship: variable_of CO_343:0100006 ! %

[Term]
id: CO_343:0000300
name: vine cuttings planted
namespace: YamTrait
def: "Vine cuttings planted" []
synonym: "NVP" EXACT []
is_a: CO_343:1000008 ! Agronomical_trait
created_by: A.Amele

[Term]
id: CO_343:0000301
name: Vine cuttings planted count
namespace: YamTrait
def: "The number vine cuttings planted by counting" []
synonym: "NVP_cout_number" EXACT []
is_a: CO_343:1000003 ! Variable
relationship: variable_of CO_343:0000300 ! vine cuttings planted
relationship: variable_of CO_343:0010067 ! vine cuttings planted -counting
relationship: variable_of CO_343:0100030 ! number of plant

[Term]
id: CO_343:0000302
name: vine cutting establishment rate
namespace: YamTrait
def: "Proportion of vine cuttings established well that producing shoots" []
synonym: "Vestrat" EXACT []
is_a: CO_343:1000008 ! Agronomical_trait
created_by: A.Amele

[Term]
id: CO_343:0000303
name: Vine cutting establishment rate percentage
namespace: YamTrait
def: "Computation of the proportion or ratio of vines cuttings that survived (established well) and producing shoots from the total of planted vine cuttings." []
synonym: "Vestrat_Comp_Pct" EXACT []
is_a: CO_343:1000003 ! Variable
relationship: variable_of CO_343:0000302 ! vine cutting establishment rate
relationship: variable_of CO_343:0010068 ! vines established-computation
relationship: variable_of CO_343:0100006 ! %

[Term]
id: CO_343:0000304
name: time to 50% foliage senescence
namespace: YamTrait
def: "Time when 50% of the plants in a plot are showing signs of foliage senescence" []
synonym: "DATS" EXACT []
synonym: "Datsen" EXACT []
synonym: "Partial senescence time" EXACT []
is_a: CO_343:1000006 ! Phenological_trait
created_by: A.Amele

[Term]
id: CO_343:0000305
name: Time to 50% foliage senescence estimation in yy/mm/dd
namespace: YamTrait
def: "Visual observation of time or date (yyyymmdd) when 50% plants in a plot are showing signs of foliage senescence." []
synonym: "DATS" EXACT []
synonym: "Datsen_date_ymd" EXACT []
is_a: CO_343:1000003 ! Variable
relationship: variable_of CO_343:0000304 ! time to 50% foliage senescence
relationship: variable_of CO_343:0010069 ! time to 50% foliage senescence time - estimation
relationship: variable_of CO_343:0100002 ! date (yyyymmdd)

[Term]
id: CO_343:0000307
name: Foliage senescence time estimation in yy/mm/dd
namespace: YamTrait
def: "Visual observation of the time or date (yyyymmdd) when all plants in a plot or unit area shows a sign of 100% (complete) foliage senescence." []
synonym: "DateHS" EXACT []
synonym: "Datfsen_date_ymd" EXACT []
is_a: CO_343:1000003 ! Variable
relationship: variable_of CO_343:0000111 ! foliage senescence time
relationship: variable_of CO_343:0010070 ! foliage senescence time - estimation
relationship: variable_of CO_343:0100002 ! date (yyyymmdd)

[Term]
id: CO_343:0000308
name: Time to 50% foliage senescence computation in days
namespace: YamTrait
def: "Computation of the number of days (time) required for 50% of the plants in a plot are showing signs of foliage senescence." []
synonym: "DM" EXACT []
synonym: "TIMsen_dt_day" EXACT []
is_a: CO_343:1000003 ! Variable
relationship: variable_of CO_343:0000304 ! time to 50% foliage senescence
relationship: variable_of CO_343:0010071 ! time to 50% foliage senescence time - computation
relationship: variable_of CO_343:0100003 ! days

[Term]
id: CO_343:0000309
name: Foliage senescence time computation in days
namespace: YamTrait
def: "Computation of the number of days (time) required from sprout emergence or planting to when all plants had fully senesced (complete foliage senescence) in a plot or unit area." []
synonym: "DAYHS" EXACT []
synonym: "TIMfsen_dt_day" EXACT []
is_a: CO_343:1000003 ! Variable
relationship: variable_of CO_343:0000111 ! foliage senescence time
relationship: variable_of CO_343:0010072 ! foliage senescence time - computation
relationship: variable_of CO_343:0100003 ! days

[Term]
id: CO_343:0000310
name: time to maturity
namespace: YamTrait
def: "Length of time toward crop maturity" []
synonym: "GDD" EXACT []
synonym: "Growing degree days" EXACT []
synonym: "Mat" EXACT []
is_a: CO_343:1000006 ! Phenological_trait
created_by: A.Amele

[Term]
id: CO_343:0000311
name: Maturity time estimation GGD
namespace: YamTrait
def: "Computation of the number of growing degree days required from planting (or 50% emergence) to 50% foliage senescence or maturity as the length of time toward crop maturity in GDD°C." []
synonym: "Mat _Comp_GGD" EXACT []
is_a: CO_343:1000003 ! Variable
relationship: variable_of CO_343:0000310 ! time to maturity
relationship: variable_of CO_343:0010073 ! growing degere days to maturity-estimation
relationship: variable_of CO_343:0100031 ! gdd°c

[Term]
id: CO_343:0000312
name: senescenece class
namespace: YamTrait
def: "Foliage senescence or maturity class" []
synonym: "MatC" EXACT []
synonym: "Maturity class" EXACT []
synonym: "SE" EXACT []
is_a: CO_343:1000009 ! Physiological_trait
created_by: A.Amele

[Term]
id: CO_343:0000313
name: Senescence class estimation 1-9
namespace: YamTrait
def: "Visual observation of the status of foliage senescence (leaf or vine yellowing) of plants in plot at 6 month onward and rating the maturity class (status) using a 1-9 scale, where 1= Very Late (all the plants in a plot still show green foliage (green leaf and vine), 3= Late (75% of the plants in a plot with still green foliage but few plants (upto 25% plants in a plot) showing up to 25% of leaves senescence, 5= Medium (50% of the plants are still green or on the onset of senescence. Only 50% plants in a plot with 25% of the leaves showing senescence or slight yellowing, 7= early (The plants have senescent foliage (75% of the plants in a plot with 50% leaves showing sign of yellowing but the vines still green), and 9= very early (The plants are completely senescent, yellowing is complete and uniform (both leaves and vines 100% senescence)." []
synonym: "MatC" EXACT []
synonym: "SE_E_1to9" EXACT []
is_a: CO_343:1000003 ! Variable
relationship: variable_of CO_343:0000312 ! senescenece class
relationship: variable_of CO_343:0010074 ! maturity class - estimation
relationship: variable_of CO_343:0100032 ! 1-9 scale

[Term]
id: CO_343:0000314
name: yam tuber dry rot presence
namespace: YamTrait
def: "Dry rot caused by nematodes (Scutellonema bradys and Practylenchus spp.) in tubers at harvest" []
synonym: "Dryrot" EXACT []
is_a: CO_343:1000005 ! Biotic_stress_trait
created_by: A.Amele

[Term]
id: CO_343:0000315
name: Presence of tuber dry rot estimation in 0&1
namespace: YamTrait
def: "Visual observation of the occurance or presence of dry rot caused by nematods (Scutellonema bradys and Practylenchus spp.) on harvested tubers and Visual assessment of the presence and absence using a 0-1 scale, where 0= Absent and 1=Present." []
synonym: "Dryrot_E_0to1" EXACT []
is_a: CO_343:1000003 ! Variable
relationship: variable_of CO_343:0000314 ! yam tuber dry rot presence
relationship: variable_of CO_343:0010075 ! dry rot presence on harvested tubers-estimation
relationship: variable_of CO_343:0100007 ! 0-1 scale

[Term]
id: CO_343:0000317
name: Number of dry rot tubers  count
namespace: YamTrait
def: "The number of dry rot caused by nematodes (Scutellonema bradys and Practylenchus spp.) in tubers per plot at harvest is done by counting." []
synonym: "Ndryrot_cou_tbr" EXACT []
is_a: CO_343:1000003 ! Variable
relationship: variable_of CO_343:0000042 ! yam tuber dry rot incidence
relationship: variable_of CO_343:0010076 ! dry rot tuber number-counting
relationship: variable_of CO_343:0100033 ! number

[Term]
id: CO_343:0000318
name: Tuber dry rot incidence computation in %
namespace: YamTrait
def: "Computation of the proportion in % of dry rot tubers caused by nematodes (Scutellonema bradys and Practylenchus spp.) from the total number of harvested tubers per effective plot." []
synonym: "Dryrotinc_Comp_pct" EXACT []
synonym: "S_Bri" EXACT []
is_a: CO_343:1000003 ! Variable
relationship: variable_of CO_343:0000042 ! yam tuber dry rot incidence
relationship: variable_of CO_343:0010077 ! tuber dry rot incidence - computation
relationship: variable_of CO_343:0100006 ! %

[Term]
id: CO_343:0000319
name: Tuber dry rot severity estimation 0-4
namespace: YamTrait
def: "Visual assessment and scoring of the severity of dry rot caused by nematodes (Scutellonema bradys and Practylenchus spp.) in harvested tubers using a 0-4 general scale, where 0= No symptoms, 1= 1-25% tuber skin showing symptoms, 2= 26-50% tuber skin showing symptoms, 3= 51-75% tuber skin showing symptoms, and 4= 76-100% tuber skin showing symptoms." []
synonym: "Dryrotsev_E_0to4" EXACT []
synonym: "S_Brs" EXACT []
is_a: CO_343:1000003 ! Variable
relationship: variable_of CO_343:0000045 ! yam tuber dry rot severity
relationship: variable_of CO_343:0010078 ! tuber dry rot severity - estimation
relationship: variable_of CO_343:0100034 ! 0-4 general scale

[Term]
id: CO_343:0000320
name: Leaf beetle damage incidence computation %
namespace: YamTrait
def: "Computation of the proportion (incidence) of plants in % with leaf beetle damage from the total number of plants in the effective plots and the record is taken twice(at two and five months after planting date)." []
synonym: "Btl_I" EXACT []
synonym: "Lfbtinc_Comp_pct" EXACT []
is_a: CO_343:1000003 ! Variable
relationship: variable_of CO_343:0000153 ! leaf beetle damage incidence
relationship: variable_of CO_343:0010079 ! leaf beetle incidence - computation
relationship: variable_of CO_343:0100006 ! %

[Term]
id: CO_343:0000321
name: Leaf beetle damage severity estimation in 1-5
namespace: YamTrait
def: "Visual assessment of the leaf beetle infestation at two and five months after planting and its severity of the damage using a 1-5 scale, where 1= No infestation, 2= Low (few perforated leaves), 3= Moderate (few perforated leaves in the upper and middle third of the plant), 4= High (several perforated leaves in the upper third of the plant), and 5= Very high (many perforated leaves in all the third of the plant)." []
synonym: "Btl_S" EXACT []
synonym: "Lfbtsev_E_1to5" EXACT []
is_a: CO_343:1000003 ! Variable
relationship: variable_of CO_343:0000156 ! leaf beetle damage severity
relationship: variable_of CO_343:0010080 ! leaf beetle severity - estimation
relationship: variable_of CO_343:0100008 ! 1-5 scale

[Term]
id: CO_343:0000322
name: Mealybug incidence computation %
namespace: YamTrait
def: "Computation of the proportion in % tubers infested with mealybugs from the total number of harvested tubers per effective plot at time of harvesting as the incidence of mealybug tuber infestation." []
synonym: "M_Bi" EXACT []
synonym: "MbugInc_Comp_pct" EXACT []
is_a: CO_343:1000003 ! Variable
relationship: variable_of CO_343:0000159 ! mealybug tuber infestation incidence
relationship: variable_of CO_343:0010081 ! mealybug tuber incidence - computation
relationship: variable_of CO_343:0100006 ! %

[Term]
id: CO_343:0000323
name: Mealybug severity estimation in 1-5
namespace: YamTrait
def: "Visual assessment of the mealybug tuber severity estimation on infested tubers at time harvesting using a 1-5 scale, where 1= No infestation, 2= Low (few nymph in one part of the tuber), 3= Moderate (few nymph in several parts of the tuber), 4= High (several nymph in many parts of the tuber), and 5= Very high (many nymph in all parts of the tuber)." []
synonym: "M_Bs" EXACT []
synonym: "MbugSev_E_1to5" EXACT []
is_a: CO_343:1000003 ! Variable
relationship: variable_of CO_343:0000162 ! mealybug tuber infestation severity
relationship: variable_of CO_343:0010082 ! mealybug tuber severity - estimation
relationship: variable_of CO_343:0100008 ! 1-5 scale

[Term]
id: CO_343:0000324
name: Root knot nematode incidence computation %
namespace: YamTrait
def: "Computation of the proportion (incidence) in % of tubers showing root knot nematode symptoms caused by Meloidogyne spp from the total number of harvested tubers in effective plot." []
synonym: "R_Kni" EXACT []
synonym: "RKNInc_Comp_pct" EXACT []
is_a: CO_343:1000003 ! Variable
relationship: variable_of CO_343:0000048 ! root knot nematode incidence
relationship: variable_of CO_343:0010083 ! root knot nematode incidence - computation
relationship: variable_of CO_343:0100006 ! %

[Term]
id: CO_343:0000325
name: Root knot nematode severity estimation in 1-5
namespace: YamTrait
def: "Root knot nematode severity estimation caused by Meloidogyne spp in a range from no symptoms to highly severe galling scored in secondary roots of the plant and tubers adventitious roots using a 1-5 scale, where 1= No symptoms, 2= Symptoms are slightly present, 3= Symptoms are moderated, 4= Symptoms are severe, and 5= Symptoms are very severe." []
synonym: "R_kns" EXACT []
synonym: "RKNSev_E_1to5" EXACT []
is_a: CO_343:1000003 ! Variable
relationship: variable_of CO_343:0000051 ! root knot nematode severity
relationship: variable_of CO_343:0010084 ! root knot nematode severity - estimation
relationship: variable_of CO_343:0100008 ! 1-5 scale

[Term]
id: CO_343:0000326
name: Tuber beetle incidence computation %
namespace: YamTrait
def: "Computation of the proportion (incidence) in % of tubers with tuber's beetle damage from the total number of harvested tubers in the effective plot at harvesting time." []
synonym: "Tbeti" EXACT []
synonym: "Tubtlinc_Comp_pct" EXACT []
is_a: CO_343:1000003 ! Variable
relationship: variable_of CO_343:0000165 ! tuber beetle incidence
relationship: variable_of CO_343:0010085 ! tuber beetle incidence - computation
relationship: variable_of CO_343:0100006 ! %

[Term]
id: CO_343:0000327
name: Tuber beetle severity estimation in 1-5
namespace: YamTrait
def: "Visual assessment of tuber beetle severity or intensity estimated usually as number of nymph present in tubers at harvesting time by using a 1-5 scale, where 1= No infestation, 2= Low (1 to 2 perforations in the tuber), 3= Severe (more than three perforations in the tuber), 4= High (several nymph in many parts of the tuber), and 5= Very high (many nymph in all parts of the tuber)." []
synonym: "Tbets" EXACT []
synonym: "Tubtlsev_E_1to5" EXACT []
is_a: CO_343:1000003 ! Variable
relationship: variable_of CO_343:0000168 ! tuber beetle severity
relationship: variable_of CO_343:0010086 ! tuber beetle severity - estimation
relationship: variable_of CO_343:0100008 ! 1-5 scale

[Term]
id: CO_343:0000328
name: Virus incidence computation %
namespace: YamTrait
def: "Computation of the proportion in % of virus symptomatic individuals or their parts or commonly the portion of plant units in a plot by taking the virus incidence record thrice, where First inspection at 8 to 10 weeks after planting and second inspection after 4 to 6 weeks after first inspection for virus symptoms and the third and final inspection 4 to 6 weeks after the second inspection; as the reaction of the total plants per plot to the virus infection, producing yellow mottle, mosaic and leaves deformation." []
synonym: "VirusInc_comp_pct" EXACT []
synonym: "VRSI" EXACT []
is_a: CO_343:1000003 ! Variable
relationship: variable_of CO_343:0000081 ! virus incidence
relationship: variable_of CO_343:0010087 ! viruses infection incidence - computation
relationship: variable_of CO_343:0100006 ! %

[Term]
id: CO_343:0000329
name: virus severity estimation in 1-5
namespace: YamTrait
def: "Visual assessment of the grade of reaction of the plant to the viruses infection, varying from mottle, mosaics until total leaves deformation by observing the relative or absolute area of plant tissue affected by virus disease and recording of the severity as a proportion or percentage of plant surface affected using visual five ordinal scale (1-5 scale), where 1= no visible symptoms, 2=mosaic on few leaves, symptom recovery over time, 3=mild symptoms on many leaves but no leaf distortion, 4= severe mosaic on most leaves, leaf distortion, and 5 = severe mosaic (bleaching), severe leaf distortion and stunting." []
synonym: "VirusSev_E_1to5" EXACT []
synonym: "VRSS" EXACT []
is_a: CO_343:1000003 ! Variable
relationship: variable_of CO_343:0000084 ! virus severity
relationship: variable_of CO_343:0010088 ! viruses infection severity - estimation
relationship: variable_of CO_343:0100008 ! 1-5 scale

[Term]
id: CO_343:0000330
name: yam anthracnose disease incidence computation %
namespace: YamTrait
def: "Computation of the proportion (incidence) in % of anthracnose damaged individuals or their parts caused by the pathogen Colletotricum gloeosporioides ; commonly the portion of plant units in a plot by counting the anthracnose disease ‘blight’ or '' leaf spot'' affected plants in plot twice (First inspection at 10 to 12 weeks post planting and second inspection after 2 to 4 weeks before harvesting ) and the proportion of damaged is also computed." []
synonym: "AnthracInc" EXACT []
synonym: "YADI_E_pct" EXACT []
is_a: CO_343:1000003 ! Variable
relationship: variable_of CO_343:0000075 ! yam anthracnose disease incidence
relationship: variable_of CO_343:0010089 ! anthracnose incidence - estimation
relationship: variable_of CO_343:0100006 ! %

[Term]
id: CO_343:0000331
name: yam anthracnose disease severity estimation in 1-5
namespace: YamTrait
def: "Visual assessment of anthracnose severity caused by the pathogen Colletotricum gloeosporioides by observing the relative or absolute area of plant tissue affected by yam anthracnose disease and recording of the severity as a proportion or percentage of plant surface affected using a visual 1-5 general scale, where 1= No visible symptoms of anthracnose disease or infection spot on the leaf surface, 2= Few anthracnose spots or sysmptoms on 1 t0 ~25% of the plant (i.e. one or two spots of less than 1 cm diameter width, and dry tissue on the leaf surface), 3= Anthracnose symptoms covering ~26 t0 ~50% of the plant (i.e. one or two spots of more than 1 cm diameter width, and dry tissue on the leaf surface. Small dark and no dried spots with more than 1 cm width, are present), 4= Symptom on >51% of the plant (i.e. coalesced spots with dry tissue and covering a signifcant proprotion of the leaf surface. Areas with less than 1 cm width are coalescing to bigger spots also. Yellowing of green tissue is intense around the spots areas), and 5=Severe necrosis and death of the plant(i.e. Coalesced spots with dry tissue more than 1.5 cm of diameter and covering a great proprotion of the leaf surface andellowing of the gree tissue is generalised in the leaf blade)" []
synonym: "AnthracSev" EXACT []
synonym: "YADS_E_1to5" EXACT []
is_a: CO_343:1000003 ! Variable
relationship: variable_of CO_343:0000021 ! yam anthracnose disease severity
relationship: variable_of CO_343:0010090 ! anthracnose severity - estimation
relationship: variable_of CO_343:0100035 ! 1-5 general scale

[Term]
id: CO_343:0000332
name: Bulbils per plot count
namespace: YamTrait
def: "The number of vine bulbils or aerial tubers produced per net plot by counting" []
synonym: "Aetbrp" EXACT []
synonym: "Bulbp_Ct_NPlot" EXACT []
is_a: CO_343:1000003 ! Variable
relationship: variable_of CO_343:0000117 ! number of bulbil
relationship: variable_of CO_343:0010091 ! number of bulbil - counting
relationship: variable_of CO_343:0100036 ! number of bulbils

[Term]
id: CO_343:0000334
name: Bulbils per plant computation
namespace: YamTrait
def: "The number of vine bulbils or aerial tubers on plants in a net plot by counting and the computation of the average number of bulbils per plant" []
synonym: "Aetbrpl" EXACT []
synonym: "Bulbpl_Comp_NPlant" EXACT []
is_a: CO_343:1000003 ! Variable
relationship: variable_of CO_343:0000117 ! number of bulbil
relationship: variable_of CO_343:0010092 ! number of bulbil - computation
relationship: variable_of CO_343:0100037 ! bulbil/plant

[Term]
id: CO_343:0000335
name: bulbil shape
namespace: YamTrait
def: "Predominant shape of the bulbils" []
synonym: "Aerial tuber shape" EXACT []
synonym: "Aetbrshap" EXACT []
synonym: "Bulbsp" EXACT []
is_a: CO_343:1000010 ! Morphological_trait
created_by: A.Amele

[Term]
id: CO_343:0000336
name: Shape of bulbil estimation 1-4
namespace: YamTrait
def: "The predominant shape of bulbils or aerial tubers recorded using a 1-4 scale where 1= round, 2= oval, 3=irregular (not uniform) and 4= elongate" []
synonym: "Aetbrshap" EXACT []
synonym: "Bulbsp_E_1to4" EXACT []
is_a: CO_343:1000003 ! Variable
relationship: variable_of CO_343:0000335 ! bulbil shape
relationship: variable_of CO_343:0010093 ! bulbil shape-estimation
relationship: variable_of CO_343:0100016 ! 1-4 general scale

[Term]
id: CO_343:0000337
name: bulbil weight
namespace: YamTrait
def: "Weight of vine bulbils or aerial tubers harvest" []
synonym: "Aerial tuber weight" EXACT []
synonym: "Aetubwtp" EXACT []
synonym: "Bulbwtp" EXACT []
is_a: CO_343:1000008 ! Agronomical_trait
created_by: A.Amele

[Term]
id: CO_343:0000338
name: Bulbil weight per plot measurement in kg
namespace: YamTrait
def: "The fresh weight of harvested bulbil or aerial tuber per net plot recorded in kg" []
synonym: "Aetubwtp" EXACT []
synonym: "BulbwtP_M_kgPlot" EXACT []
is_a: CO_343:1000003 ! Variable
relationship: variable_of CO_343:0000337 ! bulbil weight
relationship: variable_of CO_343:0010094 ! bulbil yield (plot weight) - measurement
relationship: variable_of CO_343:0100038 ! kg

[Term]
id: CO_343:0000340
name: Bulbil yield per plant measurement in kg
namespace: YamTrait
def: "The yield weight of harvested vine bulbils or aerial tubers per plant is computed in kg" []
synonym: "AetbrwtPl" EXACT []
synonym: "Bulbwtpl_Comp_kgplnt" EXACT []
is_a: CO_343:1000003 ! Variable
relationship: variable_of CO_343:0000120 ! bulbil yield
relationship: variable_of CO_343:0010095 ! bulbil yield (fresh weight) per plant-computation
relationship: variable_of CO_343:0100039 ! kg/plant

[Term]
id: CO_343:0000341
name: Bulbil yield estimation in t/ha
namespace: YamTrait
def: "The yield of vine bulbils or aerial tubers per hectare using the formula and computed in tons/ha" []
synonym: "AetbrYld" EXACT []
synonym: "Bulbyld_FW_tha" EXACT []
is_a: CO_343:1000003 ! Variable
relationship: variable_of CO_343:0000120 ! bulbil yield
relationship: variable_of CO_343:0010096 ! bulbil yield (fresh weight) per hectar- computation
relationship: variable_of CO_343:0100040 ! tons/ha

[Term]
id: CO_343:0000342
name: Bulbil initiation time estimation in yy/mm/dd
namespace: YamTrait
def: "The date (yyyymmdd) and initiation time of bulbils or aerial tubers is recorded when 50%of the plant in a plot begins to produce." []
synonym: "Aetbrin" EXACT []
synonym: "Datblbin_date_ymd" EXACT []
is_a: CO_343:1000003 ! Variable
relationship: variable_of CO_343:0000108 ! time to bulbil initiation
relationship: variable_of CO_343:0010097 ! bulbil initiaition time - estimation
relationship: variable_of CO_343:0100002 ! date (yyyymmdd)

[Term]
id: CO_343:0000344
name: Times to bulbil initiation computation
namespace: YamTrait
def: "Computation of initiation time and the number of days required from sprout emergence to 50% of plants in a plot start forming bulbils or aerial tubers" []
synonym: "Dayaetbrin" EXACT []
synonym: "TIMbulb_dt_day" EXACT []
is_a: CO_343:1000003 ! Variable
relationship: variable_of CO_343:0000108 ! time to bulbil initiation
relationship: variable_of CO_343:0010098 ! bulbil initiation time - computation
relationship: variable_of CO_343:0100003 ! days

[Term]
id: CO_343:0000345
name: Bulbil presence estimation 0&1
namespace: YamTrait
def: "The presence and absence of bulbils or aerial tubers in the nodes of the vines of yam plant is recorded using a 0-1 scale where 0= Absent and 1= Present" []
synonym: "AeTuber" EXACT []
synonym: "Bulbil_E_0to1" EXACT []
is_a: CO_343:1000003 ! Variable
relationship: variable_of CO_343:0000105 ! presence of bulbil
relationship: variable_of CO_343:0010099 ! presence of bulbil  - estimation
relationship: variable_of CO_343:0100007 ! 0-1 scale

[Term]
id: CO_343:0000346
name: Plant stand harvested count
namespace: YamTrait
def: "The number of plants where tubers were harvested in a plot is counted" []
synonym: "No_stdh" EXACT []
synonym: "NPH_Cou_standPlot" EXACT []
is_a: CO_343:1000003 ! Variable
relationship: variable_of CO_343:0000123 ! stand harvested number
relationship: variable_of CO_343:0010100 ! plant harvested number - counting
relationship: variable_of CO_343:0100041 ! plant per plot

[Term]
id: CO_343:0000347
name: big size tubers per plot
namespace: YamTrait
def: "Number of big size tubers that weighing ≥1 kg in a net plot or unit area" []
synonym: "NBTP" EXACT []
synonym: "NTSzAp" EXACT []
synonym: "Tubers per plot size 1" EXACT []
is_a: CO_343:1000008 ! Agronomical_trait
created_by: A.Amele

[Term]
id: CO_343:0000348
name: Big tubers per plot counting number
namespace: YamTrait
def: "The number of big size tubers harvested in a net plot or unit area weighing ≥1kg is counted" []
synonym: "NBTP_cou_number/plot" EXACT []
is_a: CO_343:1000003 ! Variable
relationship: variable_of CO_343:0000347 ! big size tubers per plot
relationship: variable_of CO_343:0010101 ! big size tubers harvested number - counting
relationship: variable_of CO_343:0100042 ! tuber number/plot

[Term]
id: CO_343:0000349
name: medium size tubers per plot
namespace: YamTrait
def: "Number  of medium size tubers that weighing ≥ 0.5kg and <1 kg in a net plot or unit area" []
synonym: "NMTP" EXACT []
synonym: "NTSzBp" EXACT []
synonym: "Tubers per plot size 2" EXACT []
is_a: CO_343:1000008 ! Agronomical_trait
created_by: A.Amele

[Term]
id: CO_343:0000350
name: Medium tubers per plot counting number
namespace: YamTrait
def: "The number of medium size tubers harvested in a net plot or unit area weighing ≥0.5kg (500gm) and <1 kg is counted" []
synonym: "NMTP_cou_number/plot" EXACT []
is_a: CO_343:1000003 ! Variable
relationship: variable_of CO_343:0000349 ! medium size tubers per plot
relationship: variable_of CO_343:0010102 ! medium size tubers harvested number- counting
relationship: variable_of CO_343:0100042 ! tuber number/plot

[Term]
id: CO_343:0000351
name: small size tubers per plot
namespace: YamTrait
def: "Number of small size tubers that weighing <0.5kg in a net plot or unit area" []
synonym: "NSTP" EXACT []
synonym: "NTSzCp" EXACT []
synonym: "Tubers per plot size 3" EXACT []
is_a: CO_343:1000008 ! Agronomical_trait
created_by: A.Amele

[Term]
id: CO_343:0000352
name: Small tubers per plot counting number
namespace: YamTrait
def: "The number of small size tubers harvested in a net plot or unit area weighing ≥0.5kg (500gm) and <1 kg is counted" []
synonym: "NSTP_cou_number/plot" EXACT []
is_a: CO_343:1000003 ! Variable
relationship: variable_of CO_343:0000351 ! small size tubers per plot
relationship: variable_of CO_343:0010103 ! small size tubers harvested per plot number - counting
relationship: variable_of CO_343:0100042 ! tuber number/plot

[Term]
id: CO_343:0000353
name: Rotten tubers per plot counting number
namespace: YamTrait
def: "The number of rotten yam tubers and/or diseased tubers in a net plot or unit area is counted." []
synonym: "NRD_E_tbrsplot" EXACT []
synonym: "NRDT" EXACT []
is_a: CO_343:1000003 ! Variable
relationship: variable_of CO_343:0000138 ! rotten or diseased tubers per plot
relationship: variable_of CO_343:0010104 ! rotten tubers in a plot number-counting
relationship: variable_of CO_343:0100042 ! tuber number/plot

[Term]
id: CO_343:0000354
name: Total tubers per plot computation
namespace: YamTrait
def: "The total sum of all category/size tubers is computed (big, medium, small and rotten/diseased) in a net plot or unit area" []
synonym: "TNTP_Comp_TbrsPlot" EXACT []
is_a: CO_343:1000003 ! Variable
relationship: variable_of CO_343:0000126 ! total tubers per plot
relationship: variable_of CO_343:0010105 ! total tuber harvested number-computation
relationship: variable_of CO_343:0100042 ! tuber number/plot

[Term]
id: CO_343:0000355
name: big size tubers per plant
namespace: YamTrait
def: "Number of big size tubers ( ≥1 kg) per plant" []
synonym: "NBTPL" EXACT []
synonym: "NTSzBpl" EXACT []
is_a: CO_343:1000008 ! Agronomical_trait
created_by: A.Amele

[Term]
id: CO_343:0000356
name: Big tubers  per plant computation
namespace: YamTrait
def: "The number of big size tubers (≥1kg)produced per plant is computed using the formula number of big size tuber in a plot divided by the total number of harvested plants" []
synonym: "NBTPL_Comp_tbrplt" EXACT []
is_a: CO_343:1000003 ! Variable
relationship: variable_of CO_343:0000355 ! big size tubers per plant
relationship: variable_of CO_343:0010106 ! big size tubers per plant-computation
relationship: variable_of CO_343:0100043 ! tuber number/plant

[Term]
id: CO_343:0000357
name: medium size tubers per plant
namespace: YamTrait
def: "Number of medium size tubers (≥ 0.5kg and <1 kg) per plant" []
synonym: "NMTPL" EXACT []
synonym: "NTSzNpl" EXACT []
is_a: CO_343:1000008 ! Agronomical_trait
created_by: A.Amele

[Term]
id: CO_343:0000358
name: Medium tubers per plant computation
namespace: YamTrait
def: "The number of medium size tubers (≥ 0.5kg and<1kg)produced per plant is computed using the formula number of big size tuber in a plot divided by the total number of harvested plants" []
synonym: "NMTPL_Comp_tbrplt" EXACT []
is_a: CO_343:1000003 ! Variable
relationship: variable_of CO_343:0000357 ! medium size tubers per plant
relationship: variable_of CO_343:0010107 ! medium size tubers per plant-computation
relationship: variable_of CO_343:0100043 ! tuber number/plant

[Term]
id: CO_343:0000359
name: small size tubers per plant
namespace: YamTrait
def: "Number of small size tubers ( <0.5kg) per plant" []
synonym: "NSTPL" EXACT []
synonym: "NTSzSpl" EXACT []
is_a: CO_343:1000008 ! Agronomical_trait
created_by: A.Amele

[Term]
id: CO_343:0000360
name: Small tubers per plant compuatation
namespace: YamTrait
def: "The number of small size tubers ( <0.5kg) produced per plant is computed using the formula number of big size tuber in a plot divided by the total number of harvested plants" []
synonym: "NSTPL_Comp_tbrsplt" EXACT []
is_a: CO_343:1000003 ! Variable
relationship: variable_of CO_343:0000359 ! small size tubers per plant
relationship: variable_of CO_343:0010108 ! small size tubers per plant-computation
relationship: variable_of CO_343:0100043 ! tuber number/plant

[Term]
id: CO_343:0000361
name: total tubers per plant
namespace: YamTrait
def: "Number of tubers harvested per plant" []
synonym: "TNTPL" EXACT []
is_a: CO_343:1000008 ! Agronomical_trait
created_by: A.Amele

[Term]
id: CO_343:0000362
name: Total tubers per plant computation
namespace: YamTrait
def: "The total number of harvested tubers per plant in a net plot is computed by dividing the number of harvested plant per net plot" []
synonym: "TNTPL_Comp_tbrplt" EXACT []
is_a: CO_343:1000003 ! Variable
relationship: variable_of CO_343:0000361 ! total tubers per plant
relationship: variable_of CO_343:0010109 ! total tubers per plant-computation
relationship: variable_of CO_343:0100043 ! tuber number/plant

[Term]
id: CO_343:0000363
name: big size tubers weight per plot
namespace: YamTrait
def: "Weight of big size tubers ( ≥1 kg) in a net plot or unit area" []
synonym: "BSzTW" EXACT []
synonym: "BTW" EXACT []
is_a: CO_343:1000008 ! Agronomical_trait
created_by: A.Amele

[Term]
id: CO_343:0000364
name: Weight of big tubers per plot measurement in kg
namespace: YamTrait
def: "The weight of big size tubers ( ≥1 kg) in a net plot or unit area is recorded in kg/plot" []
synonym: "Btbrwt" EXACT []
synonym: "BTW_FW_kgplot" EXACT []
is_a: CO_343:1000003 ! Variable
relationship: variable_of CO_343:0000363 ! big size tubers weight per plot
relationship: variable_of CO_343:0010110 ! big size tubers fresh weight per plot- measurement
relationship: variable_of CO_343:0100044 ! kg/plot

[Term]
id: CO_343:0000365
name: medium size tubers weight per plot
namespace: YamTrait
def: "Weight of medium size tubers (≥ 0.5kg and <1 kg) in a net plot or unit area" []
synonym: "MSzTW" EXACT []
synonym: "MTW" EXACT []
is_a: CO_343:1000008 ! Agronomical_trait
created_by: A.Amele

[Term]
id: CO_343:0000366
name: Weight medium tubers per plot  measurement in kg
namespace: YamTrait
def: "The weight of medium size tubers ( ≥ 0.5kg and <1 kg) in a net plot or unit area is recorded in kg/plot" []
synonym: "Mtbrwt" EXACT []
synonym: "MTW_FW_kgplot" EXACT []
is_a: CO_343:1000003 ! Variable
relationship: variable_of CO_343:0000365 ! medium size tubers weight per plot
relationship: variable_of CO_343:0010111 ! medium size tubers fresh weight per plot -measurement
relationship: variable_of CO_343:0100044 ! kg/plot

[Term]
id: CO_343:0000367
name: small size tubers weight per plot
namespace: YamTrait
def: "Weight of small size tubers ( <0.5kg ) in a net plot or unit area" []
synonym: "SSzTW" EXACT []
synonym: "STW" EXACT []
is_a: CO_343:1000008 ! Agronomical_trait
created_by: A.Amele

[Term]
id: CO_343:0000368
name: Weight of small tubers per plot measurement in kg
namespace: YamTrait
def: "The weight (in kg/plot)of small size tubers ( <0.5kg) in a net plot or unit area is recorded." []
synonym: "Stbrwt" EXACT []
synonym: "STW_FW_kgplot" EXACT []
is_a: CO_343:1000003 ! Variable
relationship: variable_of CO_343:0000367 ! small size tubers weight per plot
relationship: variable_of CO_343:0010112 ! small size tubers fresh weight per plot- measurement
relationship: variable_of CO_343:0100044 ! kg/plot

[Term]
id: CO_343:0000369
name: Weight of rotten/diseased tubers per plot measurement in kg
namespace: YamTrait
def: "The weight of rotten and/or diseased tubers harvested in a net plot is recorded in kg/plot" []
synonym: "RDTW_FW_kgPlot" EXACT []
synonym: "Rot_Wt" EXACT []
is_a: CO_343:1000003 ! Variable
relationship: variable_of CO_343:0000138 ! rotten or diseased tubers per plot
relationship: variable_of CO_343:0010113 ! rotten tuber fresh weight per plot - measurement
relationship: variable_of CO_343:0100044 ! kg/plot

[Term]
id: CO_343:0000370
name: total fresh tuber weight per plot
namespace: YamTrait
def: "Total fresh weight of all category or size tubers harvested in a net plot" []
synonym: "TTWP" EXACT []
is_a: CO_343:1000008 ! Agronomical_trait
created_by: A.Amele

[Term]
id: CO_343:0000371
name: Total tuber weight per plot computation in kg
namespace: YamTrait
def: "Computation of the sum of total fresh weight (in kg/plot) of all category or size of tubers (Big, medium, small size, and rotten and diseased) harvested in a net plot" []
synonym: "TTWP_FW_kgplot" EXACT []
is_a: CO_343:1000003 ! Variable
relationship: variable_of CO_343:0000370 ! total fresh tuber weight per plot
relationship: variable_of CO_343:0010114 ! total tuber fresh weight per plot -computation
relationship: variable_of CO_343:0100044 ! kg/plot

[Term]
id: CO_343:0000372
name: total tuber weight per plant
namespace: YamTrait
def: "Total fresh weight of all category or size tubers per plant" []
synonym: "TTWPL" EXACT []
is_a: CO_343:1000008 ! Agronomical_trait
created_by: A.Amele

[Term]
id: CO_343:0000373
name: Total tuber weight per plant computation in kg
namespace: YamTrait
def: "Computation of the total fresh weight (in kg/plant) of all category or size of tubers per plant by dividing fresh weight measurement taken in a plot to the number of harvested plant in a net plot" []
synonym: "TTWPL_FW_kgplt" EXACT []
is_a: CO_343:1000003 ! Variable
relationship: variable_of CO_343:0000372 ! total tuber weight per plant
relationship: variable_of CO_343:0010115 ! total tuber fresh weight per plant-computation
relationship: variable_of CO_343:0100039 ! kg/plant

[Term]
id: CO_343:0000374
name: big size tuber weight per plant
namespace: YamTrait
def: "Weight of big size tubers per plant" []
synonym: "WBTPL" EXACT []
is_a: CO_343:1000008 ! Agronomical_trait
created_by: A.Amele

[Term]
id: CO_343:0000375
name: Weight of big tubers per plant measurement in kg
namespace: YamTrait
def: "Computation of weight (in kg/plant ) of big size tubers per plant by dividing fresh weight measurement taken to the number of harvested plants in a net plot" []
synonym: "MTWPL" EXACT []
synonym: "WBTPL_FW_kg" EXACT []
is_a: CO_343:1000003 ! Variable
relationship: variable_of CO_343:0000374 ! big size tuber weight per plant
relationship: variable_of CO_343:0010116 ! big size yam fresh weight per plant- computation
relationship: variable_of CO_343:0100039 ! kg/plant

[Term]
id: CO_343:0000376
name: medium size tuber weight per plant
namespace: YamTrait
def: "Weight of medium size tuber yam per plant" []
synonym: "WMTPL" EXACT []
is_a: CO_343:1000008 ! Agronomical_trait
created_by: A.Amele

[Term]
id: CO_343:0000377
name: Weight of medium tubers per plant computation kgplt
namespace: YamTrait
def: "Computation of weight (in kg/plant) of medium size tuber yam per plant by dividing fresh weight measurement taken to the number of harvested plants in a net plot" []
synonym: "WMTPL_FW_kg" EXACT []
is_a: CO_343:1000003 ! Variable
relationship: variable_of CO_343:0000376 ! medium size tuber weight per plant
relationship: variable_of CO_343:0010117 ! medium size yam fresh weight per plant-computation
relationship: variable_of CO_343:0100039 ! kg/plant

[Term]
id: CO_343:0000378
name: small size tuber weight per plant
namespace: YamTrait
def: "Weight of small size yam per plant" []
synonym: "WSTPL" EXACT []
is_a: CO_343:1000008 ! Agronomical_trait
created_by: A.Amele

[Term]
id: CO_343:0000379
name: Weight of small tuber per plant computation kgplant
namespace: YamTrait
def: "Computation of the weight (in kg/plant) of small size yam per plant by dividing fresh weight measurement taken to the number of harvested plants in a net plot" []
synonym: "WSTPL_FW_kg" EXACT []
is_a: CO_343:1000003 ! Variable
relationship: variable_of CO_343:0000378 ! small size tuber weight per plant
relationship: variable_of CO_343:0010118 ! small size yam fresh weight per plant-computation
relationship: variable_of CO_343:0100039 ! kg/plant

[Term]
id: CO_343:0000380
name: Total tuber yield computation in t/ha
namespace: YamTrait
def: "Total tuber yield nonadjusted in tons/ hectare is computed as total tuber weight per plot divided by the size of net (effective) harvest plot and result multiplied by 10." []
synonym: "TTYNA_FW_tonha" EXACT []
synonym: "TubYld" EXACT []
is_a: CO_343:1000003 ! Variable
relationship: variable_of CO_343:0000132 ! total tuber yield
relationship: variable_of CO_343:0010119 ! tuber yield no adjusted- computation
relationship: variable_of CO_343:0100040 ! tons/ha

[Term]
id: CO_343:0000381
name: Big tuber yield computation in t/ha
namespace: YamTrait
def: "Big size tubers yield nonadjusted in tons/hectare is calculated as big size yam tuber weight per plot divided by size of effective harvest plot mutiplied by 10." []
synonym: "BTYNA_FW_tonha" EXACT []
is_a: CO_343:1000003 ! Variable
relationship: variable_of CO_343:0000135 ! big size yam yield
relationship: variable_of CO_343:0010120 ! big size yam yield no adjusted- computation
relationship: variable_of CO_343:0100040 ! tons/ha

[Term]
id: CO_343:0000382
name: total tuber yield adjusted
namespace: YamTrait
def: "Total tuber yield adjusted tons per hectare" []
synonym: "TTYA" EXACT []
is_a: CO_343:1000008 ! Agronomical_trait
created_by: A.Amele

[Term]
id: CO_343:0000383
name: Tuber yield adjusted computation in t/ha
namespace: YamTrait
def: "Total tuber yield adjusted in tons/hectare is computed as the total tubers weight per plant multiplied by planting density and result divided by 1000" []
synonym: "TTYA_Adj_tonha" EXACT []
is_a: CO_343:1000003 ! Variable
relationship: variable_of CO_343:0000382 ! total tuber yield adjusted
relationship: variable_of CO_343:0010121 ! total tuber yield adjusted-computation
relationship: variable_of CO_343:0100040 ! tons/ha

[Term]
id: CO_343:0000384
name: big size tuber yield adjusted
namespace: YamTrait
def: "Big size tubers yield adjusted tons per hectare" []
synonym: "BTYA" EXACT []
is_a: CO_343:1000008 ! Agronomical_trait
created_by: A.Amele

[Term]
id: CO_343:0000385
name: Big tuber yield adjusted computation in t/ha
namespace: YamTrait
def: "Big size tubers yield adjusted in tons/hectare is calculated as big size yam tuber weight per per plant mutiplied by planting density and result divided by 1000" []
synonym: "BTYA-Adj_tonha" EXACT []
is_a: CO_343:1000003 ! Variable
relationship: variable_of CO_343:0000384 ! big size tuber yield adjusted
relationship: variable_of CO_343:0010122 ! big size yam yield adjusted-computation
relationship: variable_of CO_343:0100040 ! tons/ha

[Term]
id: CO_343:0000386
name: average weigth of big size tuber
namespace: YamTrait
def: "Average weight of big size tubers in kg" []
synonym: "AWBT" EXACT []
is_a: CO_343:1000008 ! Agronomical_trait
created_by: A.Amele

[Term]
id: CO_343:0000387
name: Big tuber average weight computation in kg
namespace: YamTrait
def: "Average weight of big size tubers in kg is calculated as weight of big size tubers per plot divided by total number of big size tubers per plot" []
synonym: "AWBT_comp_gm" EXACT []
is_a: CO_343:1000003 ! Variable
relationship: variable_of CO_343:0000386 ! average weigth of big size tuber
relationship: variable_of CO_343:0010123 ! big yam tuber average weight-computation
relationship: variable_of CO_343:0100038 ! kg

[Term]
id: CO_343:0000388
name: average tuber weight
namespace: YamTrait
def: "Average tuber weight in kg" []
synonym: "ATW" EXACT []
is_a: CO_343:1000008 ! Agronomical_trait
created_by: A.Amele

[Term]
id: CO_343:0000389
name: Average tuber weight computation in kg
namespace: YamTrait
def: "Average tuber weight in kg is calculated as total tuber weight per plot divided by total number of tubers per plot" []
synonym: "ATW_comp_gm" EXACT []
is_a: CO_343:1000003 ! Variable
relationship: variable_of CO_343:0000388 ! average tuber weight
relationship: variable_of CO_343:0010124 ! average tuber weight -computation
relationship: variable_of CO_343:0100038 ! kg

[Term]
id: CO_343:0000390
name: place of roots on tubers
namespace: YamTrait
def: "Position of appearance of roots at surface of tubers" []
synonym: "Prtbs" EXACT []
is_a: CO_343:1000010 ! Morphological_trait
created_by: A.Amele

[Term]
id: CO_343:0000391
name: Root position estimation 1-4
namespace: YamTrait
def: "The visual assessment and recording of the position (in terms of its appearance) of roots at surface tubers using a 1-4 scale where 1= lower portion, 2=Middle portion, 3=Upper portion and 4= Entire tuber" []
synonym: "Prtbrs_E_1to4" EXACT []
is_a: CO_343:1000003 ! Variable
relationship: variable_of CO_343:0000390 ! place of roots on tubers
relationship: variable_of CO_343:0010125 ! position of root appearance on tubers-estimation
relationship: variable_of CO_343:0100023 ! 1-4 scale

[Term]
id: CO_343:0000392
name: Hairiness of tuber estimation 1-3
namespace: YamTrait
def: "The presence/intensity of tuber hair or secondary roots on the surface of harvested tubers is recorded using a 1-3 scale where 1= No roots, 2= Few (few scattered roots in the surface at the proximal section of the tuber) and 3= Many roots on the entire surface of the tuber or many roots in one of the section of the tuber)" []
synonym: "Htbrs_E_1to3" EXACT []
synonym: "TBR_Hairy" EXACT []
is_a: CO_343:1000003 ! Variable
relationship: variable_of CO_343:0000183 ! tuber hairiness
relationship: variable_of CO_343:0010126 ! hairiness of tuber bark - estimation
relationship: variable_of CO_343:0100022 ! 1-3 scale

[Term]
id: CO_343:0000393
name: Appearance of tuber surface estimation 1-4
namespace: YamTrait
def: "Visual observation of the presence of roots, thorns, and sprouted buds observed on tuber surface and making a visual score using a 1-4 scale where 1= Rough, 2= Hairy (few scattered or many roots in the surface of the tuber), 3= Thorny (small prominences ending in a small thorn) and 4= Fully smooth" []
synonym: "Tbrappr_E_1to4" EXACT []
is_a: CO_343:1000003 ! Variable
relationship: variable_of CO_343:0000188 ! tuber appearance
relationship: variable_of CO_343:0010127 ! tuber surface appearance - estimation
relationship: variable_of CO_343:0100023 ! 1-4 scale

[Term]
id: CO_343:0000394
name: Tuber surface texture estimation 1-2
namespace: YamTrait
def: "The smoothness or roughness of tuber surface is recorded using a 1-2 scale where 1= Smooth and 2= Rough" []
synonym: "Tubtxtur_E_1or2" EXACT []
is_a: CO_343:1000003 ! Variable
relationship: variable_of CO_343:0000141 ! tuber surface texture
relationship: variable_of CO_343:0010128 ! tuber surface texture - estimation
relationship: variable_of CO_343:0100027 ! 1-2 scale

[Term]
id: CO_343:0000395
name: Tuber thorniness estimation 0&1
namespace: YamTrait
def: "The presence or absence of thorns or spines on the tuber surface is recorded using a binary scale of 0-1 where 0= Absent and 1= Present" []
synonym: "Thorn" EXACT []
synonym: "Thorn_E_0or1" EXACT []
is_a: CO_343:1000003 ! Variable
relationship: variable_of CO_343:0000144 ! tuber thorniness
relationship: variable_of CO_343:0010129 ! tuber thorniness - estimation
relationship: variable_of CO_343:0100045 ! 0-1 binary scale

[Term]
id: CO_343:0000396
name: tuber thorniness intensity
namespace: YamTrait
def: "Intensity of thorns on the tuber surface" []
synonym: "Spine intensity on tubers" EXACT []
synonym: "Tbrspnint" EXACT []
synonym: "ThornInt" EXACT []
is_a: CO_343:1000008 ! Agronomical_trait
created_by: A.Amele

[Term]
id: CO_343:0000397
name: Tuber thorniness intensity estimation 0-7
namespace: YamTrait
def: "The degree and intensity of thorns or spines on tuber surface is recorded in visual scale of 0-7 where 0= no thorns or spines on tuber surface, 3= few thorns or spines on tuber surface and 7= Many thorns or spines on tuber surface" []
synonym: "ThornInt_E_0to7" EXACT []
is_a: CO_343:1000003 ! Variable
relationship: variable_of CO_343:0000396 ! tuber thorniness intensity
relationship: variable_of CO_343:0010130 ! tuber thorniness intensity-estimation
relationship: variable_of CO_343:0100046 ! 0-7 scale

[Term]
id: CO_343:0000398
name: big size tuber length
namespace: YamTrait
def: "Average length of big size tubers harvested in a net plot or unit area" []
synonym: "Btbrleng" EXACT []
is_a: CO_343:1000008 ! Agronomical_trait
created_by: A.Amele

[Term]
id: CO_343:0000399
name: Big tuber length computation in cm
namespace: YamTrait
def: "Measurement and recording in cm the length and average of at most five big size tubers (≥1kg) from base to tip in a net plot at harvest" []
synonym: "Btbrleng_Comp_cm" EXACT []
is_a: CO_343:1000003 ! Variable
relationship: variable_of CO_343:0000398 ! big size tuber length
relationship: variable_of CO_343:0010131 ! length of big size tubers-computation
relationship: variable_of CO_343:0100009 ! cm

[Term]
id: CO_343:0000400
name: medium size tuber length
namespace: YamTrait
def: "Average length of medium size tubers harvested in a net plot or unit area" []
synonym: "Mtbrleng" EXACT []
is_a: CO_343:1000008 ! Agronomical_trait
created_by: A.Amele

[Term]
id: CO_343:0000401
name: Medium size tuber length computation in cm
namespace: YamTrait
def: "Measurement and recording in cm the length and average of at most five medium size tubers (≥500 gm and <1kg ) from base to tip in a net plot at harvest" []
synonym: "Mtbrleng_Comp_cm" EXACT []
is_a: CO_343:1000003 ! Variable
relationship: variable_of CO_343:0000400 ! medium size tuber length
relationship: variable_of CO_343:0010132 ! length of medium size tubers-computation
relationship: variable_of CO_343:0100009 ! cm

[Term]
id: CO_343:0000402
name: small size tuber length
namespace: YamTrait
def: "Average length of small size tubers harvested in a net plot or unit area" []
synonym: "Stbrleng" EXACT []
is_a: CO_343:1000008 ! Agronomical_trait
created_by: A.Amele

[Term]
id: CO_343:0000403
name: Small size tuber length computation in cm
namespace: YamTrait
def: "Measurement and recording in cm the length and average of at most five small size tubers (<500 gm) from base to tip in a net plot at harvest or unit area" []
synonym: "Stbrleng_Comp_cm" EXACT []
is_a: CO_343:1000003 ! Variable
relationship: variable_of CO_343:0000402 ! small size tuber length
relationship: variable_of CO_343:0010133 ! length of small size tubers-computation
relationship: variable_of CO_343:0100009 ! cm

[Term]
id: CO_343:0000404
name: tuber length
namespace: YamTrait
def: "Average length of all size tubers harvested in a net plot or unit area" []
synonym: "TBRL" EXACT []
synonym: "Tbrleng" EXACT []
is_a: CO_343:1000010 ! Morphological_trait
created_by: A.Amele

[Term]
id: CO_343:0000405
name: Average tuber length measurement in cm
namespace: YamTrait
def: "Computation of average length ( in cm) of all tuber size measurement taken in a net plot or unit area" []
synonym: "TBRL" EXACT []
synonym: "Tbrleng_Comp_cm" EXACT []
is_a: CO_343:1000003 ! Variable
relationship: variable_of CO_343:0000404 ! tuber length
relationship: variable_of CO_343:0010134 ! tuber length-computation
relationship: variable_of CO_343:0100009 ! cm

[Term]
id: CO_343:0000406
name: Tuber shape estimation 1-4
namespace: YamTrait
def: "Determination of tuber predominant shape in the entire family/plot as a unit by visual assessment using a 1-4 scale where 1= Spherical, 2= Oval, 3= Cylindrical and 4= Irregular" []
synonym: "TbrSh_E_1to4" EXACT []
synonym: "TUBSHA" EXACT []
is_a: CO_343:1000003 ! Variable
relationship: variable_of CO_343:0000024 ! tuber shape
relationship: variable_of CO_343:0010135 ! tuber shape - estimation
relationship: variable_of CO_343:0100047 ! 1-4 score

[Term]
id: CO_343:0000407
name: Tuber size estimation 1-3
namespace: YamTrait
def: "Determination of predominant size of the tuber in the entire family using a 1-3 scale where 1= Small (less than 15 cm length), 2= Medium (between 15 and 25 cm length), 3= large (More than 25 cm length)" []
synonym: "TbrSz_E_1to3" EXACT []
synonym: "TUBSIZE" EXACT []
is_a: CO_343:1000003 ! Variable
relationship: variable_of CO_343:0000027 ! tuber size
relationship: variable_of CO_343:0010136 ! tuber size - estimation
relationship: variable_of CO_343:0100022 ! 1-3 scale

[Term]
id: CO_343:0000408
name: big size tuber width
namespace: YamTrait
def: "Average width of big size tubers harvested in a net plot or unit area" []
synonym: "Btbrwd" EXACT []
synonym: "Btbrwidth" EXACT []
is_a: CO_343:1000008 ! Agronomical_trait
created_by: A.Amele

[Term]
id: CO_343:0000409
name: Big tuber width computation in cm
namespace: YamTrait
def: "Measurement and recording the width and average (in cm) of at most five big size tubers (≥1kg) from net plot at wider portion of the tuber using vernier calliper or measuring tape" []
synonym: "Btbrwd_Comp_cm" EXACT []
synonym: "Btbrwidth" EXACT []
is_a: CO_343:1000003 ! Variable
relationship: variable_of CO_343:0000408 ! big size tuber width
relationship: variable_of CO_343:0010137 ! width of big size tubers-computation
relationship: variable_of CO_343:0100009 ! cm

[Term]
id: CO_343:0000410
name: medium size tuber width
namespace: YamTrait
def: "Average width of medium size tubers harvested in a net plot or unit area" []
synonym: "Mtbrwd" EXACT []
synonym: "Mtbrwidth" EXACT []
is_a: CO_343:1000008 ! Agronomical_trait
created_by: A.Amele

[Term]
id: CO_343:0000411
name: Medium tuber width computation in cm
namespace: YamTrait
def: "Measurement and recording the width and average (in cm)of at most five medium size tubers (≥500 gm and <1kg )from net plot at wider portion of the tuber using calliper or measuring tape" []
synonym: "Mtbrwd_Comp_cm" EXACT []
synonym: "Mtbrwidth" EXACT []
is_a: CO_343:1000003 ! Variable
relationship: variable_of CO_343:0000410 ! medium size tuber width
relationship: variable_of CO_343:0010138 ! width of medium size tubers-computation
relationship: variable_of CO_343:0100009 ! cm

[Term]
id: CO_343:0000412
name: small size tuber width
namespace: YamTrait
def: "Average width of small size tubers harvested in a net plot or unit area" []
synonym: "Stbrwd" EXACT []
synonym: "Stbrwidth" EXACT []
is_a: CO_343:1000008 ! Agronomical_trait
created_by: A.Amele

[Term]
id: CO_343:0000413
name: Small tuber width computation in cm
namespace: YamTrait
def: "Measurement and recording the width and average ( in cm) of at most five small size tubers (<500 gm) from net plot at wider portion of the tuber using calliper or measuring tape" []
synonym: "Stbrwd_Comp_cm" EXACT []
synonym: "Stbrwidth" EXACT []
is_a: CO_343:1000003 ! Variable
relationship: variable_of CO_343:0000412 ! small size tuber width
relationship: variable_of CO_343:0010139 ! width of small size tubers-computation
relationship: variable_of CO_343:0100009 ! cm

[Term]
id: CO_343:0000414
name: tuber width
namespace: YamTrait
def: "Average width of all size tubers harvested in a net plot or unit area" []
synonym: "Tbrwd" EXACT []
synonym: "tbrwidth" EXACT []
is_a: CO_343:1000008 ! Agronomical_trait
created_by: A.Amele

[Term]
id: CO_343:0000415
name: Average tuber width computation in cm
namespace: YamTrait
def: "Computation of average width (in cm) of all tuber size harvested in a net plot or unit area" []
synonym: "Tbrwd_Comp_cm" EXACT []
synonym: "tbrwidth" EXACT []
is_a: CO_343:1000003 ! Variable
relationship: variable_of CO_343:0000414 ! tuber width
relationship: variable_of CO_343:0010140 ! tuber wideth-computation
relationship: variable_of CO_343:0100009 ! cm

[Term]
id: CO_343:0000416
name: tuber cracks
namespace: YamTrait
def: "Cracks on tuber surface" []
synonym: "CTBRS" EXACT []
is_a: CO_343:1000008 ! Agronomical_trait
created_by: A.Amele

[Term]
id: CO_343:0000417
name: Tuber surface crack estimation 0-3
namespace: YamTrait
def: "The appearance of cracks on tuber surface is recorded using a 0-3 scale where 0= Absent, 1= few and 2= many" []
synonym: "CTBRS_E_0to3" EXACT []
is_a: CO_343:1000003 ! Variable
relationship: variable_of CO_343:0000416 ! tuber cracks
relationship: variable_of CO_343:0010141 ! cracks on the tuber surface-estimation
relationship: variable_of CO_343:0100048 ! 0-3 scale

[Term]
id: CO_343:0000418
name: crazy roots presence
namespace: YamTrait
def: "Appearance of crazy roots on tuber surface" []
synonym: "CRZROOT" EXACT []
is_a: CO_343:1000008 ! Agronomical_trait
created_by: A.Amele

[Term]
id: CO_343:0000419
name: Crazy roots presence estimation  0&1
namespace: YamTrait
def: "The appearance of crazy roots on tuber surface at harvest is recorded using a 0-1 scale where 0= Absent and 1= Present" []
synonym: "CRZROOT_E_1to 2" EXACT []
is_a: CO_343:1000003 ! Variable
relationship: variable_of CO_343:0000418 ! crazy roots presence
relationship: variable_of CO_343:0010142 ! crazy roots presence on tubers at harvest-estimation
relationship: variable_of CO_343:0100049 ! 0-1  scale

[Term]
id: CO_343:0000420
name: corm on tuber
namespace: YamTrait
def: "Presence or absence of corm on tuber" []
synonym: "corm" EXACT []
is_a: CO_343:1000008 ! Agronomical_trait
created_by: A.Amele

[Term]
id: CO_343:0000421
name: Corm estimation binary 0&1
namespace: YamTrait
def: "Visual assessment of the presence or absence of corm on tubers using a binary scale of 0-1 where 0= Absent and 1= Present" []
synonym: "Corm" EXACT []
is_a: CO_343:1000003 ! Variable
relationship: variable_of CO_343:0000420 ! corm on tuber
relationship: variable_of CO_343:0010143 ! corm on tubers-estimation
relationship: variable_of CO_343:0100049 ! 0-1  scale

[Term]
id: CO_343:0000422
name: corm separability from tuber
namespace: YamTrait
def: "Corm separation from tuber" []
synonym: "cormsep" EXACT []
synonym: "corsep" EXACT []
is_a: CO_343:1000008 ! Agronomical_trait
created_by: A.Amele

[Term]
id: CO_343:0000423
name: Separability of corm estimation binary 0&1
namespace: YamTrait
def: "Recording the separation of corm from tuber using a binary scale of 0-1 where 0= No and 1= Yes" []
synonym: "cormsep" EXACT []
synonym: "Corsep_E_0to1" EXACT []
is_a: CO_343:1000003 ! Variable
relationship: variable_of CO_343:0000422 ! corm separability from tuber
relationship: variable_of CO_343:0010144 ! corm separation from tuber-estimation
relationship: variable_of CO_343:0100049 ! 0-1  scale

[Term]
id: CO_343:0000424
name: corm size
namespace: YamTrait
def: "Size of corm in relation to tuber" []
synonym: "Cormsize" EXACT []
synonym: "corsz" EXACT []
is_a: CO_343:1000010 ! Morphological_trait
created_by: A.Amele

[Term]
id: CO_343:0000425
name: Corm size estimation 1-3
namespace: YamTrait
def: "Recording the size of corm in relation to tuber size using a 1-3 scale where 1= small, 2= intermediate and 3= large" []
synonym: "Cormsize" EXACT []
synonym: "Corsz_E_1to3" EXACT []
is_a: CO_343:1000003 ! Variable
relationship: variable_of CO_343:0000424 ! corm size
relationship: variable_of CO_343:0010145 ! corm size-estimation
relationship: variable_of CO_343:0100011 ! 1-3 general scale

[Term]
id: CO_343:0000426
name: corm type
namespace: YamTrait
def: "Corm type" []
synonym: "Cormtype" EXACT []
synonym: "cortyp" EXACT []
is_a: CO_343:1000010 ! Morphological_trait
created_by: A.Amele

[Term]
id: CO_343:0000427
name: Corm type estimation 1-3
namespace: YamTrait
def: "Recording the corm type as regular, transversally elongated or brached using a 1-3 scalewhere 1= regular, 2= transversally elongated and 3= branched" []
synonym: "Cormtype" EXACT []
synonym: "Cortyp_E_1to3" EXACT []
is_a: CO_343:1000003 ! Variable
relationship: variable_of CO_343:0000426 ! corm type
relationship: variable_of CO_343:0010146 ! corm type-estimation
relationship: variable_of CO_343:0100011 ! 1-3 general scale

[Term]
id: CO_343:0000428
name: Tuber dormancy period estimation
namespace: YamTrait
def: "Visual assessment and rating of dormancy period of sprouted tubers at different time interval (once a week) from harvesting up to three months after harvesting using a 1-4 scale where 1= Very short (More than 50 % of the tubers sprouted at harvesting time), 2= Short (More than 50% of the tubers sprouted at one month after harvesting time), 3= Mediun (More than 50% of the tubers sprouted at two month after harvesting time) and 4= Long (More than 50% of the tubers sprouted at three month after harvesting time)" []
synonym: "Dorm" EXACT []
synonym: "TubDorm_E_1to4" EXACT []
is_a: CO_343:1000003 ! Variable
relationship: variable_of CO_343:0000036 ! tuber dormancy period
relationship: variable_of CO_343:0010147 ! dormancy period -estimation
relationship: variable_of CO_343:0100016 ! 1-4 general scale

[Term]
id: CO_343:0000429
name: Dry matter content percentage
namespace: YamTrait
def: "Computation of the proportion in % of dry matter in the tuber by selecting at least five random whole tubers from a net plot and cut small slices (1-2 mm) from proximal, middle and distal portion and mixed thoroughly; then Visual assessment of fresh weight and determing dry weight of samples by drying at 70°C for 72 h in a forced air oven and the proportion between the dry weight and the fresh weight is calculated." []
synonym: "TDMC" EXACT []
synonym: "TubDMC_Comp_pct" EXACT []
is_a: CO_343:1000003 ! Variable
relationship: variable_of CO_343:0000174 ! tuber dry matter content
relationship: variable_of CO_343:0010148 ! tuber dry matter content - computation
relationship: variable_of CO_343:0100006 ! %

[Term]
id: CO_343:0000430
name: Tuber flesh color upper portion estimation 1-9
namespace: YamTrait
def: "Observation and recording of fresh cut tuber flesh surface color at the head portion of the tuber at harvesting time using a 1-7 scale where 1= White, 2= Creamy white, 3= Yellow, 4= Purple, 5= Purplish white, 6= creamy, 7= brownish white, 8= deep purple and 9=orange" []
synonym: "Flcolr_head" EXACT []
synonym: "Tbrfcu _E_1to9" EXACT []
is_a: CO_343:1000003 ! Variable
relationship: variable_of CO_343:0000147 ! tuber flesh color
relationship: variable_of CO_343:0010149 ! tuber flesh color head portion - estimation
relationship: variable_of CO_343:0100012 ! 1-7 general scale

[Term]
id: CO_343:0000431
name: Tuber flesh color middle portion estimation 1-9
namespace: YamTrait
def: "Observation and recording of fresh cut flesh surface color at the middle part of the tuber at harvesting time using a 1-7 scale where 1= White, 2= Creamy white, 3= Yellow, 4= Purple, 5= Purplish white, 6= creamy, 7= brownish white, 8= deep purple and 9=orange" []
synonym: "Flcolr_middle" EXACT []
synonym: "Tbrfcm _E_1to9" EXACT []
is_a: CO_343:1000003 ! Variable
relationship: variable_of CO_343:0000147 ! tuber flesh color
relationship: variable_of CO_343:0010150 ! tuber flesh color middle portion - estimation
relationship: variable_of CO_343:0100012 ! 1-7 general scale

[Term]
id: CO_343:0000432
name: Tuber flesh color lower portion estimation 1-9
namespace: YamTrait
def: "Observation and recording of fresh cut tuber flesh surface color at the tail portion of the tuber at harvesting time using a 1-7 scale where 1= White, 2= Creamy white, 3= Yellow, 4= Purple, 5= Purplish white, 6= creamy, 7= brownish white, 8= deep purple and 9=orange" []
synonym: "Flcolr_tail" EXACT []
synonym: "Tbrfcl _E_1to9" EXACT []
is_a: CO_343:1000003 ! Variable
relationship: variable_of CO_343:0000147 ! tuber flesh color
relationship: variable_of CO_343:0010151 ! tuber flesh color lower or tail portion- estimation
relationship: variable_of CO_343:0100012 ! 1-7 general scale

[Term]
id: CO_343:0000434
name: Tuber flesh color measurement
namespace: YamTrait
def: "Measurement of flesh surface color of yam tuber flesh (head, middle and tail portion) at different time interval (0, 30, 60, 180 minutes after cutting) using colorimeter (a color spectrophotometer) or standard color chart." []
synonym: "Tbrflcolr" EXACT []
synonym: "TFCR_M_color" EXACT []
is_a: CO_343:1000003 ! Variable
relationship: variable_of CO_343:0000147 ! tuber flesh color
relationship: variable_of CO_343:0010152 ! tuber flesh color reading -measurement
relationship: variable_of CO_343:0100033 ! number

[Term]
id: CO_343:0000435
name: tuber flesh cross-section color uniformity
namespace: YamTrait
def: "Uniformity of tuber flesh surface color in cross-section ( from cortex to center)" []
synonym: "flcol_uni" EXACT []
synonym: "Utfc" EXACT []
is_a: CO_343:1000007 ! Quality_trait
created_by: A.Amele

[Term]
id: CO_343:0000436
name: Uniformity of tuber flesh color estimation binary 0&1
namespace: YamTrait
def: "The uniformity of tuber flesh surface color in cross-section is recorded using visual scale of 0-1 at fresh cut during harvest where 0= not uniform and 1= uniform" []
synonym: "flcol_uni" EXACT []
synonym: "Utfc_E_0to1" EXACT []
is_a: CO_343:1000003 ! Variable
relationship: variable_of CO_343:0000435 ! tuber flesh cross-section color uniformity
relationship: variable_of CO_343:0010153 ! tuber flesh cross section color uniformity-estimation
relationship: variable_of CO_343:0100007 ! 0-1 scale

[Term]
id: CO_343:0000437
name: tuber flesh oxidation intensity
namespace: YamTrait
def: "Intensity of tuber flesh enzymatic oxidation (degree of flesh color change or browning of cut yam tuber)" []
synonym: "Intoxd" EXACT []
is_a: CO_343:1000007 ! Quality_trait
created_by: A.Amele

[Term]
id: CO_343:0000438
name: Intensity of tuber flesh oxidation estimation 0-3
namespace: YamTrait
def: "The intensity of tuber flesh oxidation (degree of flesh surface color change or browning of cut yam tuber) is scored at different time interval (0, 30, 60, 180 minutes after cutting) using a 0-3 scale where 0= no oxidization, 1= slightly oxidizing and 3= highly oxidizing" []
synonym: "Intoxd_E_0to3" EXACT []
is_a: CO_343:1000003 ! Variable
relationship: variable_of CO_343:0000437 ! tuber flesh oxidation intensity
relationship: variable_of CO_343:0010154 ! tuber flesh oxidation intensity-estimation
relationship: variable_of CO_343:0100048 ! 0-3 scale

[Term]
id: CO_343:0000439
name: tuber flesh texture
namespace: YamTrait
def: "Texture of tuber flesh" []
synonym: "Txf" EXACT []
is_a: CO_343:1000007 ! Quality_trait
created_by: A.Amele

[Term]
id: CO_343:0000440
name: Fresh tuber flesh texture estimation 1-3
namespace: YamTrait
def: "The texture of tuber flesh is recorded using a 1-3 scale where 1= smooth, 2=grainy and 3= very grainy" []
synonym: "Txf_E_1to3" EXACT []
is_a: CO_343:1000003 ! Variable
relationship: variable_of CO_343:0000439 ! tuber flesh texture
relationship: variable_of CO_343:0010155 ! tuber flesh texture-estimation
relationship: variable_of CO_343:0100022 ! 1-3 scale

[Term]
id: CO_343:0000441
name: Tuber oxidation estimation 1-3
namespace: YamTrait
def: "Visual assessment of tuber flesh enzymatic oxidation rate by recording the time in minutes lasted for cut tuber flesh to become or not oxidized and scored using a 1-3 scale, where 1= oxidizes less than a minure, 2= oxidizes between 1 and 2 minure after cutting, and 3= oxidizes more than 3 minutes." []
synonym: "Oxid" EXACT []
synonym: "Tfoxd_E_1to3" EXACT []
is_a: CO_343:1000003 ! Variable
relationship: variable_of CO_343:0000150 ! tuber flesh oxidation
relationship: variable_of CO_343:0010156 ! tuber oxidation-estimation
relationship: variable_of CO_343:0100022 ! 1-3 scale

[Term]
id: CO_343:0000442
name: tuber flesh oxidation color
namespace: YamTrait
def: "Surface color resulting of tuber flesh enzymatic oxidation" []
synonym: "Foxdc" EXACT []
is_a: CO_343:1000007 ! Quality_trait
created_by: A.Amele

[Term]
id: CO_343:0000443
name: Flesh oxidation color estimation 1-4
namespace: YamTrait
def: "Visual assessment of the surface color resulting of tuber flesh enzymatic oxidation color using a 1-4 color scale, where 1= grey, 2=purple, 3=orange and 4=brown." []
synonym: "Foxdc_E_1to4" EXACT []
is_a: CO_343:1000003 ! Variable
relationship: variable_of CO_343:0000442 ! tuber flesh oxidation color
relationship: variable_of CO_343:0010157 ! tuber flesh oxidation color-estimation
relationship: variable_of CO_343:0100023 ! 1-4 scale

[Term]
id: CO_343:0000444
name: cohesiveness of pounded yam
namespace: YamTrait
def: "Degree to which particles of a sample stick together or how moldable it is" []
synonym: "cohpdym" EXACT []
is_a: CO_343:1000007 ! Quality_trait
created_by: A.Amele

[Term]
id: CO_343:0000445
name: Cohesiveness estimation 1-3
namespace: YamTrait
def: "Visual assessment of the degree to which particles of a sample stick together or how moldable it is using a 1-3 scale where 1= not cohesive, 2= slightly cohesive and 3= cohesive" []
synonym: "Cohpdym_E_1to3" EXACT []
is_a: CO_343:1000003 ! Variable
relationship: variable_of CO_343:0000444 ! cohesiveness of pounded yam
relationship: variable_of CO_343:0010158 ! cohesiveness of pounded yam- estimation
relationship: variable_of CO_343:0100022 ! 1-3 scale

[Term]
id: CO_343:0000446
name: springiness of pounded yam
namespace: YamTrait
def: "Distance to which the deformed material can be sretchable" []
synonym: "sprgpdym" EXACT []
synonym: "Strepdym" EXACT []
synonym: "tretchability or elasticity of pounded yam" EXACT []
is_a: CO_343:1000007 ! Quality_trait
created_by: A.Amele

[Term]
id: CO_343:0000447
name: Springness estimation 1-2
namespace: YamTrait
def: "Scoring of the distance to which the deformed material can be stretched or degree of stretchability of pounded yam using a 1-2 intensity scale, where 1=springy and 2= not springy or plastic." []
synonym: "Sprgpdym_E_1to2" EXACT []
synonym: "Strepdym" EXACT []
is_a: CO_343:1000003 ! Variable
relationship: variable_of CO_343:0000446 ! springiness of pounded yam
relationship: variable_of CO_343:0010159 ! springiness of pounded yam-estimation
relationship: variable_of CO_343:0100027 ! 1-2 scale

[Term]
id: CO_343:0000448
name: smoothness of pounded yam
namespace: YamTrait
def: "Smoothnessof the material, i.e., absence of lumps" []
synonym: "smthpdym" EXACT []
is_a: CO_343:1000007 ! Quality_trait
created_by: A.Amele

[Term]
id: CO_343:0000449
name: Smoothness estimation 1-3
namespace: YamTrait
def: "Visual assessment and scoring of the smoothness of pounded yam , i.e., absence of lumps by finger feeling using a 1-3 scale where 1= big lumps, 2=small lumps and 3= no lumps" []
synonym: "Smthpdym_E_1to3" EXACT []
is_a: CO_343:1000003 ! Variable
relationship: variable_of CO_343:0000448 ! smoothness of pounded yam
relationship: variable_of CO_343:0010160 ! smoothness of pounded yam- estimation
relationship: variable_of CO_343:0100022 ! 1-3 scale

[Term]
id: CO_343:0000450
name: fibrousness of pounded yam
namespace: YamTrait
def: "Presenceof ﬁber strands" []
synonym: "fbrpdym" EXACT []
is_a: CO_343:1000007 ! Quality_trait
created_by: A.Amele

[Term]
id: CO_343:0000451
name: Fiber estimation 1-2
namespace: YamTrait
def: "Visual assessment of the presence or absence of ﬁber strands on pounded yam using a 1-2 scale where 1= fibrous and 2= not fibrous" []
synonym: "Fbrpdym_E_1to2" EXACT []
is_a: CO_343:1000003 ! Variable
relationship: variable_of CO_343:0000450 ! fibrousness of pounded yam
relationship: variable_of CO_343:0010161 ! presence of fiber strand-estimation
relationship: variable_of CO_343:0100027 ! 1-2 scale

[Term]
id: CO_343:0000452
name: Stickiness estimation 1-3
namespace: YamTrait
def: "Visual assessment of the degree of stickines or adhesiveness of pounded yam to consumers fingers, mouth surface and teeth using sensory test panelist with a scale of 1-3 where 1= sticky, 2= slightly sticky and 3= Not sticky" []
synonym: "adhpdym_E_1to3" EXACT []
synonym: "Con_Stick_PY" EXACT []
is_a: CO_343:1000003 ! Variable
relationship: variable_of CO_343:0000191 ! stickiness of pounded yam
relationship: variable_of CO_343:0010162 ! stickiness of pounded yam - estimation
relationship: variable_of CO_343:0100011 ! 1-3 general scale

[Term]
id: CO_343:0000453
name: Taste estimation 1-5
namespace: YamTrait
def: "The taste of pounded yam without any additional complementary food is scored using sensory test panalist with a scale of 1-5 where 1= very bitter, 2= Slightly bitter, 3= Neutral, 4= sweet and 5= very sweet" []
synonym: "Con_Taste_PY" EXACT []
synonym: "TastPdym_E_1to5" EXACT []
is_a: CO_343:1000003 ! Variable
relationship: variable_of CO_343:0000194 ! taste of pounded yam
relationship: variable_of CO_343:0010163 ! taste of pounded yam - estimation
relationship: variable_of CO_343:0100008 ! 1-5 scale

[Term]
id: CO_343:0000454
name: scale insect infestation
namespace: YamTrait
def: "Scale insect infestation on tubers at harvest" []
synonym: "Scalisec" EXACT []
is_a: CO_343:1000005 ! Biotic_stress_trait
created_by: A.Amele

[Term]
id: CO_343:0000455
name: Scale insect infestation estimation 0-2
namespace: YamTrait
def: "Visual observation and scoring of insect infestation on tuber at harvest using a 0-2 scale where 0= Abesnt, 1= Few, 2= Many" []
synonym: "Sclinsct_E_0to2" EXACT []
is_a: CO_343:1000003 ! Variable
relationship: variable_of CO_343:0000454 ! scale insect infestation
relationship: variable_of CO_343:0010164 ! scale insect infestation - estimation
relationship: variable_of CO_343:0100010 ! 0-2 scale

[Term]
id: CO_343:0000456
name: stem color
namespace: YamTrait
def: "The surface color of stem" []
synonym: "Stmcol" EXACT []
is_a: CO_343:1000010 ! Morphological_trait
created_by: A.Amele

[Term]
id: CO_343:0000457
name: Stem color estimatiion 1-5
namespace: YamTrait
def: "Visual assessment of the predominant color surface of stem on mature plant at five to six month after emergence using a 1-5 scale where 1= Green, 2= Purplish green, 3= Brownish green, 4= Dark brown and 5= Purple" []
synonym: "Stmcol_E_1to5" EXACT []
is_a: CO_343:1000003 ! Variable
relationship: variable_of CO_343:0000456 ! stem color
relationship: variable_of CO_343:0010165 ! stem color - estimation
relationship: variable_of CO_343:0100008 ! 1-5 scale

[Term]
id: CO_343:0000458
name: leaf density
namespace: YamTrait
def: "Variation in leaf mass of the plant" []
synonym: "leaf abundance" EXACT []
synonym: "lfab" EXACT []
synonym: "Lfden" EXACT []
is_a: CO_343:1000010 ! Morphological_trait
created_by: A.Amele

[Term]
id: CO_343:0000459
name: Leaf density estimation 1-7
namespace: YamTrait
def: "Observation of variation in leaf mass or abundance on a mature plant and rate the density using a 1-7 scale where 3= Low, 5= Intermediate and 7= High" []
synonym: "Lfden_E_1to7" EXACT []
is_a: CO_343:1000003 ! Variable
relationship: variable_of CO_343:0000458 ! leaf density
relationship: variable_of CO_343:0010166 ! leaf density - estimation
relationship: variable_of CO_343:0100050 ! 1-7 scale

[Term]
id: CO_343:0000460
name: branch number
namespace: YamTrait
def: "Number of branches above ground" []
synonym: "branch" EXACT []
is_a: CO_343:1000010 ! Morphological_trait
created_by: A.Amele

[Term]
id: CO_343:0000461
name: Number of branches per plant count
namespace: YamTrait
def: "The number of branches above ground level is counted and the average on at least five mature plants in a plot is recorded" []
synonym: "Branch_comp_number/plt" EXACT []
is_a: CO_343:1000003 ! Variable
relationship: variable_of CO_343:0000460 ! branch number
relationship: variable_of CO_343:0010167 ! number of branchs - computation
relationship: variable_of CO_343:0100051 ! number of branch

[Term]
id: CO_343:0000462
name: stem height
namespace: YamTrait
def: "Height or the length of stem" []
synonym: "Stmht" EXACT []
synonym: "vine length" EXACT []
synonym: "vinlgt" EXACT []
is_a: CO_343:1000010 ! Morphological_trait
created_by: A.Amele

[Term]
id: CO_343:0000463
name: Stem height measurement in m
namespace: YamTrait
def: "Measurement of length or height of stem or vine (in m) and the average of at least five mature plants in a plot is recorded using measuring tape at five to six months after sprout emergence" []
synonym: "Stmht_Comp_m" EXACT []
is_a: CO_343:1000003 ! Variable
relationship: variable_of CO_343:0000462 ! stem height
relationship: variable_of CO_343:0010168 ! stem height - computation
relationship: variable_of CO_343:0100052 ! m

[Term]
id: CO_343:0000464
name: number of leaves
namespace: YamTrait
def: "The number of leaves on a plant" []
synonym: "Nlfyp" EXACT []
is_a: CO_343:1000010 ! Morphological_trait
created_by: A.Amele

[Term]
id: CO_343:0000465
name: Number of leaves per plant count
namespace: YamTrait
def: "The number of leaves on a plant is counted and the average on at least five young plants in a plot at 30 days after emergence is recorded" []
synonym: "Nlfyp_comp_number/plt" EXACT []
is_a: CO_343:1000003 ! Variable
relationship: variable_of CO_343:0000464 ! number of leaves
relationship: variable_of CO_343:0010169 ! number of leaves - computation
relationship: variable_of CO_343:0100053 ! number of leaf

[Term]
id: CO_343:0000466
name: leaf position
namespace: YamTrait
def: "Arrangement of leaves on stem or vine" []
synonym: "leaf arrangement" EXACT []
synonym: "lfarng" EXACT []
synonym: "lfpst" EXACT []
is_a: CO_343:1000010 ! Morphological_trait
created_by: A.Amele

[Term]
id: CO_343:0000467
name: Leaf position estiamtion 1-3
namespace: YamTrait
def: "Visual observation of the arrangement of leaves on stem or vine and rated using a 1-3 scale where 1= Alternate, 2= Opposite and 3= Alternate at base, opposite above" []
synonym: "Lfpst_E_1to3" EXACT []
is_a: CO_343:1000003 ! Variable
relationship: variable_of CO_343:0000466 ! leaf position
relationship: variable_of CO_343:0010170 ! leaf position - estimation
relationship: variable_of CO_343:0100022 ! 1-3 scale

[Term]
id: CO_343:0000468
name: leaf length
namespace: YamTrait
def: "Length of leaf" []
synonym: "lflngth" EXACT []
is_a: CO_343:1000010 ! Morphological_trait
created_by: A.Amele

[Term]
id: CO_343:0000469
name: Leaf length measurement in cm
namespace: YamTrait
def: "Measurement of the length of leaf from lobes to the tip ( in cm) using a measuring tape on sampled 20 adult leaves ( four leaves per plant and at leat five plants on a plot), and recording the average length" []
synonym: "Lflngth_Comp_cm" EXACT []
is_a: CO_343:1000003 ! Variable
relationship: variable_of CO_343:0000468 ! leaf length
relationship: variable_of CO_343:0010171 ! leaf length - computation
relationship: variable_of CO_343:0100009 ! cm

[Term]
id: CO_343:0000470
name: leaf width
namespace: YamTrait
def: "Width of leaf" []
synonym: "lfwdt" EXACT []
is_a: CO_343:1000010 ! Morphological_trait
created_by: A.Amele

[Term]
id: CO_343:0000471
name: Leaf width measurement in cm
namespace: YamTrait
def: "Measurement of the width of leaf ( in cm) from its widest part using a measuring tape on sampled 20 adult leaves ( four leaves per plant on at leat five plants in a plot), and recording the average width" []
synonym: "Lfwdt_Comp_cm" EXACT []
is_a: CO_343:1000003 ! Variable
relationship: variable_of CO_343:0000470 ! leaf width
relationship: variable_of CO_343:0010172 ! leaf width - computation
relationship: variable_of CO_343:0100009 ! cm

[Term]
id: CO_343:0000472
name: Internode length measurement in cm
namespace: YamTrait
def: "Measurement of the internode length (in cm ) at 1m height on five (5) plants and record the average" []
synonym: "Intndlgth_Comp_CM" EXACT []
is_a: CO_343:1000003 ! Variable
relationship: variable_of CO_343:0000230 ! internode length
relationship: variable_of CO_343:0010173 ! internode length - computation
relationship: variable_of CO_343:0100009 ! cm

[Term]
id: CO_343:0000473
name: stem hairiness
namespace: YamTrait
def: "Hairiness of stem" []
synonym: "stmhair" EXACT []
is_a: CO_343:1000010 ! Morphological_trait
created_by: A.Amele

[Term]
id: CO_343:0000474
name: Stem hairiness estimation 0-2
namespace: YamTrait
def: "Visual observation of the presence or absence of hairs on stem surface using a 0-2 scale where 0= Absent, 1= Sparse and 2= Dense" []
synonym: "Stmhair_E_0to2" EXACT []
is_a: CO_343:1000003 ! Variable
relationship: variable_of CO_343:0000473 ! stem hairiness
relationship: variable_of CO_343:0010174 ! hair on stem - estimation
relationship: variable_of CO_343:0100010 ! 0-2 scale

[Term]
id: CO_343:0000475
name: leaf color
namespace: YamTrait
def: "The leaf surface color or pigmentation" []
synonym: "ylfcol" EXACT []
is_a: CO_343:1000010 ! Morphological_trait
created_by: A.Amele

[Term]
id: CO_343:0000476
name: Young leaf color estimation 1-5
namespace: YamTrait
def: "Visual assessment of the color or pigmentation of leaf surface on a young plant using a 1-5 scale where 1= Yellowish, 2= Pale green, 3= Dark green, 4= Purplish green and 5= Purple" []
synonym: "ylfcol_E_1to5" EXACT []
is_a: CO_343:1000003 ! Variable
relationship: variable_of CO_343:0000475 ! leaf color
relationship: variable_of CO_343:0010175 ! leaf color - estimation
relationship: variable_of CO_343:0100008 ! 1-5 scale

[Term]
id: CO_343:0000477
name: Mature leaf color estimation 1-5
namespace: YamTrait
def: "Visual assessment of the color or pigmentation of leaf surface on a matured plant using a 1-5 scale where 1= Yellowish, 2= Pale green, 3= Dark green, 4= Purplish green and 5= Purple" []
synonym: "mlfcol_E_1to5" EXACT []
is_a: CO_343:1000003 ! Variable
relationship: variable_of CO_343:0000475 ! leaf color
relationship: variable_of CO_343:0010175 ! leaf color - estimation
relationship: variable_of CO_343:0100008 ! 1-5 scale

[Term]
id: CO_343:0000478
name: vein color
namespace: YamTrait
def: "Color or pigmentation of leaf vein" []
synonym: "uveincol" EXACT []
is_a: CO_343:1000010 ! Morphological_trait
created_by: A.Amele

[Term]
id: CO_343:0000479
name: Upper surface vein color estimation 1-4
namespace: YamTrait
def: "Visual assessment of the color or pigmentation of leaf vein on the upper surface using a 1-4 scale where 1= Yellowish, 2= Green, 3= Pale purple and 4= Purple" []
synonym: "uveincol_E_1to5" EXACT []
is_a: CO_343:1000003 ! Variable
relationship: variable_of CO_343:0000478 ! vein color
relationship: variable_of CO_343:0010176 ! vein color - estimation
relationship: variable_of CO_343:0100023 ! 1-4 scale

[Term]
id: CO_343:0000480
name: Lower surface vein color estimation 1-4
namespace: YamTrait
def: "Visual assessment of the color or pigmentation of leaf vein on the lower surface using a 1-4 scale where 1= Yellowish, 2= Green, 3= Pale purple and 4= Purple" []
synonym: "lveincol_E_1to5" EXACT []
is_a: CO_343:1000003 ! Variable
relationship: variable_of CO_343:0000478 ! vein color
relationship: variable_of CO_343:0010176 ! vein color - estimation
relationship: variable_of CO_343:0100023 ! 1-4 scale

[Term]
id: CO_343:0000481
name: leaf hairiness
namespace: YamTrait
def: "Hairiness of leaf surface" []
synonym: "ulfhair" EXACT []
is_a: CO_343:1000010 ! Morphological_trait
created_by: A.Amele

[Term]
id: CO_343:0000482
name: Upper surface leaf hairiness estimation 0-2
namespace: YamTrait
def: "Visual assessment of the hairiness of leaf surface (upper part) using a 0-2 scale where 0= Absent, 1= Sparse and 2= Dense" []
synonym: "ulfhair_E_0to2" EXACT []
is_a: CO_343:1000003 ! Variable
relationship: variable_of CO_343:0000481 ! leaf hairiness
relationship: variable_of CO_343:0010177 ! leaf hairiness - estimation
relationship: variable_of CO_343:0100010 ! 0-2 scale

[Term]
id: CO_343:0000483
name: Lower surface leaf hairiness estimation 0-2
namespace: YamTrait
def: "Visual assessment of the hairiness of leaf surface (lower part) using a 0-2 scale where 0= Absent, 1= Sparse and 2= Dense" []
synonym: "llfhair_E_0to2" EXACT []
is_a: CO_343:1000003 ! Variable
relationship: variable_of CO_343:0000481 ! leaf hairiness
relationship: variable_of CO_343:0010177 ! leaf hairiness - estimation
relationship: variable_of CO_343:0100010 ! 0-2 scale

[Term]
id: CO_343:0000484
name: petiole length
namespace: YamTrait
def: "Length of petiole" []
synonym: "petlngth" EXACT []
is_a: CO_343:1000010 ! Morphological_trait
created_by: A.Amele

[Term]
id: CO_343:0000485
name: Petiole length measurement in cm
namespace: YamTrait
def: "Measurement of the length of petiole and recording the average length (in cm) using measuring tape on sampled 20 adult leaves ( four leaves per plant on at leat five plants in a plot)" []
synonym: "petlngth_Comp_cm" EXACT []
is_a: CO_343:1000003 ! Variable
relationship: variable_of CO_343:0000484 ! petiole length
relationship: variable_of CO_343:0010178 ! petiole length - computation
relationship: variable_of CO_343:0100009 ! cm

[Term]
id: CO_343:0002000
name: peak viscosity
namespace: YamTrait
def: "Maximum viscosity during the heating or hold phase of the RVA test.It describes the water-holding capacity of the starch" []
synonym: "pkvisc" EXACT []
is_a: CO_343:0002006 ! Viscosity traits
created_by: aafolabi

[Term]
id: CO_343:0002001
name: trough viscosity
namespace: YamTrait
def: "Trough viscosity is the ability of the starch granules to remain undisrupted when the yam paste is subjected to a hold period of constant high temperature and mechanical shear stress" []
synonym: "tvisc" EXACT []
is_a: CO_343:0002006 ! Viscosity traits
created_by: aafolabi

[Term]
id: CO_343:0002002
name: final viscosity
namespace: YamTrait
def: "Final viscosity is the ability of the material to form a viscous paste after cooking and cooling" []
synonym: "fvisc" EXACT []
is_a: CO_343:0002006 ! Viscosity traits
created_by: aafolabi

[Term]
id: CO_343:0002003
name: breakdown
namespace: YamTrait
def: "Indicates the resistance of the starch paste to heat and shear" []
synonym: "brkdown" EXACT []
is_a: CO_343:0002006 ! Viscosity traits
created_by: aafolabi

[Term]
id: CO_343:0002004
name: setback
namespace: YamTrait
def: "the tendency of starch pastes to recrystallize and is an index of starch retrogradation or gelling ability. Recovery of the viscosity during cooling of the heated starch suspension and is related to the retrogradation and reordering of starch molecules, i.e., low setback values indicate a low rate of starch retrogradation and syneresis. Mathematically, setback = ﬁnal viscosity–trough viscosity" []
synonym: "setbck" EXACT []
is_a: CO_343:0002006 ! Viscosity traits
created_by: aafolabi

[Term]
id: CO_343:0002005
name: pasting temperature
namespace: YamTrait
def: "Measured at the onset of a rise in viscosity and may indicate the gelatinization temperature of the starch, thereby indicating the minimum temperature at which the starch should be cooked" []
is_a: CO_343:0002006 ! Viscosity traits
created_by: aafolabi

[Term]
id: CO_343:0002006
name: Viscosity traits
is_a: CO_343:1000007 ! Quality_trait

[Term]
id: CO_343:0002007
name: Peak viscosity measurement in centipoise
namespace: YamTrait
def: "The water-holding capacity of the starch or mixture using Rapid Visco Analyzer" []
synonym: "pkvsc" EXACT []
is_a: CO_343:1000003 ! Variable
relationship: variable_of CO_343:0002000 ! peak viscosity
relationship: variable_of CO_343:0012000 ! peak viscosity - measurement
relationship: variable_of CO_343:0102000 ! cP

[Term]
id: CO_343:0002008
name: Trough viscosity measurement in centipoise
namespace: YamTrait
def: "Ability of the starch granules to remain undisrupted when the yam paste is subjected to a hold period of constant high temperature and mechanical shear stress using Rapid Visco Analyzer measured in centipoise." []
synonym: "tvisc" EXACT []
is_a: CO_343:1000003 ! Variable
relationship: variable_of CO_343:0002001 ! trough viscosity
relationship: variable_of CO_343:0012001 ! trough viscosity - measurement
relationship: variable_of CO_343:0102000 ! cP

[Term]
id: CO_343:0002009
name: Final viscosity measurement in centipoise
namespace: YamTrait
def: "Ability of the material to form a viscous paste after cooking and cooling as measured using a Rapid Visco Analyzer in centipoise." []
synonym: "fvisc" EXACT []
is_a: CO_343:1000003 ! Variable
relationship: variable_of CO_343:0002002 ! final viscosity
relationship: variable_of CO_343:0012002 ! final viscosity - measurement
relationship: variable_of CO_343:0102000 ! cP

[Term]
id: CO_343:0002010
name: Breakdown measurement in centipoise
namespace: YamTrait
def: "The resistance of the starch paste to heat and shear as measured using Rapid Visco Analyzer in centipoise." []
synonym: "brkdown" EXACT []
is_a: CO_343:1000003 ! Variable
relationship: variable_of CO_343:0002003 ! breakdown
relationship: variable_of CO_343:0012003 ! breakdown - measurement
relationship: variable_of CO_343:0102000 ! cP

[Term]
id: CO_343:0002011
name: Setback measurement in centipoise
namespace: YamTrait
def: "Tendency of starch pastes to recrystallize and is an index of starch retrogradation or gelling ability. Recovery of the viscosity during cooling of the heated starch suspension and is related to the retrogradation and reordering of starch molecules, i.e., low setback values indicate a low rate of starch retrogradation and syneresis. It is measured using Rapid Visco Analyzer in centipoise." []
synonym: "setbck" EXACT []
is_a: CO_343:1000003 ! Variable
relationship: variable_of CO_343:0002004 ! setback
relationship: variable_of CO_343:0012004 ! setback - measurement
relationship: variable_of CO_343:0102000 ! cP

[Term]
id: CO_343:0002012
name: Pasting temperature measurement in degree celsius
namespace: YamTrait
def: "The pasting temperature is measured at the onset of a rise in viscosity and may indicate the gelatinization temperature of the starch, thereby indicating the minimum temperature at which the starch should be cooked." []
synonym: "ptemp" EXACT []
is_a: CO_343:1000003 ! Variable
relationship: variable_of CO_343:0002005 ! pasting temperature
relationship: variable_of CO_343:0012005 ! pasting temperature - measurement
relationship: variable_of CO_343:0102001 ! deg

[Term]
id: CO_343:0003001
name: Springness proportion
namespace: YamTrait
def: "Measurement of springiness based on Texture Profile Analysis using double compression test on pounded yam sample. Springiness is the ratio between distances from the onset to peak force of the second to the first compression cycle." []
is_a: CO_343:1000003 ! Variable
relationship: variable_of CO_343:0000446 ! springiness of pounded yam
relationship: variable_of CO_343:0010159 ! springiness of pounded yam-estimation
relationship: variable_of CO_343:0100227 ! unitless
created_by: D. Cornet

[Term]
id: CO_343:0003002
name: 'springiness of pounded yam - proportion'
namespace: YamMethod
def: "Texture Profile Analysis using double compression test allwo to define springiness as the ratio between distances from the onset to peak force of the second to the first compression cycle." []
is_a: CO_343:1000013 ! Computation
relationship: method_of CO_343:0000446 ! springiness of pounded yam
created_by: D. Cornet

[Term]
id: CO_343:0003003
name: Cohesiveness proportion
namespace: YamTrait
def: "Measurement of cohesiveness based on Texture Profile Analysis using double compression test on pounded yam sample. Cohesiveness is the area underneath the second compression curve divided by the area underneath the first compression curve." []
is_a: CO_343:1000003 ! Variable
relationship: variable_of CO_343:0000444 ! cohesiveness of pounded yam
relationship: variable_of CO_343:0010158 ! cohesiveness of pounded yam- estimation
relationship: variable_of CO_343:0100227 ! unitless
created_by: D. Cornet

[Term]
id: CO_343:0003004
name: 'cohesiveness of pounded yam- proportion'
namespace: YamMethod
def: "Texture Profile Analysis using double compression test allwo to define cohesiveness as the area underneath the second compression curve divided by the area underneath the first compression curve." []
is_a: CO_343:1000013 ! Computation
relationship: method_of CO_343:0000444 ! cohesiveness of pounded yam
created_by: D. Cornet

[Term]
id: CO_343:0003005
name: hardness of pounded yam
namespace: YamTrait
def: "Measurement of hardness of pounded yam" []
is_a: CO_343:1000007 ! Quality_trait
created_by: D. Cornet

[Term]
id: CO_343:0003006
name: Hardness of pounded yam measured in Newtons
namespace: YamTrait
def: "Measurement of hardness based on Texture Profile Analysis using double compression test on pounded yam sample. Hardness is the highest peak force measured during first compression." []
is_a: CO_343:1000003 ! Variable
relationship: variable_of CO_343:0003005 ! hardness of pounded yam
relationship: variable_of CO_343:0003007 ! Newtons
relationship: variable_of CO_343:0003008 ! hardness of pounded yam- measurement
created_by: D. Cornet

[Term]
id: CO_343:0003007
name: Newtons
namespace: YamScale
synonym: "N" EXACT []
is_a: CO_343:1000019 ! Numerical
relationship: scale_of CO_343:0003008 ! hardness of pounded yam- measurement

[Term]
id: CO_343:0003008
name: hardness of pounded yam- measurement
namespace: YamMethod
def: "Texture Profile Analysis using double compression test allwo to define hardness as the highest peak force measured during first compression in Newtons" []
is_a: CO_343:1000011 ! Measurement
relationship: method_of CO_343:0003006 ! Hardness of pounded yam measured in Newtons

[Term]
id: CO_343:0003009
name: Mouldability of pounded yam- boolean visual assesment
namespace: YamTrait
def: "Visual assessment of the ability of boiled yam to form a paste after mechanical pounding (dough or puree appearance). 0=mouldable, 1=not mouldable." []
is_a: CO_343:1000003 ! Variable
relationship: variable_of CO_343:0003010 ! Mouldability of pounded yam
relationship: variable_of CO_343:0003011 ! mouldability of pounded yam - estimation
relationship: variable_of CO_343:0100045 ! 0-1 binary scale
created_by: D. Cornet

[Term]
id: CO_343:0003010
name: Mouldability of pounded yam
namespace: YamTrait
def: "ability of pounded yam to form a paste" []
is_a: CO_343:1000007 ! Quality_trait
created_by: D. Cornet

[Term]
id: CO_343:0003011
name: mouldability of pounded yam - estimation
namespace: YamMethod
def: "Visual assessment of the ability of boiled yam to form a paste after mechanical pounding (dough or puree appearance)." []
is_a: CO_343:1000014 ! Estimation
relationship: method_of CO_343:0003010 ! Mouldability of pounded yam

[Term]
id: CO_343:0003012
name: Area under disease progression curve for yam anthracnose disease
namespace: YamTrait
def: "The area under disease progression curve for yam anthracnose disease calculated with the AUDPC formula." []
synonym: "AUDPC_YAD" EXACT []
is_a: CO_343:1000003 ! Variable
relationship: variable_of CO_343:0000021 ! yam anthracnose disease severity
relationship: variable_of CO_343:0003013 ! Area under disease progression curve for yam anthracnose disease calculation
relationship: variable_of CO_343:0003014 ! AUDPC for for yam anthracnose disease

[Term]
id: CO_343:0003013
name: Area under disease progression curve for yam anthracnose disease calculation
namespace: YamMethod
def: "Observe relative or absolute area of plant tissue affected by yam anthracnose disease and record the severity as a proportion or percentage of plant surface affected.It is visual score in scale under screenhouse, artificial inoculation or under field natural infestation. For artificial inoculation use a suspension of three most virulent strains of Colletothrichum gloeosporioides and inoculate the plants raised from vine cutting in vertical sack or other means by spraying. For natural infestation, scores can be taken 10 to 12 weeks after planting and second scoring about 4-6 weeks before harvesting . Artificial inoculation should be scored at 3 days after inoculation(DAI) , and repeated at 7DAI, 11DAI and 15DAI" []
is_a: CO_343:1000014 ! Estimation
relationship: method_of CO_343:0000021 ! yam anthracnose disease severity

[Term]
id: CO_343:0003014
name: AUDPC for for yam anthracnose disease
namespace: YamScale
is_a: CO_343:1000019 ! Numerical
relationship: scale_of CO_343:0003013 ! Area under disease progression curve for yam anthracnose disease calculation
property_value: seeAlso https://www.apsnet.org/edcenter/disimpactmngmnt/topc/EcologyAndEpidemiologyInR/DiseaseProgress/Pages/AUDPC.aspx xsd:string

[Term]
id: CO_343:0003015
name: 'Area under disease progression curve for yam mosaic virus calculation'
namespace: YamMethod
def: "Observe relative or absolute area of plant tissue affected by yam anthracnose disease and record the severity as a proportion or percentage of plant surface affected.It is visual score in scale under screenhouse, artificial inoculation or under field natural infestation. For artificial inoculation use a suspension of three most virulent strains of Colletothrichum gloeosporioides and inoculate the plants raised from vine cutting in vertical sack or other means by spraying. For natural infestation, scores can be taken 10 to 12 weeks after planting and second scoring about 4-6 weeks before harvesting . Artificial inoculation should be scored at 3 days after inoculation(DAI) , and repeated at 7DAI, 11DAI and 15DAI" []
is_a: CO_343:1000014 ! Estimation
relationship: method_of CO_343:0000021 ! yam anthracnose disease severity

[Term]
id: CO_343:0003016
name: 'AUDPC for for yam mosaic virus disease'
namespace: YamScale
is_a: CO_343:1000019 ! Numerical
relationship: scale_of CO_343:0003015 ! 'Area under disease progression curve for yam mosaic virus calculation'
property_value: seeAlso https://www.apsnet.org/edcenter/disimpactmngmnt/topc/EcologyAndEpidemiologyInR/DiseaseProgress/Pages/AUDPC.aspx xsd:string

[Term]
id: CO_343:0003017
name: Area under disease progression curve for yam mosaic virus severity disease
namespace: YamTrait
def: "The area under disease progression curve for yam mosaic virus disease calculated with the AUDPC formula." []
synonym: "AUDPC_YMV" EXACT []
is_a: CO_343:1000003 ! Variable
relationship: variable_of CO_343:0000021 ! yam anthracnose disease severity
relationship: variable_of CO_343:0003015 ! 'Area under disease progression curve for yam mosaic virus calculation'
relationship: variable_of CO_343:0003016 ! 'AUDPC for for yam mosaic virus disease'

[Term]
id: CO_343:0003018
name: Tuber flesh color L value chromameter read
namespace: YamTrait
def: "The tuber flesh color L value indicates lightness which represents quantitative relationship of colors on three axes. Colour reading using chromameter machine." []
is_a: CO_343:1000003 ! Variable
relationship: variable_of CO_343:0000147 ! tuber flesh color
relationship: variable_of CO_343:0003019 ! Tuber flesh color computation L value from chromameter machine
relationship: variable_of CO_343:0100227 ! unitless
created_by: Agre {comment="dateTime"}

[Term]
id: CO_343:0003019
name: Tuber flesh color computation L value from chromameter machine
namespace: YamMethod
def: "Compute the L value of the flesh surface color of tuber longitudinal section using chromameter machine" []
is_a: CO_343:1000013 ! Computation
relationship: variable_of CO_343:0000147 ! tuber flesh color

[Term]
id: CO_343:0003020
name: Tuber flesh color A value chromameter read
namespace: YamTrait
def: "The tuber flesh color A value indicates lightness which represents quantitative relationship of colors on three axes. Colour reading using chromameter machine." []
is_a: CO_343:1000003 ! Variable
relationship: variable_of CO_343:0000147 ! tuber flesh color
relationship: variable_of CO_343:0003021 ! Tuber flesh color computation A value from chromameter machine
relationship: variable_of CO_343:0100227 ! unitless
created_by: Agre

[Term]
id: CO_343:0003021
name: Tuber flesh color computation A value from chromameter machine
namespace: YamMethod
def: "Compute the A value of the flesh surface color of tuber longitudinal section using chromameter machine" []
is_a: CO_343:1000013 ! Computation
relationship: variable_of CO_343:0000147 ! tuber flesh color

[Term]
id: CO_343:0003022
name: Tuber flesh color B value chromameter read
namespace: YamTrait
def: "The tuber flesh color B value indicates lightness which represents quantitative relationship of colors on three axes. Colour reading using chromameter machine." []
is_a: CO_343:1000003 ! Variable
relationship: variable_of CO_343:0000147 ! tuber flesh color
relationship: variable_of CO_343:0003023 ! Tuber flesh color computation B value from chromameter machine
relationship: variable_of CO_343:0100227 ! unitless
created_by: Agre

[Term]
id: CO_343:0003023
name: Tuber flesh color computation B value from chromameter machine
namespace: YamMethod
def: "Compute the B value of the flesh surface color of tuber longitudinal section using chromameter machine" []
is_a: CO_343:1000013 ! Computation
relationship: variable_of CO_343:0000147 ! tuber flesh color

[Term]
id: CO_343:0003024
name: Yam tuber mealiness
namespace: YamTrait
def: "tuber mealiness traits" []
is_a: CO_343:1000007 ! Quality_trait

[Term]
id: CO_343:0003025
name: boiled tuber mealiness estimation
namespace: YamMethod
def: "The Mealiness of the boiled tuber is evaluated by a group of an individual using a (1 - 3 scale) as 1=soggy, 2= slightly mealy, 3= mealy" []
is_a: CO_343:1000014 ! Estimation
relationship: method_of boiled_tuber_mealiness_estimation_1-3_scale

[Term]
id: CO_343:0003026
name: boiled tuber mealiness estimation 1-3 scale
namespace: YamTrait
def: "The Mealiness of the boiled tuber is evaluated by a group of an individual using a (1 - 3 scale) as 1=soggy, 2= slightly mealy, 3= mealy." []
is_a: CO_343:1000003 ! Variable
relationship: variable_of CO_343:0003024 ! Yam tuber mealiness
relationship: variable_of CO_343:0010145 ! corm size-estimation
relationship: variable_of CO_343:0100011 ! 1-3 general scale

[Term]
id: CO_343:0003027
name: boiled tuber flesh texture estimation 1-3
namespace: YamTrait
def: "The texture of the boiled tuber is evaluated by a panel of individuals using (1-3 scale): Texture 1= strong; 2= intermediate; 3= soft" []
is_a: CO_343:1000003 ! Variable
relationship: variable_of CO_343:0000439 ! tuber flesh texture
relationship: variable_of CO_343:0010155 ! tuber flesh texture-estimation
relationship: variable_of CO_343:0100022 ! 1-3 scale

[Term]
id: CO_343:0003028
name: Boiled tuber color preference evaluation 1-5 scale
namespace: YamTrait
def: "The colour of the boiled yam is evaluated using a 1-5 scale: 1= Dislike extremely; 2=Dislike; 3=Neither like nor dislike; 4=Like; 5=Like extremely." []
is_a: CO_343:1000003 ! Variable
relationship: variable_of CO_343:0000147 ! tuber flesh color
relationship: variable_of CO_343:0003029 ! boiled tuber flesh color - estimation
relationship: variable_of CO_343:0100008 ! 1-5 scale

[Term]
id: CO_343:0003029
name: boiled tuber flesh color - estimation
namespace: YamMethod
def: "the colour of the boiled yam - visual evaluation" []
is_a: CO_343:1000014 ! Estimation
relationship: method_of CO_343:0000147 ! tuber flesh color

[Term]
id: CO_343:0010000
name: tubers (seed yams or setts) planted - counting
namespace: YamMethod
def: "Count the number of tubers (seed yams or setts) planted per plot (unit area)" []
is_a: CO_343:1000012 ! Counting
relationship: method_of CO_343:0000054 ! tubers planted

[Term]
id: CO_343:0010001
name: setts or seed yams planted weight - computation
namespace: YamMethod
def: "Measure the weight of N planted tubers (seed yams or setts) and record the average" []
is_a: CO_343:1000013 ! Computation
relationship: method_of CO_343:0000057 ! weight of planted tubers

[Term]
id: CO_343:0010002
name: time first sprout emergence-estimation
namespace: YamMethod
def: "Record date of first spout emergence in a plot" []
is_a: CO_343:1000014 ! Estimation
relationship: method_of CO_343:0000198 ! first sprout emergence time

[Term]
id: CO_343:0010003
name: time 50% of sprout emergence-estimation
namespace: YamMethod
def: "Record date 50% of sprouts in a plot emerged" []
is_a: CO_343:1000014 ! Estimation
relationship: method_of CO_343:0000200 ! 50% sprout emergence time

[Term]
id: CO_343:0010004
name: times to first sprout emergence-computation
namespace: YamMethod
def: "Compute the number of days required from date of planting to the date first sprout or plant in a plot or unit area emerged" []
is_a: CO_343:1000013 ! Computation
relationship: method_of CO_343:0000198 ! first sprout emergence time

[Term]
id: CO_343:0010005
name: times to 50% spout emergence-computation
namespace: YamMethod
def: "Compute the number of days required from date of planting to the date 50% of sprouts or plants in a plot emerged" []
is_a: CO_343:1000013 ! Computation
relationship: method_of CO_343:0000200 ! 50% sprout emergence time

[Term]
id: CO_343:0010006
name: emerged sprouts -counting
namespace: YamMethod
def: "Count the emerged plants (sprouts) per plot every week starting from first plant/sprout emergence date till the last plant or spourt emerge in a plot" []
is_a: CO_343:1000012 ! Counting
relationship: method_of CO_343:0000204 ! number of emerged plants

[Term]
id: CO_343:0010007
name: emerged sprouts or plants proportion-computation
namespace: YamMethod
def: "Compute the proportion or ratio of plants/sprouts emerged as the number of emerged plants/sprouts divided by the total number of tubers (seed yam or setts) planted in a plot multiplied by 100" []
is_a: CO_343:1000013 ! Computation
relationship: method_of CO_343:0000066 ! proportion of emerged plants

[Term]
id: CO_343:0010008
name: number of well established plants -counting
namespace: yamMethod
def: "Take count of well established plants in a plot usually at two months after planting" []
is_a: CO_343:1000012 ! Counting
relationship: method_of CO_343:0000207 ! established plants

[Term]
id: CO_343:0010009
name: field establishment-computation
namespace: YamMethod
def: "Compute the proportion or ratio of well-established plants in a plot from the total number of tubers (seed yam or setts) planted" []
is_a: CO_343:1000013 ! Computation
relationship: method_of CO_343:0000069 ! proportion of established plants

[Term]
id: CO_343:0010010
name: secondary sprouting - estimation
namespace: YamMethod
def: "Record emergence of new secondary sprouts from the planted seed tuber/sett in a plot at three months after planting" []
is_a: CO_343:1000014 ! Estimation
relationship: method_of CO_343:0000087 ! secondary sprouting

[Term]
id: CO_343:0010011
name: sprout color - estimation
namespace: YamMethod
def: "Record the predominant color of the sprouts (plant) per plot at 20 days after emergence" []
is_a: CO_343:1000014 ! Estimation
relationship: method_of CO_343:0000063 ! sprout color

[Term]
id: CO_343:0010012
name: sprout length-computation
namespace: YamMethod
def: "Compute the average sprout length of five representative plants measurement taken in a plot" []
is_a: CO_343:1000013 ! Computation
relationship: method_of CO_343:0000212 ! sprout length

[Term]
id: CO_343:0010013
name: colored spots on spine base-estimation
namespace: YamMethod
def: "Record of the existance of colored spot at base of spines on a sprout (vine)" []
is_a: CO_343:1000014 ! Estimation
relationship: method_of CO_343:0000214 ! presence of spot on spine base

[Term]
id: CO_343:0010014
name: spines on sprout base-estimation
namespace: YamMethod
def: "Record absence or presence of spines on a sprout (vine)" []
is_a: CO_343:1000014 ! Estimation
relationship: method_of CO_343:0000216 ! spines on sprout presence

[Term]
id: CO_343:0010015
name: hairiness of sprout - estimation
namespace: YamMethod
def: "Record existance of hairs on a sprout (vine)" []
is_a: CO_343:1000014 ! Estimation
relationship: method_of CO_343:0000218 ! sprout hairiness

[Term]
id: CO_343:0010016
name: time of  first leaf emergence on sprouted shoot (vines)-estimation
namespace: YamMethod
def: "Record time of the first leaf emergence on sprouted shoot (vine)" []
is_a: CO_343:1000014 ! Estimation
relationship: method_of CO_343:0000220 ! time to first leaf emergence

[Term]
id: CO_343:0010017
name: times to the first leaf emergence on sprouted shoot (vines)-computation
namespace: YamMethod
def: "Compute the number of days required from first sprout emergence to the first leaf to emerge on a sprouted shoot (vine) in a plot" []
is_a: CO_343:1000013 ! Computation
relationship: method_of CO_343:0000220 ! time to first leaf emergence

[Term]
id: CO_343:0010018
name: leaf apex shape-estimation
namespace: YamMethod
def: "Record leaf apex shape of mature plants in a plot" []
is_a: CO_343:1000014 ! Estimation
relationship: method_of CO_343:0000223 ! leaf apex shape

[Term]
id: CO_343:0010019
name: leaf shape-estimation
namespace: YamMethod
def: "Record leaf shape of mature plants in a plot" []
is_a: CO_343:1000014 ! Estimation
relationship: method_of CO_343:0000225 ! leaf shape

[Term]
id: CO_343:0010020
name: number of stems per plant-computation
namespace: YamMethod
def: "Compute average of the number of stems (vines) per established plants in a plot" []
is_a: CO_343:1000013 ! Computation
relationship: method_of CO_343:0000072 ! stems per plant

[Term]
id: CO_343:0010021
name: stem diameter-computation
namespace: YamMethod
def: "Measure the stem diameter at 15 cm above the base of five plants before senescence in a plot and record the average" []
is_a: CO_343:1000013 ! Computation
relationship: method_of CO_343:0000228 ! stem diameter

[Term]
id: CO_343:0010022
name: internode length -computation
namespace: YamMethod
def: "Measure the internode length of five plants before senescence at 1 meter height and record the average" []
is_a: CO_343:1000013 ! Computation
relationship: method_of CO_343:0000230 ! internode length

[Term]
id: CO_343:0010023
name: number of internode-computation
namespace: YamMethod
def: "Compute average number of internodes to first branching of at least five plants internode counts taken in a plot" []
is_a: CO_343:1000013 ! Computation
relationship: method_of CO_343:0000232 ! number of internodes to first branching

[Term]
id: CO_343:0010024
name: density of spines on stem base of a plant-etimation
namespace: YamMethod
def: "Visual assessment of spines on a stem (vine) above the base of mature plants in a plot" []
is_a: CO_343:1000014 ! Estimation
relationship: method_of CO_343:0000234 ! spines on stem density

[Term]
id: CO_343:0010025
name: plant type-estimation
namespace: YamMethod
def: "Visual assessment of the tendency of a plant to grow in a certain shape and to attain mature height and spread" []
is_a: CO_343:1000014 ! Estimation
relationship: method_of CO_343:0000236 ! plant type

[Term]
id: CO_343:0010026
name: canopy architecture - estimation
namespace: YamMethod
def: "Determination of predominant canopy architecture" []
is_a: CO_343:1000014 ! Estimation
relationship: method_of CO_343:0000030 ! canopy architecture

[Term]
id: CO_343:0010027
name: plant vigor - estimation
namespace: YamMethod
def: "Visual assessment of the plant vigour in a plot at two month after planting" []
is_a: CO_343:1000014 ! Estimation
relationship: method_of CO_343:0000060 ! plant vigor

[Term]
id: CO_343:0010028
name: twining habit-estimation
namespace: YamMethod
def: "Record the tendency of vine to twine or climb" []
is_a: CO_343:1000014 ! Estimation
relationship: method_of CO_343:0000240 ! twining habit

[Term]
id: CO_343:0010029
name: twining direction-estimation
namespace: yamMethod
def: "Record the twining or climbing direction of the vine" []
is_a: CO_343:1000014 ! Estimation
relationship: method_of CO_343:0000242 ! twining direction

[Term]
id: CO_343:0010030
name: flower initaition time - estimation
namespace: YamMethod
def: "Record time (date) of first flower initiation in a plot or the date any of the plants in a plot shows the first flower" []
is_a: CO_343:1000014 ! Estimation
relationship: method_of CO_343:0000090 ! time to flower initiation

[Term]
id: CO_343:0010031
name: 50% flowering time - estimation
namespace: YamMethod
def: "Record time (date) 50% plants in a plot are having at least one flower/inflorescence" []
is_a: CO_343:1000014 ! Estimation
relationship: method_of CO_343:0000245 ! time to 50% flowering

[Term]
id: CO_343:0010032
name: end of flowering time - estimation
namespace: YamMethod
def: "Record time (date) when the plant does not produce more new flowers in  a plot" []
is_a: CO_343:1000014 ! Estimation
relationship: method_of CO_343:0000247 ! time to end of flowering

[Term]
id: CO_343:0010033
name: flower initaition time - computation
namespace: YamMethod
def: "Computing the number of days required from first sprout emergence to first flower initiation" []
is_a: CO_343:1000013 ! Computation
relationship: method_of CO_343:0000090 ! time to flower initiation

[Term]
id: CO_343:0010034
name: 50% flowering time - computation
namespace: YamMethod
def: "Compute the number of days required from 50% of sprouts in plot emerged to 50% of plants in a plot are having at least one flower/inflorescence" []
is_a: CO_343:1000013 ! Computation
relationship: method_of CO_343:0000245 ! time to 50% flowering

[Term]
id: CO_343:0010035
name: end of flowering time - computation
namespace: YamMethod
def: "Computing the number of days required from 50% of sprout emergence to when plant does not produce more new flowers." []
is_a: CO_343:1000013 ! Computation
relationship: method_of CO_343:0000247 ! time to end of flowering

[Term]
id: CO_343:0010036
name: date crossing-estimation
namespace: YamMethod
def: "Record the date crossing made in particular flower of a plant." []
is_a: CO_343:1000014 ! Estimation
relationship: method_of CO_343:0000252 ! crossing date

[Term]
id: CO_343:0010037
name: floret pollinated number - counting
namespace: YamMethod
def: "Count the number of pollinated florets per female parent per cross" []
is_a: CO_343:1000012 ! Counting
relationship: method_of CO_343:0000000 ! pollinated florets number

[Term]
id: CO_343:0010038
name: pollinated spike number - estimation
namespace: YamMethod
def: "Count the number of pollinated spikes per female parent per cross" []
is_a: CO_343:1000012 ! Counting
relationship: method_of CO_343:0000003 ! pollinated spikes number

[Term]
id: CO_343:0010039
name: flowering intensity - estimation
namespace: YamMethod
def: "Record the abundance or intesity of flowering when more than 50% of the plants are flowered in a plot" []
is_a: CO_343:1000014 ! Estimation
relationship: method_of CO_343:0000096 ! flowering intensity

[Term]
id: CO_343:0010040
name: first inflorescence time - estimation
namespace: YamMethod
def: "Record date when plant/s having the first inflorescence in a plot" []
is_a: CO_343:1000014 ! Estimation
relationship: method_of CO_343:0000257 ! inflorescence initiation time

[Term]
id: CO_343:0010041
name: first inflorescence time - compuation
namespace: YamMethod
def: "Compute the number of days required to first inflorescence emergence in a plot" []
is_a: CO_343:1000013 ! Computation
relationship: method_of CO_343:0000257 ! inflorescence initiation time

[Term]
id: CO_343:0010042
name: inflorescence type-estimation
namespace: YamMethod
def: "Observe the type of inflorescence and score it" []
is_a: CO_343:1000014 ! Estimation
relationship: method_of CO_343:0000260 ! inflorescence type

[Term]
id: CO_343:0010043
name: femal flowers abundance or intensity per inflorescence-estimation
namespace: YamMethod
def: "Observe the femal flowering intensity or abudance per inflorences and rate" []
is_a: CO_343:1000014 ! Estimation
relationship: method_of CO_343:0000262 ! female flowering intensity

[Term]
id: CO_343:0010044
name: pollination type-estimation
namespace: YamMethod
def: "Record the method used to transfer the pollen grains from the anther of a flower to the stigma of a flower of the same or different plant of the same species" []
is_a: CO_343:1000014 ! Estimation
relationship: method_of CO_343:0000264 ! pollination type

[Term]
id: CO_343:0010045
name: plant or flower sex-estimation
namespace: YamMethod
def: "Scoring the most frequent flower sex type when more than 50% of the plants are flowered" []
is_a: CO_343:1000014 ! Estimation
relationship: method_of CO_343:0000093 ! plant sex

[Term]
id: CO_343:0010046
name: fruits developed number - counting
namespace: YamMethod
def: "Record the number of developed fruits or fruit set in pollinated flowers/inflorescence" []
is_a: CO_343:1000012 ! Counting
relationship: method_of CO_343:0000006 ! fruit developed number

[Term]
id: CO_343:0010047
name: 50% fruit set time-estimation
namespace: YamMethod
def: "Record the date fruit set in 50% of plants in a plot" []
is_a: CO_343:1000014 ! Estimation
relationship: method_of CO_343:0000268 ! time to fruit setting

[Term]
id: CO_343:0010048
name: ability to set or form fruts-estimation
namespace: YamMethod
def: "Observe fruit setting or formation of female flowers of monoeciouse and dieciouse plants and rate the ability set for form fruits" []
is_a: CO_343:1000014 ! Estimation
relationship: method_of CO_343:0000268 ! time to fruit setting

[Term]
id: CO_343:0010049
name: fruits harvested number - counting
namespace: YamMethod
def: "Record the number of harvested fruits per cross" []
is_a: CO_343:1000012 ! Counting
relationship: method_of CO_343:0000009 ! fruits harvested number

[Term]
id: CO_343:0010050
name: fruit harvesting time- estimation
namespace: YamMethod
def: "Record the date of fruits harvest in a crossing block or from plant" []
is_a: CO_343:1000014 ! Estimation
relationship: method_of CO_343:0000272 ! time to fruit harvesting

[Term]
id: CO_343:0010051
name: fruit maturity time - estimation
namespace: YamMethod
def: "Record the date 90% of the developed fruits shows sign of physiological maturity (turning brown)" []
is_a: CO_343:1000014 ! Estimation
relationship: method_of CO_343:0000274 ! time to fruit maturity

[Term]
id: CO_343:0010052
name: fruit maturity time - computation
namespace: YamMethod
def: "Compute the number of days required from fruit set to fruit phyisological maturity" []
is_a: CO_343:1000013 ! Computation
relationship: method_of CO_343:0000274 ! time to fruit maturity

[Term]
id: CO_343:0010053
name: fruit set number - estimation
namespace: YamMethod
def: "Assess the fruit number as fruiting intensity in categorical scale when more than 50% of the plants set fruits" []
is_a: CO_343:1000014 ! Estimation
relationship: method_of CO_343:0000099 ! fruit set number

[Term]
id: CO_343:0010054
name: fruit set number - computation
namespace: YamMethod
def: "Compute the fruit set number as proportion of pollinated flowers developing or setting a fruit and expressed in %" []
is_a: CO_343:1000013 ! Computation
relationship: method_of CO_343:0000099 ! fruit set number

[Term]
id: CO_343:0010055
name: fruit development intensity-estimation
namespace: YamMethod
def: "Score the degree of fruit development in scale" []
is_a: CO_343:1000014 ! Estimation
relationship: method_of CO_343:0000279 ! status of fruit development

[Term]
id: CO_343:0010056
name: seeds set - comp
namespace: YamMethod
def: "Take count of the number of seeds set on each fruits and record the average seeds per fruit" []
is_a: CO_343:1000013 ! Computation
relationship: method_of CO_343:0000180 ! seeds set per fruit

[Term]
id: CO_343:0010057
name: quantity of true seed harvested -counting
namespace: YamMethod
def: "Record the total number of true seed or botanical seed harvested or obtained per cross or family" []
is_a: CO_343:1000012 ! Counting
relationship: method_of CO_343:0000282 ! true seeds harvested

[Term]
id: CO_343:0010058
name: fruit index
namespace: YamMethod
def: "Compute the ratio of pollinated florets developing mature fruits" []
is_a: CO_343:1000013 ! Computation
relationship: method_of CO_343:0000284 ! fruit index

[Term]
id: CO_343:0010059
name: seed index
namespace: YamMethod
def: "Compute the ratio of pollinated florets developing seeds" []
is_a: CO_343:1000013 ! Computation
relationship: method_of CO_343:0000286 ! seed index

[Term]
id: CO_343:0010060
name: number of true seeds sown-counting
namespace: YamMethod
def: "Record the number of true seeds sown per cross or family" []
is_a: CO_343:1000012 ! Counting
relationship: method_of CO_343:0000288 ! seeds sown

[Term]
id: CO_343:0010061
name: time of first seed germination-estimation
namespace: YamMethod
def: "Record date the first seed germination observed per cross or family" []
is_a: CO_343:1000014 ! Estimation
relationship: method_of CO_343:0000290 ! seeds germination start time

[Term]
id: CO_343:0010062
name: date end of seed germination-estimation
namespace: YamMethod
def: "Record date the last seed germination observed per cross or family" []
is_a: CO_343:1000014 ! Estimation
relationship: method_of CO_343:0000292 ! seeds germination end time

[Term]
id: CO_343:0010063
name: germination rate - computation
namespace: YamMethod
def: "Compute the proportion of sown true or botanical seed which germinate and produce seedling ready for transplant , usually observed at three weeks after sowing." []
is_a: CO_343:1000013 ! Computation
relationship: method_of CO_343:0000012 ! seed germination rate

[Term]
id: CO_343:0010064
name: number of germinated seedling-counting
namespace: YamMethod
def: "Record the number of germinated seedlings per cross or family" []
is_a: CO_343:1000012 ! Counting
relationship: method_of CO_343:0000295 ! seeds germinated

[Term]
id: CO_343:0010065
name: seedling establishment rate-computation
namespace: YamMethod
def: "compute the proportion of seedlings per family (cross) establish well and ready for transplanting, usually recorded at five weeks after sowing." []
is_a: CO_343:1000013 ! Computation
relationship: method_of CO_343:0000015 ! seedling establishment rate

[Term]
id: CO_343:0010066
name: seedling tranplant survival rate-computation
namespace: YamMethod
def: "Compute the proportion of seedlings survived or established well after transplant operation" []
is_a: CO_343:1000013 ! Computation
relationship: method_of CO_343:0000298 ! seedling transplant survival rate

[Term]
id: CO_343:0010067
name: vine cuttings planted -counting
namespace: YamMethod
def: "Count the numeber vine cuttings planted" []
is_a: CO_343:1000012 ! Counting
relationship: method_of CO_343:0000300 ! vine cuttings planted

[Term]
id: CO_343:0010068
name: vines established-computation
namespace: YamMethod
def: "Compute the proportion or ratio of vines cuttings survive and producing shoots from the total of planted vine cuttings" []
is_a: CO_343:1000013 ! Computation
relationship: method_of CO_343:0000302 ! vine cutting establishment rate

[Term]
id: CO_343:0010069
name: time to 50% foliage senescence time - estimation
namespace: YamMethod
def: "Record date of 50% plants in a plot are showing foliage senescence" []
is_a: CO_343:1000014 ! Estimation
relationship: method_of CO_343:0000304 ! time to 50% foliage senescence

[Term]
id: CO_343:0010070
name: foliage senescence time - estimation
namespace: YamMethod
def: "Record the date when all plants in a plot shows a sign of 100%  foliage senescence" []
is_a: CO_343:1000014 ! Estimation
relationship: method_of CO_343:0000111 ! foliage senescence time

[Term]
id: CO_343:0010071
name: time to 50% foliage senescence time - computation
namespace: YamMethod
def: "Compute the number of days required for 50% of the plants in a plot showing foliage senescence" []
is_a: CO_343:1000013 ! Computation
relationship: method_of CO_343:0000304 ! time to 50% foliage senescence

[Term]
id: CO_343:0010072
name: foliage senescence time - computation
namespace: YamMethod
def: "Compute the number of days required from sprout emergence or planting to when all plants had fully senesced" []
is_a: CO_343:1000013 ! Computation
relationship: method_of CO_343:0000111 ! foliage senescence time

[Term]
id: CO_343:0010073
name: growing degere days to maturity-estimation
namespace: YamMethod
def: "Compute number of growing degree days required from planting (or 50% emergence) to 50% foliage senescence or maturity." []
is_a: CO_343:1000013 ! Computation
relationship: method_of CO_343:0000310 ! time to maturity

[Term]
id: CO_343:0010074
name: maturity class - estimation
namespace: YamMethod
def: "Observe the status of foliage senescence (leaf or vine yellowing) of plants in plot at 6 month onward and rate the maturity status" []
is_a: CO_343:1000014 ! Estimation
relationship: method_of CO_343:0000312 ! senescenece class

[Term]
id: CO_343:0010075
name: dry rot presence on harvested tubers-estimation
namespace: YamMethod
def: "Observe the occurance or presence of dry rot caused by nematods (Scutellonema bradys and Practylenchus spp.) on harvested tubers and record the presence and absence" []
is_a: CO_343:1000014 ! Estimation
relationship: method_of CO_343:0000314 ! yam tuber dry rot presence

[Term]
id: CO_343:0010076
name: dry rot tuber number-counting
namespace: yamMethod
def: "Take count of dry rot tubers per plot at harvest" []
is_a: CO_343:1000012 ! Counting
relationship: method_of CO_343:0000042 ! yam tuber dry rot incidence

[Term]
id: CO_343:0010077
name: tuber dry rot incidence - computation
namespace: YamMethod
def: "Compute the proportion dry rot tubers from the total number of harvested tubers per effective plot" []
is_a: CO_343:1000013 ! Computation
relationship: method_of CO_343:0000042 ! yam tuber dry rot incidence

[Term]
id: CO_343:0010078
name: tuber dry rot severity - estimation
namespace: YamMethod
def: "Score the severity of dry rot in harvested tubers" []
is_a: CO_343:1000014 ! Estimation
relationship: method_of CO_343:0000045 ! yam tuber dry rot severity

[Term]
id: CO_343:0010079
name: leaf beetle incidence - computation
namespace: YamMethod
def: "Compute the proportion of plants with leaf beetle damage from the total number of plants in the effective plots on leaf beetle damange record taken twice(at two and five months after planting date)" []
is_a: CO_343:1000013 ! Computation
relationship: method_of CO_343:0000153 ! leaf beetle damage incidence

[Term]
id: CO_343:0010080
name: leaf beetle severity - estimation
namespace: YamMethod
def: "Assess the leaf beetle infestation at two and five months after planting and record its severity" []
is_a: CO_343:1000014 ! Estimation
relationship: method_of CO_343:0000156 ! leaf beetle damage severity

[Term]
id: CO_343:0010081
name: mealybug tuber incidence - computation
namespace: YamMethod
def: "Compute the proportion tubers infested with mealybugs from the total number of harvested tubers per effective plot at time of harvesting." []
is_a: CO_343:1000013 ! Computation
relationship: method_of CO_343:0000159 ! mealybug tuber infestation incidence

[Term]
id: CO_343:0010082
name: mealybug tuber severity - estimation
namespace: YamMethod
def: "Mealybug tuber severity estimation on infested tubers at time harvesting" []
is_a: CO_343:1000014 ! Estimation
relationship: method_of CO_343:0000162 ! mealybug tuber infestation severity

[Term]
id: CO_343:0010083
name: root knot nematode incidence - computation
namespace: YamMethod
def: "Compute the proportion tubers showing root knot nematode symptoms from the total number of harvested tubers in effective plot" []
is_a: CO_343:1000013 ! Computation
relationship: method_of CO_343:0000048 ! root knot nematode incidence

[Term]
id: CO_343:0010084
name: root knot nematode severity - estimation
namespace: YamMethod
def: "Root knot nematode severity estimation in a range from no symptoms to highly severe galling scored in secondary roots of the plant and tubers adventitious roots." []
is_a: CO_343:1000014 ! Estimation
relationship: method_of CO_343:0000051 ! root knot nematode severity

[Term]
id: CO_343:0010085
name: tuber beetle incidence - computation
namespace: YamMethod
def: "Compute the proportion tubers with tuber's beetle damage from the total number of harvested tubers in the effective plot at harvesting time." []
is_a: CO_343:1000013 ! Computation
relationship: method_of CO_343:0000165 ! tuber beetle incidence

[Term]
id: CO_343:0010086
name: tuber beetle severity - estimation
namespace: YamMethod
def: "Tuber beetle severity or intensity estimated usually as number of nymph present in tubers at harvesting time." []
is_a: CO_343:1000014 ! Estimation
relationship: method_of CO_343:0000168 ! tuber beetle severity

[Term]
id: CO_343:0010087
name: viruses infection incidence - computation
namespace: YamMethod
def: "Compute the proportion of virus symptomatic individuals or their parts or commonly the portion of plant units in a plot. Take virus incidence recording thrice: First inspection at 8 to 10 weeks after planting and second inspection after 4 to 6 weeks after first inspection for virus symptoms and the third and final inspection 4 to 6 weeks after the second inspection ." []
is_a: CO_343:1000013 ! Computation
relationship: method_of CO_343:0000081 ! virus incidence

[Term]
id: CO_343:0010088
name: viruses infection severity - estimation
namespace: YamMethod
def: "Observe relative or absolute area of plant tissue affected by virus disease and record the severity as a proportion or percentage of plant surface affected using visual five ordinal scale . Predominant severity per plot must be registered at least thrice : 8 to 10 weeks after planting; 4 to 6 weeks after first scoring and the last scoring at 4 to 6 weeks after the second scoring" []
is_a: CO_343:1000014 ! Estimation
relationship: method_of CO_343:0000084 ! virus severity

[Term]
id: CO_343:0010089
name: anthracnose incidence - estimation
namespace: YamMethod
def: "Compute the proportion of anthracnose damaged individuals or their parts ; commonly the portion of plant units in a plot. Count anthracnose disease ‘blight’ or '' leaf spot'' affected plants in plot twice (First inspection at 10 to 12 weeks post planting and second inspection after 2 to 4 weeks before harvesting ) and compute the proportion of damanged" []
is_a: CO_343:1000013 ! Computation
relationship: method_of CO_343:0000075 ! yam anthracnose disease incidence

[Term]
id: CO_343:0010090
name: anthracnose severity - estimation
namespace: YamMethod
def: "Observe relative or absolute area of plant tissue affected by yam anthracnose disease and record the severity as a proportion or percentage of plant surface affected.It is visual score in scale under screenhouse, artificial inoculation or under field natural infestation. For artificial inoculation use a suspension of three most virulent strains of Colletothrichum gloeosporioides and inoculate the plants raised from vine cutting in vertical sack or other means by spraying. For natural infestation, scores can be taken 10 to 12 weeks after planting and second scoring about 4-6 weeks before harvesting . Artificial inoculation should be scored at 3 days after inoculation(DAI) , and repeated at 7DAI, 11DAI and 15DAI" []
is_a: CO_343:1000014 ! Estimation
relationship: method_of CO_343:0000021 ! yam anthracnose disease severity

[Term]
id: CO_343:0010091
name: number of bulbil - counting
namespace: YamMethod
def: "Count the number of aerial tubers or vine bulbils produced per net plot." []
is_a: CO_343:1000012 ! Counting
relationship: method_of CO_343:0000117 ! number of bulbil

[Term]
id: CO_343:0010092
name: number of bulbil - computation
namespace: YamMethod
def: "Count number of aerial tubers or vine bulbils on plants in a net plot and compute the average number bulbils per plant" []
is_a: CO_343:1000013 ! Computation
relationship: method_of CO_343:0000117 ! number of bulbil

[Term]
id: CO_343:0010093
name: bulbil shape-estimation
namespace: YamMethod
def: "Record shape of bulbils or aerial tubers in scale" []
is_a: CO_343:1000014 ! Estimation
relationship: method_of CO_343:0000335 ! bulbil shape

[Term]
id: CO_343:0010094
name: bulbil yield (plot weight) - measurement
namespace: YamMethod
def: "Record the fresh weight of harvested bulbil or aerial tuber per net plot" []
is_a: CO_343:1000011 ! Measurement
relationship: method_of CO_343:0000337 ! bulbil weight

[Term]
id: CO_343:0010095
name: bulbil yield (fresh weight) per plant-computation
namespace: YamMethod
def: "Compute the weight to harvested bulbils per plant" []
is_a: CO_343:1000013 ! Computation
relationship: method_of CO_343:0000120 ! bulbil yield

[Term]
id: CO_343:0010096
name: bulbil yield (fresh weight) per hectar- computation
namespace: YamMethod
def: "Computed the yield of bulbil per hectare using the formula." []
is_a: CO_343:1000013 ! Computation
relationship: method_of CO_343:0000120 ! bulbil yield

[Term]
id: CO_343:0010097
name: bulbil initiaition time - estimation
namespace: YamMethod
def: "Record date when 50% of plants in a plot begin producing bulbils or aerial tubers" []
is_a: CO_343:1000014 ! Estimation
relationship: method_of CO_343:0000108 ! time to bulbil initiation

[Term]
id: CO_343:0010098
name: bulbil initiation time - computation
namespace: YamMethod
def: "Compute number of days required from sprout emergence to 50% of plants in a plot start forming bulbils or aerial tubers" []
is_a: CO_343:1000013 ! Computation
relationship: method_of CO_343:0000108 ! time to bulbil initiation

[Term]
id: CO_343:0010099
name: presence of bulbil  - estimation
namespace: YamMethod
def: "Record the presence and absence of bulbils (aerial tubers) in the vines of yam plant" []
is_a: CO_343:1000014 ! Estimation
relationship: method_of CO_343:0000105 ! presence of bulbil

[Term]
id: CO_343:0010100
name: plant harvested number - counting
namespace: YamMethod
def: "Counting the number of plants where tubers were harvested in a plot" []
is_a: CO_343:1000012 ! Counting
relationship: method_of CO_343:0000123 ! stand harvested number

[Term]
id: CO_343:0010101
name: big size tubers harvested number - counting
namespace: YamMethod
def: "Count the number of tubers in a plot weighing ≥1 kg harvested per effective plot" []
is_a: CO_343:1000012 ! Counting
relationship: method_of CO_343:0000347 ! big size tubers per plot

[Term]
id: CO_343:0010102
name: medium size tubers harvested number- counting
namespace: YamMethod
def: "Count the number of tubers in a plot weighing ≥ 500 gm and <1 kg harvested per effective plot" []
is_a: CO_343:1000012 ! Counting
relationship: method_of CO_343:0000349 ! medium size tubers per plot

[Term]
id: CO_343:0010103
name: small size tubers harvested per plot number - counting
namespace: YamMethod
def: "Count the number of tubers in a plot weighing less than 500 gm harvested per effective plot" []
is_a: CO_343:1000012 ! Counting
relationship: method_of CO_343:0000351 ! small size tubers per plot

[Term]
id: CO_343:0010104
name: rotten tubers in a plot number-counting
namespace: YamMethod
def: "Count the number of rotten and/or diseased tubers in effective plot" []
is_a: CO_343:1000012 ! Counting
relationship: method_of CO_343:0000138 ! rotten or diseased tubers per plot

[Term]
id: CO_343:0010105
name: total tuber harvested number-computation
namespace: YamMethod
def: "Compute the sum of all category/size tubers (big, medium, small and rotten/diseased) in a net plot" []
is_a: CO_343:1000013 ! Computation
relationship: method_of CO_343:0000126 ! total tubers per plot

[Term]
id: CO_343:0010106
name: big size tubers per plant-computation
namespace: YamMethod
def: "Compute the number of big size tubers produced per plant using the formula number of big size tuber in a plot divided by the total number of harvested plants" []
is_a: CO_343:1000013 ! Computation
relationship: method_of CO_343:0000355 ! big size tubers per plant

[Term]
id: CO_343:0010107
name: medium size tubers per plant-computation
namespace: yamMethod
def: "Compute the number of medium size tubers produced per plant using the formula number of medium size tuber in a plot divided by the total number of harvested plants" []
is_a: CO_343:1000013 ! Computation
relationship: method_of CO_343:0000357 ! medium size tubers per plant

[Term]
id: CO_343:0010108
name: small size tubers per plant-computation
namespace: YamMethod
def: "Compute the number of small size tubers produced per plant using the formula number of small size tuber in a plot divided by the total number of harvested plants" []
is_a: CO_343:1000013 ! Computation
relationship: method_of CO_343:0000359 ! small size tubers per plant

[Term]
id: CO_343:0010109
name: total tubers per plant-computation
namespace: YamMethod
def: "Compute as the total number of tubers in a net plot divided by the number of harvested plant per net plot" []
is_a: CO_343:1000013 ! Computation
relationship: method_of CO_343:0000361 ! total tubers per plant

[Term]
id: CO_343:0010110
name: big size tubers fresh weight per plot- measurement
namespace: YamMethod
def: "Record the weight of big size ( ≥1 kg) tubers in a net plot" []
is_a: CO_343:1000011 ! Measurement
relationship: method_of CO_343:0000363 ! big size tubers weight per plot

[Term]
id: CO_343:0010111
name: medium size tubers fresh weight per plot -measurement
namespace: YamMethod
def: "Record the weight of medium size ( ≥ 500 gm and <1 kg) tubers in a net plot" []
is_a: CO_343:1000011 ! Measurement
relationship: method_of CO_343:0000365 ! medium size tubers weight per plot

[Term]
id: CO_343:0010112
name: small size tubers fresh weight per plot- measurement
namespace: YamMethod
def: "Record the weight of small size ( < 500 gm) tubers in a net plot" []
is_a: CO_343:1000011 ! Measurement
relationship: method_of CO_343:0000367 ! small size tubers weight per plot

[Term]
id: CO_343:0010113
name: rotten tuber fresh weight per plot - measurement
namespace: YamMethod
def: "Record weight of rotten and/or diseased tubers harvested in a net plot" []
is_a: CO_343:1000011 ! Measurement
relationship: method_of CO_343:0000138 ! rotten or diseased tubers per plot

[Term]
id: CO_343:0010114
name: total tuber fresh weight per plot -computation
namespace: YamMethod
def: "Compute the sum all category or size of tubers (Big, medium, small size, and rotten and diseased) fresh weight per plot" []
is_a: CO_343:1000013 ! Computation
relationship: method_of CO_343:0000370 ! total fresh tuber weight per plot

[Term]
id: CO_343:0010115
name: total tuber fresh weight per plant-computation
namespace: YamMethod
def: "Compute by dividing fresh weight measurement of all categroy/size tubers taken in a plot to the number of harvested plant in a net plot" []
is_a: CO_343:1000013 ! Computation
relationship: method_of CO_343:0000372 ! total tuber weight per plant

[Term]
id: CO_343:0010116
name: big size yam fresh weight per plant- computation
namespace: YamMethod
def: "Compute by dividing fresh weight measurement of big size tubers taken to the number of harvested plants in a net plot" []
is_a: CO_343:1000013 ! Computation
relationship: method_of CO_343:0000374 ! big size tuber weight per plant

[Term]
id: CO_343:0010117
name: medium size yam fresh weight per plant-computation
namespace: yamMethod
def: "Compute by dividing fresh weight measurement of medium size tubers taken to the number of harvested plants in a net plot" []
is_a: CO_343:1000013 ! Computation
relationship: method_of CO_343:0000376 ! medium size tuber weight per plant

[Term]
id: CO_343:0010118
name: small size yam fresh weight per plant-computation
namespace: YamMethod
def: "Compute by dividing fresh weight measurement of small size tubers taken to the number of harvested plants in a net plot" []
is_a: CO_343:1000013 ! Computation
relationship: method_of CO_343:0000378 ! small size tuber weight per plant

[Term]
id: CO_343:0010119
name: tuber yield no adjusted- computation
namespace: YamMethod
def: "Computed as total tuber weight per plot divided by size of net or effective harvest plot and result multiplied by 10" []
is_a: CO_343:1000013 ! Computation
relationship: method_of CO_343:0000132 ! total tuber yield

[Term]
id: CO_343:0010120
name: big size yam yield no adjusted- computation
namespace: YamMethod
def: "Calculated as big size yam tuber weight per plot divided by size of effective harvest plot mutiplied by 10" []
is_a: CO_343:1000013 ! Computation
relationship: method_of CO_343:0000135 ! big size yam yield

[Term]
id: CO_343:0010121
name: total tuber yield adjusted-computation
namespace: YamMethod
def: "Computed as total tubers weight per plant multiplied by planting density and result divided by 1000" []
is_a: CO_343:1000013 ! Computation
relationship: method_of CO_343:0000382 ! total tuber yield adjusted

[Term]
id: CO_343:0010122
name: big size yam yield adjusted-computation
namespace: YamMethod
def: "Calculated as big size yam tuber weight per per plant mutiplied by planting density and result divided by 1000" []
is_a: CO_343:1000013 ! Computation
relationship: method_of CO_343:0000384 ! big size tuber yield adjusted

[Term]
id: CO_343:0010123
name: big yam tuber average weight-computation
namespace: YamMethod
def: "Calculated as weight of big size tubers per plot divided by total number of big size tubers per plot" []
is_a: CO_343:1000013 ! Computation
relationship: method_of CO_343:0000386 ! average weigth of big size tuber

[Term]
id: CO_343:0010124
name: average tuber weight -computation
namespace: YamMethod
def: "Calculated as total tuber weight per plot divided by total number of tubers per plot" []
is_a: CO_343:1000013 ! Computation
relationship: method_of CO_343:0000388 ! average tuber weight

[Term]
id: CO_343:0010125
name: position of root appearance on tubers-estimation
namespace: YamMethod
def: "Record position of appearance of roots at surface to tubers" []
is_a: CO_343:1000014 ! Estimation
relationship: method_of CO_343:0000390 ! place of roots on tubers

[Term]
id: CO_343:0010126
name: hairiness of tuber bark - estimation
namespace: YamMethod
def: "Record the intensity of tuber hairs or secondary roots on the surface of harvested tubers" []
is_a: CO_343:1000014 ! Estimation
relationship: method_of CO_343:0000183 ! tuber hairiness

[Term]
id: CO_343:0010127
name: tuber surface appearance - estimation
namespace: YamMethod
def: "Observe the appearance of roots, thones and srout buds on surface of harvested tubers and make visual score using scale" []
is_a: CO_343:1000014 ! Estimation
relationship: method_of CO_343:0000188 ! tuber appearance

[Term]
id: CO_343:0010128
name: tuber surface texture - estimation
namespace: YamMethod
def: "Record the smoothness or roughness of tuber skin in visual scale" []
is_a: CO_343:1000014 ! Estimation
relationship: method_of CO_343:0000141 ! tuber surface texture

[Term]
id: CO_343:0010129
name: tuber thorniness - estimation
namespace: YamMethod
def: "Record the presence or absence of thorns or spines on the tuber skin in visual scale" []
is_a: CO_343:1000014 ! Estimation
relationship: method_of CO_343:0000144 ! tuber thorniness

[Term]
id: CO_343:0010130
name: tuber thorniness intensity-estimation
namespace: YamMethod
def: "Record the degree of thorns or spines on tuber surface in visual scale" []
is_a: CO_343:1000014 ! Estimation
relationship: method_of CO_343:0000396 ! tuber thorniness intensity

[Term]
id: CO_343:0010131
name: length of big size tubers-computation
namespace: YamMethod
def: "Measure the length of at most five big size tubers (≥1kg) from base to tip in a net plot at harvest and record the average" []
is_a: CO_343:1000013 ! Computation
relationship: method_of CO_343:0000398 ! big size tuber length

[Term]
id: CO_343:0010132
name: length of medium size tubers-computation
namespace: YamMethod
def: "Measure the length of at most five medium size tubers (≥500 gm and <1kg ) from base to tip in a net plot at harvest and record the average" []
is_a: CO_343:1000013 ! Computation
relationship: method_of CO_343:0000400 ! medium size tuber length

[Term]
id: CO_343:0010133
name: length of small size tubers-computation
namespace: YamMethod
def: "Measure the length of at most five small size tubers (<500 gm) from base to tip in a net plot at harvest and record the average" []
is_a: CO_343:1000013 ! Computation
relationship: method_of CO_343:0000402 ! small size tuber length

[Term]
id: CO_343:0010134
name: tuber length-computation
namespace: YamMethod
def: "Compute average tuber length of all size tubers measurement taken in a net plot" []
is_a: CO_343:1000011 ! Measurement
relationship: method_of CO_343:0000404 ! tuber length

[Term]
id: CO_343:0010135
name: tuber shape - estimation
namespace: YamMethod
def: "Determination of the predominant shape in the entire family/plot as a unit" []
is_a: CO_343:1000014 ! Estimation
relationship: method_of CO_343:0000024 ! tuber shape

[Term]
id: CO_343:0010136
name: tuber size - estimation
namespace: YamMethod
def: "Determination of predominant size of the tuber in the entire family" []
is_a: CO_343:1000014 ! Estimation
relationship: method_of CO_343:0000027 ! tuber size

[Term]
id: CO_343:0010137
name: width of big size tubers-computation
namespace: YamMethod
def: "Measure the width of at most five big size tubers (≥1kg) from net plot at wider portion of the tuber using vernier calliper or measuring tape and record the average" []
is_a: CO_343:1000013 ! Computation
relationship: method_of CO_343:0000408 ! big size tuber width

[Term]
id: CO_343:0010138
name: width of medium size tubers-computation
namespace: YamMethod
def: "Measure the width of at most five medium size tubers (≥500 gm and <1kg )from net plot at wider portion of the tuber using calliper or measuring tape and record the average" []
is_a: CO_343:1000013 ! Computation
relationship: method_of CO_343:0000410 ! medium size tuber width

[Term]
id: CO_343:0010139
name: width of small size tubers-computation
namespace: YamMethod
def: "Measure the width of at most five small size tubers (<500 gm) from net plot at wider portion of the tuber using calliper or measuring tape and record the average" []
is_a: CO_343:1000013 ! Computation
relationship: method_of CO_343:0000412 ! small size tuber width

[Term]
id: CO_343:0010140
name: tuber wideth-computation
namespace: YamMethod
def: "Compute the average tuber width of all size measurement taken in a net plot" []
is_a: CO_343:1000013 ! Computation
relationship: method_of CO_343:0000414 ! tuber width

[Term]
id: CO_343:0010141
name: cracks on the tuber surface-estimation
namespace: YamMethod
def: "Record appearance of cracks on tuber surface as absent, few and many" []
is_a: CO_343:1000014 ! Estimation
relationship: method_of CO_343:0000416 ! tuber cracks

[Term]
id: CO_343:0010142
name: crazy roots presence on tubers at harvest-estimation
namespace: YamMethod
def: "Record appearance of crazy roots on tuber surface at harvest" []
is_a: CO_343:1000014 ! Estimation
relationship: method_of CO_343:0000418 ! crazy roots presence

[Term]
id: CO_343:0010143
name: corm on tubers-estimation
namespace: YamMethod
def: "Score corm status of tubers using a binary scale" []
is_a: CO_343:1000014 ! Estimation
relationship: method_of CO_343:0000420 ! corm on tuber

[Term]
id: CO_343:0010144
name: corm separation from tuber-estimation
namespace: YamMethod
def: "Record the corm ability to be separated from tuber in a binary scale" []
is_a: CO_343:1000014 ! Estimation
relationship: method_of CO_343:0000422 ! corm separability from tuber

[Term]
id: CO_343:0010145
name: corm size-estimation
namespace: YamMethod
def: "Record corm size in relation to tuber size using three scale" []
is_a: CO_343:1000014 ! Estimation
relationship: method_of CO_343:0000424 ! corm size

[Term]
id: CO_343:0010146
name: corm type-estimation
namespace: YamMethod
def: "Record the corm type as regular, transversally elongated or brached using scale" []
is_a: CO_343:1000014 ! Estimation
relationship: method_of CO_343:0000426 ! corm type

[Term]
id: CO_343:0010147
name: dormancy period -estimation
namespace: YamMethod
def: "Assess the proportion of sprouted tubers at different time interval (once a week) from harvesting up to three months after harvesting and rate the dormancy period in scale" []
is_a: CO_343:1000014 ! Estimation
relationship: method_of CO_343:0000036 ! tuber dormancy period

[Term]
id: CO_343:0010148
name: tuber dry matter content - computation
namespace: YamMethod
def: "Select at least five random whole tubers from a net plot and cut small slices (1-2 mm) from proximal, middle and distal portion and mixed thoroughly. Record fresh weight and determin dry weight of samples by drying at 70°C for 72 h in a forced air oven. A proportion between the dry weight and the fresh weight is calculated." []
is_a: CO_343:1000013 ! Computation
relationship: method_of CO_343:0000174 ! tuber dry matter content

[Term]
id: CO_343:0010149
name: tuber flesh color head portion - estimation
namespace: YamMethod
def: "Observe and record the fresh cut tuber flesh surface color at the head portion of the tuber at harvesting time." []
is_a: CO_343:1000014 ! Estimation
relationship: method_of CO_343:0000147 ! tuber flesh color

[Term]
id: CO_343:0010150
name: tuber flesh color middle portion - estimation
namespace: YamMethod
def: "Observe  and record the fresh cut flesh surface color at the middle part of the tuber at harvesting time." []
is_a: CO_343:1000014 ! Estimation
relationship: method_of CO_343:0000147 ! tuber flesh color

[Term]
id: CO_343:0010151
name: tuber flesh color lower or tail portion- estimation
namespace: YamMethod
def: "Observe and record fresh cut tuber flesh surface color at the tail portion of the tuber at harvesting time." []
is_a: CO_343:1000014 ! Estimation
relationship: method_of CO_343:0000147 ! tuber flesh color

[Term]
id: CO_343:0010152
name: tuber flesh color reading -measurement
namespace: yamMethod
def: "Measure the flesh surface color of tuber (head, middle and tail portion) at different time interval (0, 30, 60, 180 minutes after cutting) using colorimeter (a color spectrophotometer) or standard color chart." []
is_a: CO_343:1000011 ! Measurement
relationship: method_of CO_343:0000147 ! tuber flesh color

[Term]
id: CO_343:0010153
name: tuber flesh cross section color uniformity-estimation
namespace: yamMethod
def: "Record the uniformity of tuber flesh cross-section color using visual scale at fresh cut during harvest" []
is_a: CO_343:1000014 ! Estimation
relationship: method_of CO_343:0000435 ! tuber flesh cross-section color uniformity

[Term]
id: CO_343:0010154
name: tuber flesh oxidation intensity-estimation
namespace: yamMethod
def: "Score the intensity of tuber flesh oxidation (flesh surface color change) at different time interval (0, 30, 60, 180 minutes after cutting) using scale" []
is_a: CO_343:1000014 ! Estimation
relationship: method_of CO_343:0000437 ! tuber flesh oxidation intensity

[Term]
id: CO_343:0010155
name: tuber flesh texture-estimation
namespace: yamMethod
def: "Record the texture of tuber flesh using scale" []
is_a: CO_343:1000014 ! Estimation
relationship: method_of CO_343:0000439 ! tuber flesh texture

[Term]
id: CO_343:0010156
name: tuber oxidation-estimation
namespace: yamMethod
def: "Record time in minutes lasted for cut tuber flesh to become or not oxidized and score in scale" []
is_a: CO_343:1000014 ! Estimation
relationship: method_of CO_343:0000150 ! tuber flesh oxidation

[Term]
id: CO_343:0010157
name: tuber flesh oxidation color-estimation
namespace: yamMethod
def: "Record the flesh enzymatic oxidation color using color scale" []
is_a: CO_343:1000014 ! Estimation
relationship: method_of CO_343:0000442 ! tuber flesh oxidation color

[Term]
id: CO_343:0010158
name: cohesiveness of pounded yam- estimation
namespace: YamMethod
def: "Score the degree to which particles of a pounded yam stick together or how moldable it is using intensity scale" []
is_a: CO_343:1000014 ! Estimation
relationship: method_of CO_343:0000444 ! cohesiveness of pounded yam

[Term]
id: CO_343:0010159
name: springiness of pounded yam-estimation
namespace: YamMethod
def: "Score the distance to which the deformed material can be or degree of stretchabiliy pounded yam in intesity scale" []
is_a: CO_343:1000014 ! Estimation
relationship: method_of CO_343:0000446 ! springiness of pounded yam

[Term]
id: CO_343:0010160
name: smoothness of pounded yam- estimation
namespace: YamMethod
def: "score the smoothnessof the pounded yam , i.e., absence of lumps by finger feeling and using intensity scale" []
is_a: CO_343:1000014 ! Estimation
relationship: method_of CO_343:0000448 ! smoothness of pounded yam

[Term]
id: CO_343:0010161
name: presence of fiber strand-estimation
namespace: YamMethod
def: "Score the presence or absence of ﬁber strands on pounded yam" []
is_a: CO_343:1000014 ! Estimation
relationship: method_of CO_343:0000450 ! fibrousness of pounded yam

[Term]
id: CO_343:0010162
name: stickiness of pounded yam - estimation
namespace: YamMethod
def: "Score the sticknes or adhesiveness of pounded yam to consumern fingur using sensory test panelist" []
is_a: CO_343:1000014 ! Estimation
relationship: method_of CO_343:0000191 ! stickiness of pounded yam

[Term]
id: CO_343:0010163
name: taste of pounded yam - estimation
namespace: YamMethod
def: "Score taste of pounded yam using sensory test panalist" []
is_a: CO_343:1000014 ! Estimation
relationship: method_of CO_343:0000194 ! taste of pounded yam

[Term]
id: CO_343:0010164
name: scale insect infestation - estimation
namespace: YamMethod
def: "Observe and score scale insect infestation on tuber at harvest" []
is_a: CO_343:1000014 ! Estimation
relationship: method_of CO_343:0000454 ! scale insect infestation

[Term]
id: CO_343:0010165
name: stem color - estimation
namespace: YamMethod
def: "Record the predominant color of stem on mature plant at five to six month after emergence using a five color scale" []
is_a: CO_343:1000014 ! Estimation
relationship: method_of CO_343:0000456 ! stem color

[Term]
id: CO_343:0010166
name: leaf density - estimation
namespace: YamMethod
def: "Observe the leaf abundance or mass on a mature plant and rate the density" []
is_a: CO_343:1000014 ! Estimation
relationship: method_of CO_343:0000458 ! leaf density

[Term]
id: CO_343:0010167
name: number of branchs - computation
namespace: YamMethod
def: "Count the number of branches above ground on at least five mature plants in a plot and record the average" []
is_a: CO_343:1000012 ! Counting
relationship: method_of CO_343:0000460 ! branch number

[Term]
id: CO_343:0010168
name: stem height - computation
namespace: YamMethod
def: "Measure the length or height of stem or vine of at least five mature plants in a plot using measuring tape at five to six months after sprout emergence and record the average" []
is_a: CO_343:1000011 ! Measurement
relationship: method_of CO_343:0000462 ! stem height

[Term]
id: CO_343:0010169
name: number of leaves - computation
namespace: YamMethod
def: "Count the number of leaves on at least five young plants in a plot at 30 days after emergence and record the average" []
is_a: CO_343:1000013 ! Computation
relationship: method_of CO_343:0000464 ! number of leaves

[Term]
id: CO_343:0010170
name: leaf position - estimation
namespace: YamMethod
def: "Observe the arrangement of leaves on stem or vine and rate it" []
is_a: CO_343:1000014 ! Estimation
relationship: method_of CO_343:0000466 ! leaf position

[Term]
id: CO_343:0010171
name: leaf length - computation
namespace: YamMethod
def: "Measure the length from lobes to the tip using a measuring tape on sampled 20 adult leaves ( four leaves per plant and at leat five plants on a plot), and record the average length" []
is_a: CO_343:1000013 ! Computation
relationship: method_of CO_343:0000468 ! leaf length

[Term]
id: CO_343:0010172
name: leaf width - computation
namespace: YamMethod
def: "Measure the width from the widest part of leaf using a measuring tape on sampled 20 adult leaves ( four leaves per plant on at leat five plants in a plot), and record the average width" []
is_a: CO_343:1000013 ! Computation
relationship: method_of CO_343:0000470 ! leaf width

[Term]
id: CO_343:0010173
name: internode length - computation
namespace: YamMethod
def: "Measure the length of internode at 1m height on five (5) plants and record the average" []
is_a: CO_343:1000013 ! Computation
relationship: method_of CO_343:0000230 ! internode length

[Term]
id: CO_343:0010174
name: hair on stem - estimation
namespace: YamMethod
def: "Observe the presence or absence of hairs on stem surface" []
is_a: CO_343:1000014 ! Estimation
relationship: method_of CO_343:0000473 ! stem hairiness

[Term]
id: CO_343:0010175
name: leaf color - estimation
namespace: YamMethod
def: "Assess the color of leaf on a young plant" []
is_a: CO_343:1000014 ! Estimation
relationship: method_of CO_343:0000475 ! leaf color

[Term]
id: CO_343:0010176
name: vein color - estimation
namespace: YamMethod
def: "Assess the color of leaf vein on the upper surface" []
is_a: CO_343:1000014 ! Estimation
relationship: method_of CO_343:0000478 ! vein color

[Term]
id: CO_343:0010177
name: leaf hairiness - estimation
namespace: YamMethod
def: "Assess hairiness of leaf surface (upper part)" []
is_a: CO_343:1000014 ! Estimation
relationship: method_of CO_343:0000481 ! leaf hairiness

[Term]
id: CO_343:0010178
name: petiole length - computation
namespace: YamMethod
def: "Measure the length of petiole using measuring tape on sampled 20 adult leaves ( four leaves per plant on at leat five plants in a plot), and record the average length" []
is_a: CO_343:1000013 ! Computation
relationship: method_of CO_343:0000484 ! petiole length

[Term]
id: CO_343:0012000
name: peak viscosity - measurement
namespace: YamMethod
def: "water-holding capacity of the starch using RVA." []
is_a: CO_343:1000011 ! Measurement
relationship: method_of CO_343:0002000 ! peak viscosity

[Term]
id: CO_343:0012001
name: trough viscosity - measurement
namespace: YamMethod
def: "Measurement of teh ability of starch granules to remain undisrupted when the yam paste is subjected to a hold period of constant high temperature using RVA." []
is_a: CO_343:1000011 ! Measurement
relationship: method_of CO_343:0002001 ! trough viscosity

[Term]
id: CO_343:0012002
name: final viscosity - measurement
namespace: YamMethod
def: "Measurement of the ability of the material to form a viscous paste after cooking and cooling" []
is_a: CO_343:1000011 ! Measurement
relationship: method_of CO_343:0002002 ! final viscosity

[Term]
id: CO_343:0012003
name: breakdown - measurement
namespace: YamMethod
def: "Measurement of the resistance of the starch paste to heat and shear using RVA." []
is_a: CO_343:1000011 ! Measurement
relationship: method_of CO_343:0002003 ! breakdown

[Term]
id: CO_343:0012004
name: setback - measurement
namespace: YamMethod
def: "Measurement of the tendency of starch pastes to recrystallize and is an index of starch retrogradation or gelling ability using RVA" []
is_a: CO_343:1000011 ! Measurement
relationship: method_of CO_343:0002004 ! setback

[Term]
id: CO_343:0012005
name: pasting temperature - measurement
namespace: YamMethod
def: "Measurement of the onset of a rise in viscosity using RVA." []
is_a: CO_343:1000011 ! Measurement
relationship: method_of CO_343:0002005 ! pasting temperature

[Term]
id: CO_343:0100000
name: number of tubers
namespace: YamScale
is_a: CO_343:1000019 ! Numerical
relationship: scale_of CO_343:0010000 ! tubers (seed yams or setts) planted - counting

[Term]
id: CO_343:0100001
name: gm/sett
namespace: YamScale
is_a: CO_343:1000019 ! Numerical
relationship: scale_of CO_343:0010001 ! setts or seed yams planted weight - computation

[Term]
id: CO_343:0100002
name: date (yyyymmdd)
namespace: YamScale
is_a: CO_343:1000020 ! Time
relationship: scale_of CO_343:0010002 ! time first sprout emergence-estimation
relationship: scale_of CO_343:0010003 ! time 50% of sprout emergence-estimation
relationship: scale_of CO_343:0010016 ! time of  first leaf emergence on sprouted shoot (vines)-estimation
relationship: scale_of CO_343:0010030 ! flower initaition time - estimation
relationship: scale_of CO_343:0010031 ! 50% flowering time - estimation
relationship: scale_of CO_343:0010032 ! end of flowering time - estimation
relationship: scale_of CO_343:0010036 ! date crossing-estimation
relationship: scale_of CO_343:0010040 ! first inflorescence time - estimation
relationship: scale_of CO_343:0010047 ! 50% fruit set time-estimation
relationship: scale_of CO_343:0010050 ! fruit harvesting time- estimation
relationship: scale_of CO_343:0010051 ! fruit maturity time - estimation
relationship: scale_of CO_343:0010061 ! time of first seed germination-estimation
relationship: scale_of CO_343:0010062 ! date end of seed germination-estimation
relationship: scale_of CO_343:0010069 ! time to 50% foliage senescence time - estimation
relationship: scale_of CO_343:0010070 ! foliage senescence time - estimation
relationship: scale_of CO_343:0010097 ! bulbil initiaition time - estimation

[Term]
id: CO_343:0100003
name: days
namespace: YamScale
is_a: CO_343:1000018 ! Duration
relationship: scale_of CO_343:0010004 ! times to first sprout emergence-computation
relationship: scale_of CO_343:0010005 ! times to 50% spout emergence-computation
relationship: scale_of CO_343:0010017 ! times to the first leaf emergence on sprouted shoot (vines)-computation
relationship: scale_of CO_343:0010033 ! flower initaition time - computation
relationship: scale_of CO_343:0010034 ! 50% flowering time - computation
relationship: scale_of CO_343:0010035 ! end of flowering time - computation
relationship: scale_of CO_343:0010041 ! first inflorescence time - compuation
relationship: scale_of CO_343:0010052 ! fruit maturity time - computation
relationship: scale_of CO_343:0010071 ! time to 50% foliage senescence time - computation
relationship: scale_of CO_343:0010072 ! foliage senescence time - computation
relationship: scale_of CO_343:0010098 ! bulbil initiation time - computation

[Term]
id: CO_343:0100004
name: plants per plot
namespace: YamScale
is_a: CO_343:1000019 ! Numerical
relationship: scale_of CO_343:0010006 ! emerged sprouts -counting
relationship: scale_of CO_343:0010008 ! number of well established plants -counting

[Term]
id: CO_343:0100005
name: percentage
namespace: YamScale
is_a: CO_343:1000019 ! Numerical
relationship: scale_of CO_343:0010007 ! emerged sprouts or plants proportion-computation

[Term]
id: CO_343:0100006
name: %
namespace: YamScale
is_a: CO_343:1000019 ! Numerical
relationship: scale_of CO_343:0010009 ! field establishment-computation
relationship: scale_of CO_343:0010054 ! fruit set number - computation
relationship: scale_of CO_343:0010063 ! germination rate - computation
relationship: scale_of CO_343:0010065 ! seedling establishment rate-computation
relationship: scale_of CO_343:0010066 ! seedling tranplant survival rate-computation
relationship: scale_of CO_343:0010068 ! vines established-computation
relationship: scale_of CO_343:0010077 ! tuber dry rot incidence - computation
relationship: scale_of CO_343:0010079 ! leaf beetle incidence - computation
relationship: scale_of CO_343:0010081 ! mealybug tuber incidence - computation
relationship: scale_of CO_343:0010083 ! root knot nematode incidence - computation
relationship: scale_of CO_343:0010085 ! tuber beetle incidence - computation
relationship: scale_of CO_343:0010087 ! viruses infection incidence - computation
relationship: scale_of CO_343:0010089 ! anthracnose incidence - estimation
relationship: scale_of CO_343:0010148 ! tuber dry matter content - computation

[Term]
id: CO_343:0100007
name: 0-1 scale
namespace: YamScale
is_a: CO_343:1000017 ! Nominal
relationship: scale_of CO_343:0010010 ! secondary sprouting - estimation
relationship: scale_of CO_343:0010013 ! colored spots on spine base-estimation
relationship: scale_of CO_343:0010014 ! spines on sprout base-estimation
relationship: scale_of CO_343:0010048 ! ability to set or form fruts-estimation
relationship: scale_of CO_343:0010075 ! dry rot presence on harvested tubers-estimation
relationship: scale_of CO_343:0010099 ! presence of bulbil  - estimation
relationship: scale_of CO_343:0010153 ! tuber flesh cross section color uniformity-estimation

[Term]
id: CO_343:0100008
name: 1-5 scale
namespace: YamScale
is_a: CO_343:1000017 ! Nominal
relationship: scale_of CO_343:0010011 ! sprout color - estimation
relationship: scale_of CO_343:0010080 ! leaf beetle severity - estimation
relationship: scale_of CO_343:0010082 ! mealybug tuber severity - estimation
relationship: scale_of CO_343:0010084 ! root knot nematode severity - estimation
relationship: scale_of CO_343:0010086 ! tuber beetle severity - estimation
relationship: scale_of CO_343:0010088 ! viruses infection severity - estimation
relationship: scale_of CO_343:0010163 ! taste of pounded yam - estimation
relationship: scale_of CO_343:0010165 ! stem color - estimation
relationship: scale_of CO_343:0010175 ! leaf color - estimation

[Term]
id: CO_343:0100009
name: cm
namespace: YamScale
is_a: CO_343:1000019 ! Numerical
relationship: scale_of CO_343:0010012 ! sprout length-computation
relationship: scale_of CO_343:0010022 ! internode length -computation
relationship: scale_of CO_343:0010131 ! length of big size tubers-computation
relationship: scale_of CO_343:0010132 ! length of medium size tubers-computation
relationship: scale_of CO_343:0010133 ! length of small size tubers-computation
relationship: scale_of CO_343:0010134 ! tuber length-computation
relationship: scale_of CO_343:0010137 ! width of big size tubers-computation
relationship: scale_of CO_343:0010138 ! width of medium size tubers-computation
relationship: scale_of CO_343:0010139 ! width of small size tubers-computation
relationship: scale_of CO_343:0010140 ! tuber wideth-computation
relationship: scale_of CO_343:0010171 ! leaf length - computation
relationship: scale_of CO_343:0010172 ! leaf width - computation
relationship: scale_of CO_343:0010173 ! internode length - computation
relationship: scale_of CO_343:0010178 ! petiole length - computation

[Term]
id: CO_343:0100010
name: 0-2 scale
namespace: YamScale
is_a: CO_343:1000015 ! Ordinal
relationship: scale_of CO_343:0010015 ! hairiness of sprout - estimation
relationship: scale_of CO_343:0010024 ! density of spines on stem base of a plant-etimation
relationship: scale_of CO_343:0010164 ! scale insect infestation - estimation
relationship: scale_of CO_343:0010174 ! hair on stem - estimation
relationship: scale_of CO_343:0010177 ! leaf hairiness - estimation

[Term]
id: CO_343:0100011
name: 1-3 general scale
namespace: YamScale
is_a: CO_343:1000017 ! Nominal
relationship: scale_of CO_343:0010018 ! leaf apex shape-estimation
relationship: scale_of CO_343:0010025 ! plant type-estimation
relationship: scale_of CO_343:0010027 ! plant vigor - estimation
relationship: scale_of CO_343:0010145 ! corm size-estimation
relationship: scale_of CO_343:0010146 ! corm type-estimation
relationship: scale_of CO_343:0010162 ! stickiness of pounded yam - estimation

[Term]
id: CO_343:0100012
name: 1-7 general scale
namespace: YamScale
is_a: CO_343:1000017 ! Nominal
relationship: scale_of CO_343:0010019 ! leaf shape-estimation
relationship: scale_of CO_343:0010149 ! tuber flesh color head portion - estimation
relationship: scale_of CO_343:0010150 ! tuber flesh color middle portion - estimation
relationship: scale_of CO_343:0010151 ! tuber flesh color lower or tail portion- estimation

[Term]
id: CO_343:0100013
name: number of stem
namespace: YamScale
is_a: CO_343:1000019 ! Numerical
relationship: scale_of CO_343:0010020 ! number of stems per plant-computation

[Term]
id: CO_343:0100014
name: mm
namespace: YamScale
is_a: CO_343:1000019 ! Numerical
relationship: scale_of CO_343:0010021 ! stem diameter-computation

[Term]
id: CO_343:0100015
name: number of internode
namespace: YamScale
is_a: CO_343:1000019 ! Numerical
relationship: scale_of CO_343:0010023 ! number of internode-computation

[Term]
id: CO_343:0100016
name: 1-4 general scale
namespace: YamScale
is_a: CO_343:1000017 ! Nominal
relationship: scale_of CO_343:0010026 ! canopy architecture - estimation
relationship: scale_of CO_343:0010043 ! femal flowers abundance or intensity per inflorescence-estimation
relationship: scale_of CO_343:0010093 ! bulbil shape-estimation
relationship: scale_of CO_343:0010147 ! dormancy period -estimation

[Term]
id: CO_343:0100017
name: 0-1 nominal scale
namespace: YamScale
is_a: CO_343:1000017 ! Nominal
relationship: scale_of CO_343:0010028 ! twining habit-estimation

[Term]
id: CO_343:0100018
name: 1-2 nominal scale
namespace: yamScale
is_a: CO_343:1000017 ! Nominal
relationship: scale_of CO_343:0010029 ! twining direction-estimation

[Term]
id: CO_343:0100019
name: number of florets
namespace: YamScale
is_a: CO_343:1000019 ! Numerical
relationship: scale_of CO_343:0010037 ! floret pollinated number - counting

[Term]
id: CO_343:0100020
name: number of spikes
namespace: YamScale
is_a: CO_343:1000019 ! Numerical
relationship: scale_of CO_343:0010038 ! pollinated spike number - estimation

[Term]
id: CO_343:0100021
name: 0-9 scale
namespace: YamScale
is_a: CO_343:1000015 ! Ordinal
relationship: scale_of CO_343:0010039 ! flowering intensity - estimation

[Term]
id: CO_343:0100022
name: 1-3 scale
namespace: YamScale
is_a: CO_343:1000017 ! Nominal
relationship: scale_of CO_343:0010042 ! inflorescence type-estimation
relationship: scale_of CO_343:0010053 ! fruit set number - estimation
relationship: scale_of CO_343:0010126 ! hairiness of tuber bark - estimation
relationship: scale_of CO_343:0010136 ! tuber size - estimation
relationship: scale_of CO_343:0010155 ! tuber flesh texture-estimation
relationship: scale_of CO_343:0010156 ! tuber oxidation-estimation
relationship: scale_of CO_343:0010158 ! cohesiveness of pounded yam- estimation
relationship: scale_of CO_343:0010160 ! smoothness of pounded yam- estimation
relationship: scale_of CO_343:0010170 ! leaf position - estimation

[Term]
id: CO_343:0100023
name: 1-4 scale
namespace: YamScale
is_a: CO_343:1000017 ! Nominal
relationship: scale_of CO_343:0010044 ! pollination type-estimation
relationship: scale_of CO_343:0010125 ! position of root appearance on tubers-estimation
relationship: scale_of CO_343:0010127 ! tuber surface appearance - estimation
relationship: scale_of CO_343:0010157 ! tuber flesh oxidation color-estimation
relationship: scale_of CO_343:0010176 ! vein color - estimation

[Term]
id: CO_343:0100024
name: 0-4 scale
namespace: YamScale
is_a: CO_343:1000017 ! Nominal
relationship: scale_of CO_343:0010045 ! plant or flower sex-estimation

[Term]
id: CO_343:0100025
name: fruits/cross
namespace: YamScale
is_a: CO_343:1000019 ! Numerical
relationship: scale_of CO_343:0010046 ! fruits developed number - counting

[Term]
id: CO_343:0100026
name: number of fruits
namespace: YamScale
is_a: CO_343:1000019 ! Numerical
relationship: scale_of CO_343:0010049 ! fruits harvested number - counting

[Term]
id: CO_343:0100027
name: 1-2 scale
namespace: YamScale
is_a: CO_343:1000015 ! Ordinal
relationship: scale_of CO_343:0010055 ! fruit development intensity-estimation
relationship: scale_of CO_343:0010128 ! tuber surface texture - estimation
relationship: scale_of CO_343:0010159 ! springiness of pounded yam-estimation
relationship: scale_of CO_343:0010161 ! presence of fiber strand-estimation

[Term]
id: CO_343:0100028
name: number of seed
namespace: YamScale
is_a: CO_343:1000019 ! Numerical
relationship: scale_of CO_343:0010056 ! seeds set - comp
relationship: scale_of CO_343:0010057 ! quantity of true seed harvested -counting
relationship: scale_of CO_343:0010059 ! seed index
relationship: scale_of CO_343:0010060 ! number of true seeds sown-counting
relationship: scale_of CO_343:0010064 ! number of germinated seedling-counting

[Term]
id: CO_343:0100029
name: number of fruit
namespace: YamScale
is_a: CO_343:1000019 ! Numerical
relationship: scale_of CO_343:0010058 ! fruit index

[Term]
id: CO_343:0100030
name: number of plant
namespace: YamScale
is_a: CO_343:1000019 ! Numerical
relationship: scale_of CO_343:0010067 ! vine cuttings planted -counting

[Term]
id: CO_343:0100031
name: gdd°c
namespace: YamScale
is_a: CO_343:1000018 ! Duration
relationship: scale_of CO_343:0010073 ! growing degere days to maturity-estimation

[Term]
id: CO_343:0100032
name: 1-9 scale
namespace: YamScale
is_a: CO_343:1000015 ! Ordinal
relationship: scale_of CO_343:0010074 ! maturity class - estimation

[Term]
id: CO_343:0100033
name: number
namespace: yamScale
is_a: CO_343:1000019 ! Numerical
relationship: scale_of CO_343:0010076 ! dry rot tuber number-counting
relationship: scale_of CO_343:0010152 ! tuber flesh color reading -measurement

[Term]
id: CO_343:0100034
name: 0-4 general scale
namespace: YamScale
is_a: CO_343:1000015 ! Ordinal
relationship: scale_of CO_343:0010078 ! tuber dry rot severity - estimation

[Term]
id: CO_343:0100035
name: 1-5 general scale
namespace: YamScale
is_a: CO_343:1000015 ! Ordinal
relationship: scale_of CO_343:0010090 ! anthracnose severity - estimation

[Term]
id: CO_343:0100036
name: number of bulbils
namespace: YamScale
is_a: CO_343:1000019 ! Numerical
relationship: scale_of CO_343:0010091 ! number of bulbil - counting

[Term]
id: CO_343:0100037
name: bulbil/plant
namespace: YamScale
is_a: CO_343:1000019 ! Numerical
relationship: scale_of CO_343:0010092 ! number of bulbil - computation

[Term]
id: CO_343:0100038
name: kg
namespace: YamScale
is_a: CO_343:1000019 ! Numerical
relationship: scale_of CO_343:0010094 ! bulbil yield (plot weight) - measurement
relationship: scale_of CO_343:0010123 ! big yam tuber average weight-computation
relationship: scale_of CO_343:0010124 ! average tuber weight -computation

[Term]
id: CO_343:0100039
name: kg/plant
namespace: YamScale
is_a: CO_343:1000019 ! Numerical
relationship: scale_of CO_343:0010095 ! bulbil yield (fresh weight) per plant-computation
relationship: scale_of CO_343:0010115 ! total tuber fresh weight per plant-computation
relationship: scale_of CO_343:0010116 ! big size yam fresh weight per plant- computation
relationship: scale_of CO_343:0010117 ! medium size yam fresh weight per plant-computation
relationship: scale_of CO_343:0010118 ! small size yam fresh weight per plant-computation

[Term]
id: CO_343:0100040
name: tons/ha
namespace: YamScale
is_a: CO_343:1000019 ! Numerical
relationship: scale_of CO_343:0010096 ! bulbil yield (fresh weight) per hectar- computation
relationship: scale_of CO_343:0010119 ! tuber yield no adjusted- computation
relationship: scale_of CO_343:0010120 ! big size yam yield no adjusted- computation
relationship: scale_of CO_343:0010121 ! total tuber yield adjusted-computation
relationship: scale_of CO_343:0010122 ! big size yam yield adjusted-computation

[Term]
id: CO_343:0100041
name: plant per plot
namespace: YamScale
is_a: CO_343:1000019 ! Numerical
relationship: scale_of CO_343:0010100 ! plant harvested number - counting

[Term]
id: CO_343:0100042
name: tuber number/plot
namespace: YamScale
is_a: CO_343:1000019 ! Numerical
relationship: scale_of CO_343:0010101 ! big size tubers harvested number - counting
relationship: scale_of CO_343:0010102 ! medium size tubers harvested number- counting
relationship: scale_of CO_343:0010103 ! small size tubers harvested per plot number - counting
relationship: scale_of CO_343:0010104 ! rotten tubers in a plot number-counting
relationship: scale_of CO_343:0010105 ! total tuber harvested number-computation

[Term]
id: CO_343:0100043
name: tuber number/plant
namespace: YamScale
is_a: CO_343:1000019 ! Numerical
relationship: scale_of CO_343:0010106 ! big size tubers per plant-computation
relationship: scale_of CO_343:0010107 ! medium size tubers per plant-computation
relationship: scale_of CO_343:0010108 ! small size tubers per plant-computation
relationship: scale_of CO_343:0010109 ! total tubers per plant-computation

[Term]
id: CO_343:0100044
name: kg/plot
namespace: YamScale
is_a: CO_343:1000019 ! Numerical
relationship: scale_of CO_343:0010110 ! big size tubers fresh weight per plot- measurement
relationship: scale_of CO_343:0010111 ! medium size tubers fresh weight per plot -measurement
relationship: scale_of CO_343:0010112 ! small size tubers fresh weight per plot- measurement
relationship: scale_of CO_343:0010113 ! rotten tuber fresh weight per plot - measurement
relationship: scale_of CO_343:0010114 ! total tuber fresh weight per plot -computation

[Term]
id: CO_343:0100045
name: 0-1 binary scale
namespace: YamScale
is_a: CO_343:1000017 ! Nominal
relationship: scale_of CO_343:0010129 ! tuber thorniness - estimation

[Term]
id: CO_343:0100046
name: 0-7 scale
namespace: YamScale
is_a: CO_343:1000015 ! Ordinal
relationship: scale_of CO_343:0010130 ! tuber thorniness intensity-estimation

[Term]
id: CO_343:0100047
name: 1-4 score
namespace: YamScale
is_a: CO_343:1000017 ! Nominal
relationship: scale_of CO_343:0010135 ! tuber shape - estimation

[Term]
id: CO_343:0100048
name: 0-3 scale
namespace: YamScale
is_a: CO_343:1000015 ! Ordinal
relationship: scale_of CO_343:0010141 ! cracks on the tuber surface-estimation
relationship: scale_of CO_343:0010154 ! tuber flesh oxidation intensity-estimation

[Term]
id: CO_343:0100049
name: 0-1  scale
namespace: YamScale
is_a: CO_343:1000017 ! Nominal
relationship: scale_of CO_343:0010142 ! crazy roots presence on tubers at harvest-estimation
relationship: scale_of CO_343:0010143 ! corm on tubers-estimation
relationship: scale_of CO_343:0010144 ! corm separation from tuber-estimation

[Term]
id: CO_343:0100050
name: 1-7 scale
namespace: YamScale
is_a: CO_343:1000015 ! Ordinal
relationship: scale_of CO_343:0010166 ! leaf density - estimation

[Term]
id: CO_343:0100051
name: number of branch
namespace: YamScale
is_a: CO_343:1000019 ! Numerical
relationship: scale_of CO_343:0010167 ! number of branchs - computation

[Term]
id: CO_343:0100052
name: m
namespace: YamScale
is_a: CO_343:1000019 ! Numerical
relationship: scale_of CO_343:0010168 ! stem height - computation

[Term]
id: CO_343:0100053
name: number of leaf
namespace: YamScale
is_a: CO_343:1000019 ! Numerical
relationship: scale_of CO_343:0010169 ! number of leaves - computation

[Term]
id: CO_343:0100199
name: Earliness of emergence computation in number of days from planting to 50% sprouts emergence
namespace: YamTrait
def: "Earliness of emergence in number of days from planting to 50% sprouts emergence" []
is_a: CO_343:1000003 ! Variable
relationship: variable_of CO_343:0100003 ! days
relationship: variable_of CO_343:0100200 ! Earliness of emergence
relationship: variable_of CO_343:0100201 ! Period from planting to median emergence
created_by: D. Cornut

[Term]
id: CO_343:0100200
name: Earliness of emergence
namespace: YamTrait
def: "Elapsed time between planting date and date of 50% emergence sprouts in a plot" []
is_a: CO_343:1000006 ! Phenological_trait

[Term]
id: CO_343:0100201
name: Period from planting to median emergence
namespace: YamMethod
def: "Computation of inflection point value using log-logistic time-to-event modeling of weekly sprout counts expressed in days after planting" []
is_a: CO_343:1000013 ! Computation
relationship: method_of CO_343:0100200 ! Earliness of emergence

[Term]
id: CO_343:0100202
name: Latency period duration computation in number of days from planting to 5% sprouts emergence
namespace: YamTrait
def: "Latency period duration in number of days from planting to 5% sprouts emergence" []
is_a: CO_343:1000003 ! Variable
relationship: variable_of CO_343:0100003 ! days
relationship: variable_of CO_343:0100203 ! Latency before emergence
relationship: variable_of CO_343:0100204 ! Period from planting to 5% emergence
created_by: D. Cornut

[Term]
id: CO_343:0100203
name: Latency before emergence
namespace: YamTrait
def: "Elapsed time between planting date and date of 5th percentile emergence sprouts in a plot" []
is_a: CO_343:1000006 ! Phenological_trait

[Term]
id: CO_343:0100204
name: Period from planting to 5% emergence
namespace: YamMethod
def: "Computation of the necessary time before 5% emergence using after-fitting inverse regression of log-logistic time-to-event modeling of weekly sprout counts expressed in days after planting" []
is_a: CO_343:1000013 ! Computation
relationship: method_of CO_343:0100203 ! Latency before emergence

[Term]
id: CO_343:0100205
name: Emergence vigor computation in number of days between 5% and 95% sprouts emergence
namespace: YamTrait
def: "Emergence vigor expressed in number of days between 5% and 95% sprouts emergence" []
is_a: CO_343:1000003 ! Variable
relationship: variable_of CO_343:0100003 ! days
relationship: variable_of CO_343:0100206 ! Emergence vigor
relationship: variable_of CO_343:0100207 ! Period from 5% to 95% emergence
created_by: D. Cornut

[Term]
id: CO_343:0100206
name: Emergence vigor
namespace: YamTrait
def: "Elapsed time between time of 5th and 95th percentiles emergence sprouts in a plot" []
is_a: CO_343:1000008 ! Agronomical_trait

[Term]
id: CO_343:0100207
name: Period from 5% to 95% emergence
namespace: YamMethod
def: "Computation of the substraction between the necessary time before 95% and 5% emergence using after-fitting inverse regression of log-logistic time-to-event modeling of weekly sprout counts expressed in days after planting" []
is_a: CO_343:1000013 ! Computation
relationship: method_of CO_343:0100206 ! Emergence vigor

[Term]
id: CO_343:0100208
name: Heterophylly presence estimation nominal 0&1
namespace: YamTrait
def: "Estimation of heterophylly presence (0: absence - 1: presence)" []
is_a: CO_343:1000003 ! Variable
relationship: variable_of CO_343:0100007 ! 0-1 scale
relationship: variable_of CO_343:0100209 ! Heterophylly presence
relationship: variable_of CO_343:0100210 ! Presence of cataphylle
created_by: D. Cornut

[Term]
id: CO_343:0100209
name: Heterophylly presence
namespace: YamTrait
def: "Presence of cataphylles during early stage" []
is_a: CO_343:1000010 ! Morphological_trait

[Term]
id: CO_343:0100210
name: Presence of cataphylle
namespace: YamMethod
def: "Observe the presence or absence of cataphylle" []
is_a: CO_343:1000014 ! Estimation
relationship: method_of CO_343:0100209 ! Heterophylly presence

[Term]
id: CO_343:0100211
name: Number of nodes carrying cataphylles before first true leaf counting/plant
namespace: YamTrait
def: "Number of nodes carrying cataphylles before first true leaf expressed in number of nodes per plant" []
is_a: CO_343:1000003 ! Variable
relationship: variable_of CO_343:0100212 ! Number of nodes carrying cataphylles
relationship: variable_of CO_343:0100213 ! Nodes carrying cataphylles  - Counting
relationship: variable_of CO_343:0100214 ! Nodes carrying cataphylle per plant
created_by: D. Cornut

[Term]
id: CO_343:0100212
name: Number of nodes carrying cataphylles
namespace: YamTrait
def: "Mean number of nodes carrying cataphylles on main stem of 5 plants choosen randomly" []
is_a: CO_343:1000010 ! Morphological_trait

[Term]
id: CO_343:0100213
name: Nodes carrying cataphylles  - Counting
namespace: YamMethod
def: "Compute the average of the number of nodes carrying cataphylles on the main stem of 5 plants choosen randomly" []
is_a: CO_343:1000012 ! Counting
relationship: method_of CO_343:0100212 ! Number of nodes carrying cataphylles

[Term]
id: CO_343:0100214
name: Nodes carrying cataphylle per plant
namespace: YamScale
is_a: CO_343:1000019 ! Numerical
relationship: scale_of CO_343:0100213 ! Nodes carrying cataphylles  - Counting

[Term]
id: CO_343:0100215
name: Duration of heterophyllic period computation in days after planting
namespace: YamTrait
def: "Duration from emergence to first true leaf in days after planting" []
is_a: CO_343:1000003 ! Variable
relationship: variable_of CO_343:0100003 ! days
relationship: variable_of CO_343:0100216 ! Duration from emergence to first true leaf
relationship: variable_of CO_343:0100217 ! Duration of heterophylly period - Computing
created_by: D. Cornut

[Term]
id: CO_343:0100216
name: Duration from emergence to first true leaf
namespace: YamTrait
def: "Mean duration between fisrt emergence and first true leaf apprearance on main stem of 5 plants choosen randomly" []
is_a: CO_343:1000006 ! Phenological_trait

[Term]
id: CO_343:0100217
name: Duration of heterophylly period - Computing
namespace: YamMethod
def: "Compute the average of the period from emergence to first true leaf appearance on the main stem of 5 plants choosen randomly" []
is_a: CO_343:1000013 ! Computation
relationship: method_of CO_343:0100216 ! Duration from emergence to first true leaf

[Term]
id: CO_343:0100218
name: Maximum ground cover computation in %
namespace: YamTrait
def: "Subplot maximum ground cover from weekly image analysis in %" []
is_a: CO_343:1000003 ! Variable
relationship: variable_of CO_343:0100006 ! %
relationship: variable_of CO_343:0100219 ! Maximum ground cover
relationship: variable_of CO_343:0100220 ! Subplot maximum ground cover from weekly image analysis - Computation
created_by: D. Cornut

[Term]
id: CO_343:0100219
name: Maximum ground cover
namespace: YamTrait
def: "Maximum ground cover" []
is_a: CO_343:1000008 ! Agronomical_trait

[Term]
id: CO_343:0100220
name: Subplot maximum ground cover from weekly image analysis - Computation
namespace: YamMethod
def: "Averaged maximum ground cover over two subplots. \nGround cover computed from weekly images analysis. \nMaximum ground cover computed from ground cover dynamic modeled using time to event Beta Growth model. " []
is_a: CO_343:1000013 ! Computation
relationship: method_of CO_343:0100219 ! Maximum ground cover

[Term]
id: CO_343:0100221
name: Crop vigor computation in days from median emergence to 80% of maximum ground cover
namespace: YamTrait
def: "Duration from median emergence to 80% of maximum ground cover of subplot in days" []
is_a: CO_343:1000003 ! Variable
relationship: variable_of CO_343:0100003 ! days
relationship: variable_of CO_343:0100222 ! Crop vigor
relationship: variable_of CO_343:0100223 ! Duration from median emergence to 80% of maximum ground cover of subplot - Computation
created_by: D. Cornut

[Term]
id: CO_343:0100222
name: Crop vigor
namespace: YamTrait
def: "Duration from median emergence to 80% of maximum ground cover" []
is_a: CO_343:1000008 ! Agronomical_trait

[Term]
id: CO_343:0100223
name: Duration from median emergence to 80% of maximum ground cover of subplot - Computation
namespace: YamMethod
def: "Averaged crop vigor expressed in days from median emergence to 80% of maximum ground cover in subplots.\nGround cover computed from weekly images analysis. \nTime at 80% of maximum growth computed via inverse regression of time to event Beta ground cover dynamic model. " []
is_a: CO_343:1000013 ! Computation
relationship: method_of CO_343:0100222 ! Crop vigor

[Term]
id: CO_343:0100224
name: Crop cover compactness computation
namespace: YamTrait
def: "Ratio between subplot ground cover area and its respective convex hull area" []
is_a: CO_343:1000003 ! Variable
relationship: variable_of CO_343:0100225 ! Crop folliage compactness
relationship: variable_of CO_343:0100226 ! Ratio between subplot ground cover area and its respective convex hull area - Computation
relationship: variable_of CO_343:0100227 ! unitless
created_by: D. Cornut

[Term]
id: CO_343:0100225
name: Crop folliage compactness
namespace: YamTrait
def: "Crop cover compactness" []
is_a: CO_343:1000010 ! Morphological_trait

[Term]
id: CO_343:0100226
name: Ratio between subplot ground cover area and its respective convex hull area - Computation
namespace: YamMethod
def: "Averaged crop cover compactness over two subplots images around time of 50% of maximum ground cover.\nGround cover computed from weekly images analysis. \nTime at 50% of maximum growth computed via inverse regression of time to event Beta ground cover dynamic model. \nImages choosen as near as possible of date of time at 50% of maximum growth .\nCompactness computed as the ration between ground cover area (pixels) and its respective convex hull area (pixels)." []
is_a: CO_343:1000013 ! Computation
relationship: method_of CO_343:0100225 ! Crop folliage compactness

[Term]
id: CO_343:0100227
name: unitless
namespace: YamScale
is_a: CO_343:1000019 ! Numerical
relationship: scale_of CO_343:0100226 ! Ratio between subplot ground cover area and its respective convex hull area - Computation
relationship: scale_of CO_343:0100239 ! Tuber flesh color computation from standardized image L*a*b* values
relationship: scale_of CO_343:0100242 ! Color difference bewteen mean tuber head and tail flesh color computed from standardized image L*a*b* values
relationship: scale_of CO_343:0100245 ! Tuber flesh brown index computation from standardized image L*a*b* values
relationship: scale_of CO_343:0100248 ! Tuber flesh white index computation from standardized image L*a*b* values
relationship: scale_of CO_343:0100251 ! Tuber flesh yellow index computation from standardized image L*a*b* values
relationship: scale_of CO_343:0100253 ! Mean color difference between average tuber flesh color computed from standardized image L*a*b* values and  tuber flesh color of individual pixel values
relationship: scale_of CO_343:0100256 ! Color difference bewteen mean tuber flesh color computed from standardized image L*a*b* values at cutting and 15 minutes latter

[Term]
id: CO_343:0100228
name: Senescence earliness computation in days from median emergence to 5% senescence
namespace: YamTrait
def: "Senescence earliness as the duration in days from median emergence to 5% senescence of subplot" []
is_a: CO_343:1000003 ! Variable
relationship: variable_of CO_343:0100003 ! days
relationship: variable_of CO_343:0100229 ! Senescence earliness
relationship: variable_of CO_343:0100230 ! Duration from median emergence to 5% senescence of subplot - Computation
created_by: D. Cornut

[Term]
id: CO_343:0100229
name: Senescence earliness
namespace: YamTrait
def: "Time from median emergence to 5% senescence" []
is_a: CO_343:1000006 ! Phenological_trait

[Term]
id: CO_343:0100230
name: Duration from median emergence to 5% senescence of subplot - Computation
namespace: YamMethod
def: "Averaged senescence earliness expressed in days from median emergence to 5% senescence (i.e. 95% of maximum ground cover after time to maximum ground cover) in two subplots.\nGround cover computed from weekly images analysis. \nTime at 95% of maximum growth after time at maximum growth computed via inverse regression of time to event Beta ground cover dynamic model." []
is_a: CO_343:1000013 ! Computation
relationship: method_of CO_343:0100229 ! Senescence earliness

[Term]
id: CO_343:0100231
name: Senescence period duration computation in days between 5 and 95% senescence
namespace: YamTrait
def: "Duration of the senescence period of a subplot in days between 5% emergence and 95% senescence" []
is_a: CO_343:1000003 ! Variable
relationship: variable_of CO_343:0100003 ! days
relationship: variable_of CO_343:0100232 ! Senescence duration
relationship: variable_of CO_343:0100233 ! Duration between 5 and 95% senescence of subplot - Computation
created_by: D. Cornut

[Term]
id: CO_343:0100232
name: Senescence duration
namespace: YamTrait
def: "Time between 5 and 95% senescence" []
is_a: CO_343:1000006 ! Phenological_trait

[Term]
id: CO_343:0100233
name: Duration between 5 and 95% senescence of subplot - Computation
namespace: YamMethod
def: "Averaged senescence period duration expressed in days between 5 and 95% senescence (i.e. 95%  and 5% of maximum ground cover after time to maximum ground cover) in two subplots.\nGround cover computed from weekly images analysis. \nTime at 95% and 5% of maximum growth after time at maximum growth computed via inverse regression of time to event Beta ground cover dynamic model." []
is_a: CO_343:1000013 ! Computation
relationship: method_of CO_343:0100232 ! Senescence duration

[Term]
id: CO_343:0100234
name: Growth cycle length computation in days between 5% emergence and 95% senescence
namespace: YamTrait
def: "Duration of the growth cycle of a subplot in days between 5% emergence and 95% senescence" []
is_a: CO_343:1000003 ! Variable
relationship: variable_of CO_343:0100003 ! days
relationship: variable_of CO_343:0100235 ! Growth cycle length
relationship: variable_of CO_343:0100236 ! Duration between 5% emergence and 95% senescence of subplot - Computation
created_by: D. Cornut

[Term]
id: CO_343:0100235
name: Growth cycle length
namespace: YamTrait
def: "Time between 5% emergence and 95% senescence" []
is_a: CO_343:1000006 ! Phenological_trait

[Term]
id: CO_343:0100236
name: Duration between 5% emergence and 95% senescence of subplot - Computation
namespace: YamMethod
def: "Averaged growth cycle duration expressed in days between  5% emergence and 95% senescence (i.e. 5% of maximum ground cover after time to maximum ground cover) in two subplots.\nGround cover computed from weekly images analysis. \nMedian senescence computed from inflection point value using log-logistic time-to-event modeling of weekly sprout counts expressed in days after planting.\nTime at 5% of maximum growth after time at maximum growth computed via inverse regression of time to event Beta ground cover dynamic model." []
is_a: CO_343:1000013 ! Computation
relationship: method_of CO_343:0100235 ! Growth cycle length

[Term]
id: CO_343:0100237
name: Tuber flesh color computation
namespace: YamTrait
def: "The tuber flesh color computation from standardized image" []
is_a: CO_343:1000003 ! Variable
relationship: variable_of CO_343:0000147 ! tuber flesh color
relationship: variable_of CO_343:0100227 ! unitless
relationship: variable_of CO_343:0100239 ! Tuber flesh color computation from standardized image L*a*b* values
created_by: D. Cornut

[Term]
id: CO_343:0100239
name: Tuber flesh color computation from standardized image L*a*b* values
namespace: YamMethod
def: "Compute the average of the flesh surface color of tuber longitudinal section using image analysis with a color correction based on a custom color chart " []
is_a: CO_343:1000013 ! Computation
relationship: variable_of CO_343:0000147 ! tuber flesh color

[Term]
id: CO_343:0100240
name: Tuber flesh color gradient computation
namespace: YamTrait
def: "The color difference bewteen mean tuber head and tail flesh color computed from standardized image" []
is_a: CO_343:1000003 ! Variable
relationship: variable_of CO_343:0100227 ! unitless
relationship: variable_of CO_343:0100241 ! Tuber flesh uniformity
relationship: variable_of CO_343:0100242 ! Color difference bewteen mean tuber head and tail flesh color computed from standardized image L*a*b* values
created_by: D. Cornut

[Term]
id: CO_343:0100241
name: Tuber flesh uniformity
namespace: YamTrait
def: "Uniformity of tuber flesh surface color in longitudinal section" []
is_a: CO_343:1000007 ! Quality_trait

[Term]
id: CO_343:0100242
name: Color difference bewteen mean tuber head and tail flesh color computed from standardized image L*a*b* values
namespace: YamMethod
def: "Compute the ∆E2000 bewteen mean tuber head and tail flesh color computed from standardized image L*a*b* values " []
is_a: CO_343:1000013 ! Computation
relationship: method_of CO_343:0100241 ! Tuber flesh uniformity

[Term]
id: CO_343:0100243
name: Tuber flesh brownness computation
namespace: YamTrait
def: "The tuber flesh brown index computation from standardized image" []
is_a: CO_343:1000003 ! Variable
relationship: variable_of CO_343:0100227 ! unitless
relationship: variable_of CO_343:0100244 ! Browness of the Tuber flesh colour
relationship: variable_of CO_343:0100245 ! Tuber flesh brown index computation from standardized image L*a*b* values
created_by: D. Cornut

[Term]
id: CO_343:0100244
name: Browness of the Tuber flesh colour
namespace: YamTrait
def: "The surface browness of the yam tuber flesh" []
is_a: CO_343:1000007 ! Quality_trait

[Term]
id: CO_343:0100245
name: Tuber flesh brown index computation from standardized image L*a*b* values
namespace: YamMethod
def: "Compute the brown index based on the flesh surface color of tuber longitudinal section using image analysis with a color correction based on a custom color chart " []
is_a: CO_343:1000013 ! Computation
relationship: method_of CO_343:0100244 ! Browness of the Tuber flesh colour

[Term]
id: CO_343:0100246
name: Tuber flesh whiteness computation
namespace: YamTrait
def: "The tuber flesh white index computation from standardized image" []
is_a: CO_343:1000003 ! Variable
relationship: variable_of CO_343:0100227 ! unitless
relationship: variable_of CO_343:0100247 ! Whitness of the Flesh colour
relationship: variable_of CO_343:0100248 ! Tuber flesh white index computation from standardized image L*a*b* values
created_by: D. Cornut

[Term]
id: CO_343:0100247
name: Whitness of the Flesh colour
namespace: YamTrait
def: "The surface whiteness of the yam tuber flesh" []
is_a: CO_343:1000007 ! Quality_trait

[Term]
id: CO_343:0100248
name: Tuber flesh white index computation from standardized image L*a*b* values
namespace: YamMethod
def: "Compute the white index based on the flesh surface color of tuber longitudinal section using image analysis with a color correction based on a custom color chart " []
is_a: CO_343:1000013 ! Computation
relationship: method_of CO_343:0100247 ! Whitness of the Flesh colour

[Term]
id: CO_343:0100249
name: Tuber flesh yellowness computation
namespace: YamTrait
def: "The tuber flesh yellow index computation from standardized image" []
is_a: CO_343:1000003 ! Variable
relationship: variable_of CO_343:0100227 ! unitless
relationship: variable_of CO_343:0100250 ! Yellowness of the Flesh colour
relationship: variable_of CO_343:0100251 ! Tuber flesh yellow index computation from standardized image L*a*b* values
created_by: D. Cornut

[Term]
id: CO_343:0100250
name: Yellowness of the Flesh colour
namespace: YamTrait
def: "The surface yellowness of the yam tuber flesh" []
is_a: CO_343:1000007 ! Quality_trait

[Term]
id: CO_343:0100251
name: Tuber flesh yellow index computation from standardized image L*a*b* values
namespace: YamMethod
def: "Compute the yellow index based on the flesh surface color of tuber longitudinal section using image analysis with a color correction based on a custom color chart " []
is_a: CO_343:1000013 ! Computation
relationship: method_of CO_343:0100250 ! Yellowness of the Flesh colour

[Term]
id: CO_343:0100252
name: Tuber color uniformity computation
namespace: YamTrait
def: "The mean color difference between average tuber flesh color computed from standardized image" []
is_a: CO_343:1000003 ! Variable
relationship: variable_of CO_343:0100227 ! unitless
relationship: variable_of CO_343:0100241 ! Tuber flesh uniformity
relationship: variable_of CO_343:0100253 ! Mean color difference between average tuber flesh color computed from standardized image L*a*b* values and  tuber flesh color of individual pixel values
created_by: D. Cornut

[Term]
id: CO_343:0100253
name: Mean color difference between average tuber flesh color computed from standardized image L*a*b* values and  tuber flesh color of individual pixel values
namespace: YamMethod
def: "Compute the ∆E2000 between average tuber flesh color computed from standardized image L*a*b* values and  tuber flesh color of individual pixel values " []
is_a: CO_343:1000013 ! Computation
relationship: method_of CO_343:0100241 ! Tuber flesh uniformity

[Term]
id: CO_343:0100254
name: Intensity of tuber flesh oxidation computation
namespace: YamTrait
def: "The color difference bewteen mean tuber flesh color computed from standardized image." []
is_a: CO_343:1000003 ! Variable
relationship: variable_of CO_343:0100227 ! unitless
relationship: variable_of CO_343:0100255 ! Tuber flesh browning
relationship: variable_of CO_343:0100256 ! Color difference bewteen mean tuber flesh color computed from standardized image L*a*b* values at cutting and 15 minutes latter
created_by: D. Cornut

[Term]
id: CO_343:0100255
name: Tuber flesh browning
namespace: YamTrait
def: "Intensity of tuber flesh enzymatic oxidation (degree of flesh color change or browning of cut yam tuber)" []
is_a: CO_343:1000007 ! Quality_trait

[Term]
id: CO_343:0100256
name: Color difference bewteen mean tuber flesh color computed from standardized image L*a*b* values at cutting and 15 minutes latter
namespace: YamMethod
def: "Compute the ∆E2000 bewteen mean tuber flesh color computed from standardized image L*a*b* values at cutting and 15 minutes latter " []
is_a: CO_343:1000013 ! Computation
relationship: method_of CO_343:0100255 ! Tuber flesh browning

[Term]
id: CO_343:0100257
name: Tuber flour protein content computation
namespace: YamTrait
def: "The flour protein content predicted by NIRS model in %" []
is_a: CO_343:1000003 ! Variable
relationship: variable_of CO_343:0100006 ! %
relationship: variable_of CO_343:0100258 ! Tuber flour protein content
relationship: variable_of CO_343:0100259 ! NIRS model prediction - computation
created_by: D. Cornut

[Term]
id: CO_343:0100258
name: Tuber flour protein content
namespace: YamTrait
def: "Tuber flour protein content" []
is_a: CO_343:1000007 ! Quality_trait

[Term]
id: CO_343:0100259
name: NIRS model prediction - computation
namespace: YamMethod
def: "Prediction of sugar content using NIRS spectra (FOSS 6500) of tuber flour sample" []
is_a: CO_343:1000021 ! Prediction
relationship: method_of CO_343:0100258 ! Tuber flour protein content
relationship: method_of CO_343:0100261 ! Tuber flour starch content
relationship: method_of CO_343:0100263 ! Tuber flour sugar content

[Term]
id: CO_343:0100260
name: Tuber flour starch content computation
namespace: YamTrait
def: "The flour starch content predicted by NIRS model in %" []
is_a: CO_343:1000003 ! Variable
relationship: variable_of CO_343:0100006 ! %
relationship: variable_of CO_343:0100259 ! NIRS model prediction - computation
relationship: variable_of CO_343:0100261 ! Tuber flour starch content
created_by: D. Cornut

[Term]
id: CO_343:0100261
name: Tuber flour starch content
namespace: YamTrait
def: "Tuber flour starch content" []
is_a: CO_343:1000007 ! Quality_trait

[Term]
id: CO_343:0100262
name: Tuber flour sugar content computation
namespace: YamTrait
def: "The tuber flour sugar content predicted by NIRS model in %" []
is_a: CO_343:1000003 ! Variable
relationship: variable_of CO_343:0100006 ! %
relationship: variable_of CO_343:0100259 ! NIRS model prediction - computation
relationship: variable_of CO_343:0100263 ! Tuber flour sugar content
created_by: D. Cornut

[Term]
id: CO_343:0100263
name: Tuber flour sugar content
namespace: YamTrait
def: "Tuber flour sugar content" []
is_a: CO_343:1000007 ! Quality_trait

[Term]
id: CO_343:0100264
name: Starch grain size computation
namespace: YamTrait
def: "The starch grain size in µm computed from microscopy image analysis" []
is_a: CO_343:1000003 ! Variable
relationship: variable_of CO_343:0100265 ! Starch grain size
relationship: variable_of CO_343:0100266 ! Microscopy image analysis
relationship: variable_of CO_343:0100267 ! µm
created_by: D. Cornut

[Term]
id: CO_343:0100265
name: Starch grain size
namespace: YamTrait
def: "Mean starch grain size of yam tuber flour" []
is_a: CO_343:1000007 ! Quality_trait

[Term]
id: CO_343:0100266
name: Microscopy image analysis
namespace: YamMethod
def: "Microscopy (10x) image analysis of iodin colored yam tuber flour (0.5mm)" []
is_a: CO_343:1000013 ! Computation
relationship: method_of CO_343:0100265 ! Starch grain size

[Term]
id: CO_343:0100267
name: µm
namespace: YamScale
is_a: CO_343:1000019 ! Numerical
relationship: scale_of CO_343:0100266 ! Microscopy image analysis

[Term]
id: CO_343:0102000
name: cP
namespace: YamScale
def: "Viscosity in centipoise" []
is_a: CO_343:1000019 ! Numerical
relationship: scale_of CO_343:0012000 ! peak viscosity - measurement
relationship: scale_of CO_343:0012001 ! trough viscosity - measurement
relationship: scale_of CO_343:0012002 ! final viscosity - measurement
relationship: scale_of CO_343:0012003 ! breakdown - measurement
relationship: scale_of CO_343:0012004 ! setback - measurement

[Term]
id: CO_343:0102001
name: deg
namespace: YamScale
def: "Degree Celsius" []
is_a: CO_343:1000019 ! Numerical
relationship: scale_of CO_343:0012005 ! pasting temperature - measurement

[Term]
id: CO_343:1000000
name: YamTrait
namespace: YamTrait

[Term]
id: CO_343:1000001
name: Method
namespace: YamMethod

[Term]
id: CO_343:1000002
name: Scale
namespace: YamScale

[Term]
id: CO_343:1000003
name: Variable
namespace: YamTrait
is_a: CO_343:1000000 ! YamTrait

[Term]
id: CO_343:1000005
name: Biotic_stress_trait
namespace: YamTrait
is_a: CO_343:1000000 ! YamTrait

[Term]
id: CO_343:1000006
name: Phenological_trait
namespace: YamTrait
is_a: CO_343:1000000 ! YamTrait

[Term]
id: CO_343:1000007
name: Quality_trait
namespace: YamTrait
is_a: CO_343:1000000 ! YamTrait

[Term]
id: CO_343:1000008
name: Agronomical_trait
namespace: YamTrait
is_a: CO_343:1000000 ! YamTrait

[Term]
id: CO_343:1000009
name: Physiological_trait
namespace: YamTrait
is_a: CO_343:1000000 ! YamTrait

[Term]
id: CO_343:1000010
name: Morphological_trait
namespace: YamTrait
is_a: CO_343:1000000 ! YamTrait

[Term]
id: CO_343:1000011
name: Measurement
namespace: YamMethod
is_a: CO_343:1000001 ! Method

[Term]
id: CO_343:1000012
name: Counting
namespace: YamMethod
is_a: CO_343:1000001 ! Method

[Term]
id: CO_343:1000013
name: Computation
namespace: YamMethod
is_a: CO_343:1000001 ! Method

[Term]
id: CO_343:1000014
name: Estimation
namespace: YamMethod
is_a: CO_343:1000001 ! Method

[Term]
id: CO_343:1000015
name: Ordinal
namespace: YamScale
is_a: CO_343:1000002 ! Scale

[Term]
id: CO_343:1000017
name: Nominal
namespace: YamScale
is_a: CO_343:1000002 ! Scale

[Term]
id: CO_343:1000018
name: Duration
namespace: YamScale
is_a: CO_343:1000002 ! Scale

[Term]
id: CO_343:1000019
name: Numerical
namespace: YamScale
is_a: CO_343:1000002 ! Scale

[Term]
id: CO_343:1000020
name: Time
namespace: YamScale
is_a: CO_343:1000002 ! Scale

[Term]
id: CO_343:1000021
name: Prediction
namespace: YamMethod
is_a: CO_343:1000001 ! Method

[Typedef]
id: method_of
name: method_of

[Typedef]
id: scale_of
name: scale_of

[Typedef]
id: variable_of
name: variable_of

